func_cor_pop.thy
@@ -3,44 +3,40 @@ theory func_cor_pop
 begin
 
 definition p1_post :: "nat \<Rightarrow> assn"
-  where "p1_post t = (\<langle>[t\<diamondop>END]\<^sub>v =\<^sub>b [K_NO_WAIT]\<^sub>n\<rangle>\<^sub>S\<^sub>L \<and>\<^sub>S\<^sub>L Aemp)"
+  where "p1_post t = (\<langle>[END]\<^sub>v =\<^sub>b [K_NO_WAIT]\<^sub>n\<rangle>\<^sub>S\<^sub>L \<and>\<^sub>S\<^sub>L Aemp)"
 
 definition p4_post_noframe :: "nat \<Rightarrow> nat \<Rightarrow> stack_mem \<Rightarrow> assn"
-  where "p4_post_noframe t s st = ([A_Stack]\<^sub>v \<longmapsto> [s]\<^sub>n) ** (stack_node s st \<and>\<^sub>S\<^sub>L \<langle>[t \<diamondop> ADDR]\<^sub>v =\<^sub>b [s]\<^sub>n\<rangle>\<^sub>S\<^sub>L
-      \<and>\<^sub>S\<^sub>L \<langle>[t \<diamondop> NEXT]\<^sub>v =\<^sub>b [stack_next st]\<^sub>n\<rangle>\<^sub>S\<^sub>L \<and>\<^sub>S\<^sub>L \<langle>[t \<diamondop> BASE]\<^sub>v =\<^sub>b [stack_base st]\<^sub>n\<rangle>\<^sub>S\<^sub>L)"
+  where "p4_post_noframe t s st = ([A_Stack]\<^sub>v \<longmapsto> [s]\<^sub>n) ** (stack_node s st \<and>\<^sub>S\<^sub>L \<langle>[ADDR]\<^sub>v =\<^sub>b [s]\<^sub>n\<rangle>\<^sub>S\<^sub>L
+      \<and>\<^sub>S\<^sub>L \<langle>[ NEXT]\<^sub>v =\<^sub>b [stack_next st]\<^sub>n\<rangle>\<^sub>S\<^sub>L \<and>\<^sub>S\<^sub>L \<langle>[ BASE]\<^sub>v =\<^sub>b [stack_base st]\<^sub>n\<rangle>\<^sub>S\<^sub>L)"
   
 lemma safe_p24_noframe : "fvAs \<Gamma> = {} \<Longrightarrow> t \<noteq> NULL \<Longrightarrow>
                           \<Gamma>(Cur := inv_cur, Readyq := inv_readyq, Stack := inv_stack) \<turnstile>
                           {([A_Stack]\<^sub>v \<longmapsto> [s]\<^sub>n) ** stack_node s st}
-                          (t \<^enum> (t \<diamondop> ADDR) :=\<^sub>C \<lbrakk>[A_Stack]\<^sub>v\<rbrakk>) ;;
-                          (t \<^enum> (t \<diamondop> NEXT) :=\<^sub>C \<lbrakk>[t \<diamondop> ADDR]\<^sub>v\<Down>\<^sub>snext\<rbrakk>) ;;
-                          (t \<^enum> (t \<diamondop> BASE) :=\<^sub>C \<lbrakk>[t \<diamondop> ADDR]\<^sub>v\<Down>\<^sub>sbase\<rbrakk>) 
+                          (t \<^enum> ( ADDR) :=\<^sub>C \<lbrakk>[A_Stack]\<^sub>v\<rbrakk>) ;;
+                          (t \<^enum> ( NEXT) :=\<^sub>C \<lbrakk>[ ADDR]\<^sub>v\<Down>\<^sub>snext\<rbrakk>) ;;
+                          (t \<^enum> ( BASE) :=\<^sub>C \<lbrakk>[ ADDR]\<^sub>v\<Down>\<^sub>sbase\<rbrakk>) 
                           {p4_post_noframe t s st}"
-  apply (rule_tac Q = "([A_Stack]\<^sub>v \<longmapsto> [s]\<^sub>n) ** (stack_node s st \<and>\<^sub>S\<^sub>L \<langle>[t \<diamondop> ADDR]\<^sub>v =\<^sub>b [s]\<^sub>n\<rangle>\<^sub>S\<^sub>L
-      \<and>\<^sub>S\<^sub>L \<langle>[t \<diamondop> NEXT]\<^sub>v =\<^sub>b [stack_next st]\<^sub>n\<rangle>\<^sub>S\<^sub>L)" in rule_seq)
-   apply (rule_tac Q = "([A_Stack]\<^sub>v \<longmapsto> [s]\<^sub>n) ** (stack_node s st \<and>\<^sub>S\<^sub>L \<langle>[t \<diamondop> ADDR]\<^sub>v =\<^sub>b [s]\<^sub>n\<rangle>\<^sub>S\<^sub>L)" in rule_seq)
+  apply (rule_tac Q = "([A_Stack]\<^sub>v \<longmapsto> [s]\<^sub>n) ** (stack_node s st \<and>\<^sub>S\<^sub>L \<langle>[ ADDR]\<^sub>v =\<^sub>b [s]\<^sub>n\<rangle>\<^sub>S\<^sub>L
+      \<and>\<^sub>S\<^sub>L \<langle>[ NEXT]\<^sub>v =\<^sub>b [stack_next st]\<^sub>n\<rangle>\<^sub>S\<^sub>L)" in rule_seq)
+   apply (rule_tac Q = "([A_Stack]\<^sub>v \<longmapsto> [s]\<^sub>n) ** (stack_node s st \<and>\<^sub>S\<^sub>L \<langle>[ ADDR]\<^sub>v =\<^sub>b [s]\<^sub>n\<rangle>\<^sub>S\<^sub>L)" in rule_seq)
   apply (rule_tac Pa = "[A_Stack]\<^sub>v \<longmapsto> [s]\<^sub>n ** stack_node s st" and Qa = "([A_Stack]\<^sub>v \<longmapsto> [s]\<^sub>n \<and>\<^sub>S\<^sub>L 
-  \<langle>[t \<diamondop> ADDR]\<^sub>v =\<^sub>b [s]\<^sub>n\<rangle>\<^sub>S\<^sub>L) ** stack_node s st" in safe_assn_equiv, simp add: assn_equiv_reflex)
+  \<langle>[ ADDR]\<^sub>v =\<^sub>b [s]\<^sub>n\<rangle>\<^sub>S\<^sub>L) ** stack_node s st" in safe_assn_equiv, simp add: assn_equiv_reflex)
      apply (simp add: assn_equiv_def) apply auto[1]
     apply (rule rule_frame, rule rule_stm_stack', simp_all)
-  apply (simp add: disjoint_def Thread_Local_def)
-        apply (simp add: Thread_Local_def, simp add: Thread_Local_def)
-      apply (rule rule_read,  simp add: fvA_Gamma2 fvA_inv_cur fvA_inv_readyq fvA_inv_stack)
-      apply (simp add: Thread_Local_def, simp add: Thread_Local_def)
+  apply (simp add: disjoint_def)
+     apply (rule rule_read,  simp add: fvA_Gamma2 fvA_inv_cur fvA_inv_readyq fvA_inv_stack)
     apply (simp add: stack_node_def) apply (rule rule_frame1)
     apply (rule rule_stm_stack' , simp_all)
-        apply (simp add: disjoint_def Thread_Local_def)
-        apply (simp add: stack_node_def Thread_Local_def, simp add: stack_node_def Thread_Local_def)
-    apply (rule stack_node_read_next, simp add: Thread_Local_def)
+        apply (simp add: disjoint_def)
+        apply (simp add: stack_node_def, simp add: stack_node_def)
+    apply (rule stack_node_read_next)
      apply (simp_all add: fvA_Gamma2 fvA_inv_cur fvA_inv_readyq fvA_inv_stack)
-     apply (simp add: Thread_Local_def, simp add: Thread_Local_def)
-    apply (simp add: disjoint_def stm_def Thread_Local_def)
-  apply (simp add: stm_def disjoint_def Thread_Local_def)
+    apply (simp add: disjoint_def stm_def)
   apply (simp add: p4_post_noframe_def, rule rule_frame1, rule rule_stm_stack', simp_all)
-       apply (simp add: disjoint_def Thread_Local_def)
-      apply (simp add: stack_node_def Thread_Local_def, simp add: stack_node_def Thread_Local_def)
-    apply (rule stack_node_read_base1, simp add: Thread_Local_def, simp add: Thread_Local_def)
-     apply (simp_all add: fvA_Gamma2 fvA_inv_cur fvA_inv_readyq fvA_inv_stack disjoint_def stm_def Thread_Local_def)
+       apply (simp add: disjoint_def)
+      apply (simp add: stack_node_def , simp add: stack_node_def)
+    apply (rule stack_node_read_base1, simp, simp)
+     apply (simp_all add: fvA_Gamma2 fvA_inv_cur fvA_inv_readyq fvA_inv_stack disjoint_def stm_def )
   done
 
 definition p4_frame :: " stack_mem \<Rightarrow> assn"
@@ -65,47 +61,47 @@ lemma safe_p24_pre_equiv : "inv_stack1 s st \<equiv>\<^sub>S\<^sub>L  (([A_Stack
 lemma safe_p24 : "fvAs \<Gamma> = {} \<Longrightarrow> t \<noteq> NULL \<Longrightarrow>
                           \<Gamma>(Cur := inv_cur, Readyq := inv_readyq, Stack := inv_stack) \<turnstile>
                           {p1_post t ** inv_stack1 s st}
-                          (t \<^enum> (t \<diamondop> ADDR) :=\<^sub>C \<lbrakk>[A_Stack]\<^sub>v\<rbrakk>) ;;
-                          (t \<^enum> (t \<diamondop> NEXT) :=\<^sub>C \<lbrakk>[t \<diamondop> ADDR]\<^sub>v\<Down>\<^sub>snext\<rbrakk>) ;;
-                          (t \<^enum> (t \<diamondop> BASE) :=\<^sub>C \<lbrakk>[t \<diamondop> ADDR]\<^sub>v\<Down>\<^sub>sbase\<rbrakk>) 
+                          (t \<^enum> ( ADDR) :=\<^sub>C \<lbrakk>[A_Stack]\<^sub>v\<rbrakk>) ;;
+                          (t \<^enum> ( NEXT) :=\<^sub>C \<lbrakk>[ ADDR]\<^sub>v\<Down>\<^sub>snext\<rbrakk>) ;;
+                          (t \<^enum> ( BASE) :=\<^sub>C \<lbrakk>[ ADDR]\<^sub>v\<Down>\<^sub>sbase\<rbrakk>) 
                           {p1_post t ** (p4_post_noframe t s st ** p4_frame st)}"
   apply (rule rule_frame1, rule_tac Pa = "([A_Stack]\<^sub>v \<longmapsto> [s]\<^sub>n) ** stack_node s st ** p4_frame st"
   and Qa = "p4_post_noframe t s st ** p4_frame st" in safe_assn_equiv)
      apply (simp add: assn_equiv_symmetry safe_p24_pre_equiv, simp add: assn_equiv_reflex)
    apply (rule rule_frame, simp add: safe_p24_noframe, simp_all add: disjoint_def)
    apply (simp add: p4_frame_def fvA_is_waitq fvA_buf inv_stack_pt_def inv_stack_buf_waitq_def)
-  by (simp add: p1_post_def stm_def Thread_Local_def)   
+  by (simp add: p1_post_def stm_def )   
 
 definition p5_pre_noframe :: "nat \<Rightarrow> nat \<Rightarrow> stack_mem \<Rightarrow> assn"
-  where "p5_pre_noframe t s st = (stack_node s st \<and>\<^sub>S\<^sub>L \<langle>[t \<diamondop> ADDR]\<^sub>v =\<^sub>b [s]\<^sub>n\<rangle>\<^sub>S\<^sub>L \<and>\<^sub>S\<^sub>L \<langle>[t \<diamondop> NEXT]\<^sub>v =\<^sub>b 
+  where "p5_pre_noframe t s st = (stack_node s st \<and>\<^sub>S\<^sub>L \<langle>[ ADDR]\<^sub>v =\<^sub>b [s]\<^sub>n\<rangle>\<^sub>S\<^sub>L \<and>\<^sub>S\<^sub>L \<langle>[ NEXT]\<^sub>v =\<^sub>b 
   [stack_next st]\<^sub>n\<rangle>\<^sub>S\<^sub>L) ** (buf (stack_base st) (stack_top st) (stack_buf st))"
 
 definition p5_cond :: "stack_mem \<Rightarrow> bool"
   where "p5_cond st = ((stack_next st > stack_base st) \<and> (stack_next st \<le> stack_top st))"
 
 definition p5_post :: "nat \<Rightarrow> nat \<Rightarrow> stack_mem \<Rightarrow> assn"
-  where "p5_post t s st = (stack_node s (st:=\<^sub>n\<^sub>e (stack_next st - 1)) \<and>\<^sub>S\<^sub>L \<langle>[t \<diamondop> ADDR]\<^sub>v =\<^sub>b [s]\<^sub>n\<rangle>\<^sub>S\<^sub>L 
-  \<and>\<^sub>S\<^sub>L \<langle>[t \<diamondop> NEXT]\<^sub>v =\<^sub>b  [stack_next st]\<^sub>n\<rangle>\<^sub>S\<^sub>L) ** (buf (stack_base st) (stack_top st) (stack_buf st))" 
+  where "p5_post t s st = (stack_node s (st:=\<^sub>n\<^sub>e (stack_next st - 1)) \<and>\<^sub>S\<^sub>L \<langle>[ ADDR]\<^sub>v =\<^sub>b [s]\<^sub>n\<rangle>\<^sub>S\<^sub>L 
+  \<and>\<^sub>S\<^sub>L \<langle>[ NEXT]\<^sub>v =\<^sub>b  [stack_next st]\<^sub>n\<rangle>\<^sub>S\<^sub>L) ** (buf (stack_base st) (stack_top st) (stack_buf st))" 
 
 definition p6_pre :: "nat \<Rightarrow> nat \<Rightarrow> stack_mem \<Rightarrow> assn"
   where "p6_pre t s st = (stack_node s (st:=\<^sub>n\<^sub>e (stack_next st - 1)) 
-  \<and>\<^sub>S\<^sub>L \<langle>[t \<diamondop> ADDR]\<^sub>v =\<^sub>b [s]\<^sub>n\<rangle>\<^sub>S\<^sub>L) ** (buf (stack_base st) (stack_top st) (stack_buf st))"
+  \<and>\<^sub>S\<^sub>L \<langle>[ ADDR]\<^sub>v =\<^sub>b [s]\<^sub>n\<rangle>\<^sub>S\<^sub>L) ** (buf (stack_base st) (stack_top st) (stack_buf st))"
 
 lemma p5_post_implies : "p5_post t s st \<sqsubseteq> p6_pre t s st"
   apply (simp add: p5_post_def p6_pre_def implies_def) by blast
 
 definition p6_post :: "nat \<Rightarrow> nat \<Rightarrow> stack_mem \<Rightarrow> assn"
-  where "p6_post t s st = (stack_node s (st:=\<^sub>n\<^sub>e (stack_next st - 1)) \<and>\<^sub>S\<^sub>L \<langle>[t \<diamondop> ADDR]\<^sub>v =\<^sub>b [s]\<^sub>n\<rangle>\<^sub>S\<^sub>L \<and>\<^sub>S\<^sub>L
-  \<langle>[t \<diamondop> NEXT]\<^sub>v =\<^sub>b [stack_next (st:=\<^sub>n\<^sub>e (stack_next st - 1))]\<^sub>n\<rangle>\<^sub>S\<^sub>L) ** 
+  where "p6_post t s st = (stack_node s (st:=\<^sub>n\<^sub>e (stack_next st - 1)) \<and>\<^sub>S\<^sub>L \<langle>[ ADDR]\<^sub>v =\<^sub>b [s]\<^sub>n\<rangle>\<^sub>S\<^sub>L \<and>\<^sub>S\<^sub>L
+  \<langle>[ NEXT]\<^sub>v =\<^sub>b [stack_next (st:=\<^sub>n\<^sub>e (stack_next st - 1))]\<^sub>n\<rangle>\<^sub>S\<^sub>L) ** 
   (buf (stack_base st) (stack_top st) (stack_buf st))"
 
 definition p7_pre' :: "nat \<Rightarrow> nat \<Rightarrow> stack_mem \<Rightarrow> assn"
-  where "p7_pre' t s st = (stack_node s (st:=\<^sub>n\<^sub>e (stack_next st - 1)) \<and>\<^sub>S\<^sub>L \<langle>[t \<diamondop> NEXT]\<^sub>v =\<^sub>b 
+  where "p7_pre' t s st = (stack_node s (st:=\<^sub>n\<^sub>e (stack_next st - 1)) \<and>\<^sub>S\<^sub>L \<langle>[ NEXT]\<^sub>v =\<^sub>b 
   [stack_next st - 1]\<^sub>n\<rangle>\<^sub>S\<^sub>L) ** (buf (stack_base st) (stack_top st) (stack_buf st))"
 
 definition p7_pre :: "nat \<Rightarrow> nat \<Rightarrow> stack_mem \<Rightarrow> assn"
   where "p7_pre t s st = stack_node s (st:=\<^sub>n\<^sub>e (stack_next st - 1)) ** (buf (stack_base st) 
-  (stack_top st) (stack_buf st) \<and>\<^sub>S\<^sub>L \<langle>[t \<diamondop> NEXT]\<^sub>v =\<^sub>b [stack_next st - 1]\<^sub>n\<rangle>\<^sub>S\<^sub>L)"
+  (stack_top st) (stack_buf st) \<and>\<^sub>S\<^sub>L \<langle>[ NEXT]\<^sub>v =\<^sub>b [stack_next st - 1]\<^sub>n\<rangle>\<^sub>S\<^sub>L)"
 
 lemma p6_post_implies : "p6_post t s st \<sqsubseteq> p7_pre t s st"
   apply (rule_tac Q = "p7_pre' t s st" in implies_trans)
@@ -114,22 +110,22 @@ lemma p6_post_implies : "p6_post t s st \<sqsubseteq> p7_pre t s st"
 
 definition p7_post :: "nat \<Rightarrow> nat \<Rightarrow> stack_mem \<Rightarrow> assn"
   where "p7_post t s st = stack_node s (st:=\<^sub>n\<^sub>e (stack_next st - 1)) ** (buf (stack_base st) 
-  (stack_top st) (stack_buf st) \<and>\<^sub>S\<^sub>L \<langle>[t \<diamondop> NEXT]\<^sub>v =\<^sub>b [stack_next st - 1]\<^sub>n\<rangle>\<^sub>S\<^sub>L \<and>\<^sub>S\<^sub>L 
-  \<langle>[t \<diamondop> DATA]\<^sub>v =\<^sub>b [(stack_buf st) ! (stack_next st - 1 - stack_base st)]\<^sub>n\<rangle>\<^sub>S\<^sub>L)"
+  (stack_top st) (stack_buf st) \<and>\<^sub>S\<^sub>L \<langle>[ NEXT]\<^sub>v =\<^sub>b [stack_next st - 1]\<^sub>n\<rangle>\<^sub>S\<^sub>L \<and>\<^sub>S\<^sub>L 
+  \<langle>[ DATA]\<^sub>v =\<^sub>b [(stack_buf st) ! (stack_next st - 1 - stack_base st)]\<^sub>n\<rangle>\<^sub>S\<^sub>L)"
 
 definition p8_pre :: "nat \<Rightarrow> nat \<Rightarrow> stack_mem \<Rightarrow> assn"
   where "p8_pre t s st = stack_node s (st:=\<^sub>n\<^sub>e (stack_next st - 1)) ** (buf (stack_base st) 
-  (stack_top st) (stack_buf st)  \<and>\<^sub>S\<^sub>L \<langle>[t \<diamondop> DATA]\<^sub>v =\<^sub>b [(stack_buf st) ! (stack_next st 
+  (stack_top st) (stack_buf st)  \<and>\<^sub>S\<^sub>L \<langle>[ DATA]\<^sub>v =\<^sub>b [(stack_buf st) ! (stack_next st 
   - 1 - stack_base st)]\<^sub>n\<rangle>\<^sub>S\<^sub>L)"
 
 lemma p7_post_implies : "p7_post t s st \<sqsubseteq> p8_pre t s st"
   apply (simp add: p7_post_def p8_pre_def implies_def) by blast
 
 definition p8_post :: "nat \<Rightarrow> nat \<Rightarrow> stack_mem \<Rightarrow> assn"
-  where "p8_post t s st = (p8_pre t s st \<and>\<^sub>S\<^sub>L \<langle>[(t \<diamondop> RET)]\<^sub>v =\<^sub>b [0]\<^sub>n\<rangle>\<^sub>S\<^sub>L)"
+  where "p8_post t s st = (p8_pre t s st \<and>\<^sub>S\<^sub>L \<langle>[( RET)]\<^sub>v =\<^sub>b [0]\<^sub>n\<rangle>\<^sub>S\<^sub>L)"
 
 definition p9_post :: "nat \<Rightarrow> nat \<Rightarrow> stack_mem \<Rightarrow> assn"
-  where "p9_post t s st = (p8_post t s st \<and>\<^sub>S\<^sub>L \<langle>[(t \<diamondop> END)]\<^sub>v =\<^sub>b [1]\<^sub>n\<rangle>\<^sub>S\<^sub>L)"
+  where "p9_post t s st = (p8_post t s st \<and>\<^sub>S\<^sub>L \<langle>[( END)]\<^sub>v =\<^sub>b [1]\<^sub>n\<rangle>\<^sub>S\<^sub>L)"
 
 definition  p9_post_noframe :: "nat \<Rightarrow> nat \<Rightarrow> stack_mem \<Rightarrow> assn"
   where "p9_post_noframe t s st = stack_node s (st:=\<^sub>n\<^sub>e (stack_next st - 1)) ** buf (stack_base st) 
@@ -138,11 +134,11 @@ definition  p9_post_noframe :: "nat \<Rightarrow> nat \<Rightarrow> stack_mem \<
 lemma safe_p59_noframe : "fvAs \<Gamma> = {} \<Longrightarrow> p5_cond st \<Longrightarrow> t \<noteq> NULL \<Longrightarrow>
                           \<Gamma>(Cur := inv_cur, Readyq := inv_readyq, Stack := inv_stack) \<turnstile>
                           {p5_pre_noframe t s st}
-                            (t \<^enum> \<lbrakk>([t \<diamondop> ADDR]\<^sub>v\<Down>\<^sub>snext)\<rbrakk> :=\<^sub>C [t \<diamondop> NEXT]\<^sub>v -\<^sub>e [1]\<^sub>n);;
-                            (t \<^enum> (t \<diamondop> NEXT) :=\<^sub>C \<lbrakk>[t \<diamondop> ADDR]\<^sub>v\<Down>\<^sub>snext\<rbrakk>) ;;
-                            (t \<^enum> (t \<diamondop> DATA) :=\<^sub>C \<lbrakk>[t \<diamondop> NEXT]\<^sub>v\<rbrakk>) ;;
-                            (t \<^enum> (t \<diamondop> RET) :=\<^sub>C [0]\<^sub>n) ;;
-                            (t \<^enum> (t \<diamondop> END) :=\<^sub>C [1]\<^sub>n) 
+                            (t \<^enum> \<lbrakk>([ ADDR]\<^sub>v\<Down>\<^sub>snext)\<rbrakk> :=\<^sub>C [ NEXT]\<^sub>v -\<^sub>e [1]\<^sub>n);;
+                            (t \<^enum> ( NEXT) :=\<^sub>C \<lbrakk>[ ADDR]\<^sub>v\<Down>\<^sub>snext\<rbrakk>) ;;
+                            (t \<^enum> ( DATA) :=\<^sub>C \<lbrakk>[ NEXT]\<^sub>v\<rbrakk>) ;;
+                            (t \<^enum> ( RET) :=\<^sub>C [0]\<^sub>n) ;;
+                            (t \<^enum> ( END) :=\<^sub>C [1]\<^sub>n) 
                           {p9_post_noframe t s st}"
   apply (rule_tac Q = "p8_post t s st" in rule_seq)
   apply (rule_tac Q = "p7_post t s st" in rule_seq)
@@ -150,48 +146,46 @@ lemma safe_p59_noframe : "fvAs \<Gamma> = {} \<Longrightarrow> p5_cond st \<Long
      apply (rule_tac Q = "p5_post t s st" in rule_seq)
   apply (simp only: p5_pre_noframe_def p5_post_def, rule rule_frame)
        apply (rule rule_stm_stack', simp, simp, simp)
-           apply (simp add: stack_node_def Thread_Local_def, simp add: Thread_Local_def)
-         apply (simp add: stack_node_def Thread_Local_def)
-       apply (rule stack_node_write_next_minus1, simp add: Thread_Local_def)
+           apply (simp add: stack_node_def , simp add: )
+         apply (simp add: stack_node_def )
+       apply (rule stack_node_write_next_minus1, simp add: )
         apply (simp_all add: fvA_Gamma2 fvA_inv_cur fvA_inv_readyq fvA_buf fvA_inv_stack)
-       apply (simp add: Thread_Local_def, simp add: Thread_Local_def)
      apply (rule_tac P = "p6_pre t s st" and Q = "p6_post t s st" in rule_conseq)
   apply (simp only: p6_pre_def p6_post_def, rule rule_frame)
         apply (rule rule_stm_stack', simp_all)
-            apply (simp add: disjoint_def Thread_Local_def)
-           apply (simp add: stack_node_def Thread_Local_def, simp add: stack_node_def Thread_Local_def)
-         apply (rule stack_node_read_next, simp add: Thread_Local_def)
+            apply (simp add: disjoint_def )
+           apply (simp add: stack_node_def , simp add: stack_node_def )
+         apply (rule stack_node_read_next, simp add: )
          apply (simp_all add: fvA_Gamma2 fvA_buf fvA_inv_cur fvA_inv_readyq fvA_inv_stack)
-        apply (simp add: Thread_Local_def, simp add: Thread_Local_def, simp add: Thread_Local_def)
       apply (simp add: p5_post_implies, simp add: implies_def)
     apply (rule_tac P = "p7_pre t s st" and Q = "p7_post t s st" in rule_conseq)
       apply (simp only: p7_pre_def p7_post_def, rule rule_frame1, rule rule_stm_stack', simp)
-            apply (simp add: disjoint_def Thread_Local_def)
-           apply (simp add: fvA_buf Thread_Local_def, simp)
-  apply (simp add: fvA_buf Thread_Local_def)
-        apply (rule read_buf_with_var, simp add: fvA_Gamma2 fvA_inv_readyq fvA_inv_cur fvA_inv_stack Thread_Local_def)
+            apply (simp add: disjoint_def )
+           apply (simp add: fvA_buf , simp)
+  apply (simp add: fvA_buf )
+        apply (rule read_buf_with_var, simp add: fvA_Gamma2 fvA_inv_readyq fvA_inv_cur fvA_inv_stack )
         apply (simp add: p5_cond_def) apply linarith 
-        apply (simp add: Thread_Local_def)
+        apply (simp add: )
       apply (simp add: stack_node_def, simp add: p6_post_implies, simp add: implies_def)
    apply (rule_tac P = "p8_pre t s st" and Q = "p8_post t s st" in rule_conseq)
      apply (rule rule_stm_stack', simp_all)
-         apply (simp add: disjoint_def Thread_Local_def)
-        apply (simp add: p8_pre_def fvA_buf stack_node_def Thread_Local_def)
-  apply (simp add: p8_pre_def fvA_buf stack_node_def Thread_Local_def)
+         apply (simp add: disjoint_def )
+        apply (simp add: p8_pre_def fvA_buf stack_node_def )
+  apply (simp add: p8_pre_def fvA_buf stack_node_def )
   apply (simp add: p8_post_def, rule rule_assign_num1)
-      apply ( simp add: fvA_Gamma2 fvA_inv_readyq fvA_inv_cur fvA_inv_stack p8_pre_def stack_node_def 
-      fvA_buf Thread_Local_def, simp add: Thread_Local_def)
+      apply (simp add: fvA_Gamma2 fvA_inv_readyq fvA_inv_cur fvA_inv_stack p8_pre_def stack_node_def 
+      fvA_buf)
     apply (simp add: p7_post_implies, simp add: implies_def)
   apply (rule rule_stm_stack', simp_all) 
-      apply (simp add: disjoint_def Thread_Local_def)
-     apply (simp add: p8_post_def p8_pre_def fvA_buf stack_node_def Thread_Local_def)
-  apply (simp add: p8_post_def p8_pre_def fvA_buf stack_node_def Thread_Local_def)
+      apply (simp add: disjoint_def )
+     apply (simp add: p8_post_def p8_pre_def fvA_buf stack_node_def )
+  apply (simp add: p8_post_def p8_pre_def fvA_buf stack_node_def )
   apply (rule_tac P = "p8_post t s st" and Q = "p9_post t s st" in rule_conseq)
   apply (simp add: p9_post_def, rule rule_assign_num1)
      apply (simp add: fvA_Gamma2 fvA_inv_readyq fvA_inv_cur fvA_inv_stack p8_post_def p8_pre_def 
-      stack_node_def fvA_buf Thread_Local_def)
+      stack_node_def fvA_buf )
    apply (simp_all add: implies_def, simp add: p9_post_def p8_post_def p8_pre_def p9_post_noframe_def)
-   apply blast apply (simp add: Thread_Local_def)
+   apply blast 
   done
 
 definition p5_cond_if :: "stack_mem \<Rightarrow> bool"
@@ -236,10 +230,10 @@ lemma p5_pre_implies_aux : "P1 ** P2 ** (P3 ** P4 \<and>\<^sub>S\<^sub>L \<langl
    stack_node_equiv1_aux stack_node_equiv2_aux, simp add: assn_equiv_reflex)
   apply (simp add: assn_equiv_def) by blast
 
-lemma p5_pre_implies : " (p4_post_noframe t s st \<and>\<^sub>S\<^sub>L \<langle>[t\<diamondop>NEXT]\<^sub>v >\<^sub>b [t\<diamondop>BASE]\<^sub>v\<rangle>\<^sub>S\<^sub>L) ** p4_frame st 
+lemma p5_pre_implies : " (p4_post_noframe t s st \<and>\<^sub>S\<^sub>L \<langle>[NEXT]\<^sub>v >\<^sub>b [BASE]\<^sub>v\<rangle>\<^sub>S\<^sub>L) ** p4_frame st 
                           \<sqsubseteq> p5_pre_noframe t s st ** p5_frame s st"
-  apply (rule_tac Q = "[A_Stack]\<^sub>v \<longmapsto> [s]\<^sub>n ** (stack_node s st \<and>\<^sub>S\<^sub>L  \<langle>[t\<diamondop>ADDR]\<^sub>v =\<^sub>b [s]\<^sub>n\<rangle>\<^sub>S\<^sub>L 
-  \<and>\<^sub>S\<^sub>L \<langle>[t\<diamondop>NEXT]\<^sub>v =\<^sub>b [stack_next st]\<^sub>n\<rangle>\<^sub>S\<^sub>L ) ** p4_frame st" in implies_trans)
+  apply (rule_tac Q = "[A_Stack]\<^sub>v \<longmapsto> [s]\<^sub>n ** (stack_node s st \<and>\<^sub>S\<^sub>L  \<langle>[ADDR]\<^sub>v =\<^sub>b [s]\<^sub>n\<rangle>\<^sub>S\<^sub>L 
+  \<and>\<^sub>S\<^sub>L \<langle>[NEXT]\<^sub>v =\<^sub>b [stack_next st]\<^sub>n\<rangle>\<^sub>S\<^sub>L ) ** p4_frame st" in implies_trans)
    apply (simp add: p4_post_noframe_def implies_def) apply auto
   apply (rule equiv_implies, simp add: p4_frame_def p5_pre_noframe_def p5_frame_def)
   by (simp add: inv_stack_buf_waitq_def inv_stack_pt_def p5_pre_implies_aux)
@@ -247,39 +241,39 @@ lemma p5_pre_implies : " (p4_post_noframe t s st \<and>\<^sub>S\<^sub>L \<langle
 lemma safe_p59 : "fvAs \<Gamma> = {} \<Longrightarrow> p5_cond_if st \<Longrightarrow> t \<noteq> NULL \<Longrightarrow>
                           \<Gamma>(Cur := inv_cur, Readyq := inv_readyq, Stack := inv_stack) \<turnstile>
                           {p5_pre_noframe t s st ** p5_frame s st}
-                            (t \<^enum> \<lbrakk>([t \<diamondop> ADDR]\<^sub>v\<Down>\<^sub>snext)\<rbrakk> :=\<^sub>C [t \<diamondop> NEXT]\<^sub>v -\<^sub>e [1]\<^sub>n);;
-                            (t \<^enum> (t \<diamondop> NEXT) :=\<^sub>C \<lbrakk>[t \<diamondop> ADDR]\<^sub>v\<Down>\<^sub>snext\<rbrakk>) ;;
-                            (t \<^enum> (t \<diamondop> DATA) :=\<^sub>C \<lbrakk>[t \<diamondop> NEXT]\<^sub>v\<rbrakk>) ;;
-                            (t \<^enum> (t \<diamondop> RET) :=\<^sub>C [0]\<^sub>n) ;;
-                            (t \<^enum> (t \<diamondop> END) :=\<^sub>C [1]\<^sub>n) 
+                            (t \<^enum> \<lbrakk>([ ADDR]\<^sub>v\<Down>\<^sub>snext)\<rbrakk> :=\<^sub>C [ NEXT]\<^sub>v -\<^sub>e [1]\<^sub>n);;
+                            (t \<^enum> ( NEXT) :=\<^sub>C \<lbrakk>[ ADDR]\<^sub>v\<Down>\<^sub>snext\<rbrakk>) ;;
+                            (t \<^enum> ( DATA) :=\<^sub>C \<lbrakk>[ NEXT]\<^sub>v\<rbrakk>) ;;
+                            (t \<^enum> ( RET) :=\<^sub>C [0]\<^sub>n) ;;
+                            (t \<^enum> ( END) :=\<^sub>C [1]\<^sub>n) 
                           {inv_stack1 s (st:=\<^sub>n\<^sub>e (stack_next st - 1))}"
   apply (rule_tac Pa = "p5_pre_noframe t s st ** p5_frame s st" and Qa = "p9_post_noframe t 
   s st ** p5_frame s st" in safe_assn_equiv, simp add: assn_equiv_reflex)
   using p9_post_equiv apply auto[1] apply (rule rule_frame, rule safe_p59_noframe, simp)
     apply (simp add: p5_cond_if_def p5_cond_def, simp)
   apply (simp add: p5_frame_def fvA_is_waitq stm_def)
-  by (simp add:  inv_stack_buf_waitq_def inv_stack_pt_def  disjoint_def Thread_Local_def)
+  by (simp add:  inv_stack_buf_waitq_def inv_stack_pt_def  disjoint_def )
 
 lemma safe_p1011_noframe : "fvAs \<Gamma> = {} \<Longrightarrow> t \<noteq> NULL \<Longrightarrow>
                           \<Gamma>(Cur := inv_cur, Readyq := inv_readyq, Stack := inv_stack) \<turnstile> 
                           {inv_stack1 s st}  
-                         (t \<^enum> (t \<diamondop> RET) :=\<^sub>C ([EBUSY]\<^sub>n)) ;;
-                         (t \<^enum> (t \<diamondop> END) :=\<^sub>C ([1]\<^sub>n)) 
+                         (t \<^enum> ( RET) :=\<^sub>C ([EBUSY]\<^sub>n)) ;;
+                         (t \<^enum> ( END) :=\<^sub>C ([1]\<^sub>n)) 
                           {inv_stack1 s st}"
-  apply (rule_tac Q = "inv_stack1 s st \<and>\<^sub>S\<^sub>L \<langle>[t \<diamondop> RET]\<^sub>v =\<^sub>b [EBUSY]\<^sub>n\<rangle>\<^sub>S\<^sub>L" in rule_seq)
-   apply (rule rule_stm_stack', simp, simp add: disjoint_def Thread_Local_def)
-       apply (simp add: inv_stack1_def fvA_is_stack Thread_Local_def, simp)
-  apply (simp add: inv_stack1_def fvA_is_stack Thread_Local_def)
+  apply (rule_tac Q = "inv_stack1 s st \<and>\<^sub>S\<^sub>L \<langle>[ RET]\<^sub>v =\<^sub>b [EBUSY]\<^sub>n\<rangle>\<^sub>S\<^sub>L" in rule_seq)
+   apply (rule rule_stm_stack', simp, simp add: disjoint_def )
+       apply (simp add: inv_stack1_def fvA_is_stack , simp)
+  apply (simp add: inv_stack1_def fvA_is_stack )
     apply (rule rule_assign_num1, simp add: fvA_Gamma2 fvA_inv_cur fvA_inv_readyq)
-    apply (simp add: inv_stack1_def fvA_is_stack fvA_inv_stack Thread_Local_def)
-   apply (simp add: Thread_Local_def)
-  apply (rule_tac P = "inv_stack1 s st" and Q = "inv_stack1 s st \<and>\<^sub>S\<^sub>L \<langle>[t\<diamondop>END]\<^sub>v =\<^sub>b [1]\<^sub>n\<rangle>\<^sub>S\<^sub>L" in rule_conseq)
-    apply (rule rule_stm_stack', simp, simp add: disjoint_def Thread_Local_def)
-        apply (simp add: inv_stack1_def fvA_is_stack Thread_Local_def, simp)
-      apply (simp add: inv_stack1_def fvA_is_stack Thread_Local_def)
+    apply (simp add: inv_stack1_def fvA_is_stack fvA_inv_stack )
+   apply (simp add: )
+  apply (rule_tac P = "inv_stack1 s st" and Q = "inv_stack1 s st \<and>\<^sub>S\<^sub>L \<langle>[END]\<^sub>v =\<^sub>b [1]\<^sub>n\<rangle>\<^sub>S\<^sub>L" in rule_conseq)
+    apply (rule rule_stm_stack', simp, simp add: disjoint_def )
+        apply (simp add: inv_stack1_def fvA_is_stack , simp)
+      apply (simp add: inv_stack1_def fvA_is_stack )
     apply (rule rule_assign_num1, simp add: fvA_Gamma2 fvA_inv_cur fvA_inv_readyq)
-     apply (simp add: inv_stack1_def fvA_is_stack fvA_inv_stack Thread_Local_def)
-  apply (simp add: Thread_Local_def)
+     apply (simp add: inv_stack1_def fvA_is_stack fvA_inv_stack )
+  apply (simp add: )
   by (simp_all add: implies_def)
 
 lemma p10_pre_implies : "p4_post_noframe t s st ** p4_frame st \<sqsubseteq> inv_stack1 s st"
@@ -289,21 +283,21 @@ lemma p10_pre_implies : "p4_post_noframe t s st ** p4_frame st \<sqsubseteq> inv
   by (simp add: assn_equiv_symmetry inv_stack_buf_waitq_def inv_stack_pt_def safe_p24_pre_equiv_aux)
 
 definition p12_pre_noframe :: "nat \<Rightarrow> tcb \<Rightarrow> nat \<Rightarrow> stack_mem \<Rightarrow> assn"
-  where "p12_pre_noframe t x s st = (inv_cur1 t x) ** (stack_node s st \<and>\<^sub>S\<^sub>L \<langle>[t \<diamondop> ADDR]\<^sub>v =\<^sub>b [s]\<^sub>n\<rangle>\<^sub>S\<^sub>L) 
+  where "p12_pre_noframe t x s st = (inv_cur1 t x) ** (stack_node s st \<and>\<^sub>S\<^sub>L \<langle>[ ADDR]\<^sub>v =\<^sub>b [s]\<^sub>n\<rangle>\<^sub>S\<^sub>L) 
   ** thread_wait_sl (stack_wait st) (stack_tcbs st)"
 
 definition p12_post :: "nat \<Rightarrow> tcb \<Rightarrow> nat \<Rightarrow> stack_mem \<Rightarrow> assn"
-  where "p12_post t x s st = (inv_cur1 t x) ** (stack_node s st \<and>\<^sub>S\<^sub>L \<langle>[t \<diamondop> ADDR]\<^sub>v =\<^sub>b [s]\<^sub>n\<rangle>\<^sub>S\<^sub>L \<and>\<^sub>S\<^sub>L 
-  \<langle>[t \<diamondop> FIRST_PENDING_THREAD]\<^sub>v =\<^sub>b [stack_wait st]\<^sub>n\<rangle>\<^sub>S\<^sub>L) ** thread_wait_sl (stack_wait st) (stack_tcbs st)"
+  where "p12_post t x s st = (inv_cur1 t x) ** (stack_node s st \<and>\<^sub>S\<^sub>L \<langle>[ ADDR]\<^sub>v =\<^sub>b [s]\<^sub>n\<rangle>\<^sub>S\<^sub>L \<and>\<^sub>S\<^sub>L 
+  \<langle>[ FIRST_PENDING_THREAD]\<^sub>v =\<^sub>b [stack_wait st]\<^sub>n\<rangle>\<^sub>S\<^sub>L) ** thread_wait_sl (stack_wait st) (stack_tcbs st)"
 
 definition p13_pre' :: "nat \<Rightarrow> tcb \<Rightarrow> nat \<Rightarrow> stack_mem \<Rightarrow> assn"
-  where "p13_pre' t x s st = (inv_cur1 t x \<and>\<^sub>S\<^sub>L  \<langle>[t \<diamondop> FIRST_PENDING_THREAD]\<^sub>v =\<^sub>b 
-  [stack_wait st]\<^sub>n\<rangle>\<^sub>S\<^sub>L) ** (stack_node s st \<and>\<^sub>S\<^sub>L \<langle>[t \<diamondop> ADDR]\<^sub>v =\<^sub>b [s]\<^sub>n\<rangle>\<^sub>S\<^sub>L) ** thread_wait_sl 
+  where "p13_pre' t x s st = (inv_cur1 t x \<and>\<^sub>S\<^sub>L  \<langle>[ FIRST_PENDING_THREAD]\<^sub>v =\<^sub>b 
+  [stack_wait st]\<^sub>n\<rangle>\<^sub>S\<^sub>L) ** (stack_node s st \<and>\<^sub>S\<^sub>L \<langle>[ ADDR]\<^sub>v =\<^sub>b [s]\<^sub>n\<rangle>\<^sub>S\<^sub>L) ** thread_wait_sl 
   (stack_wait st) (stack_tcbs st)"
 
 definition p13_pre :: "nat \<Rightarrow> tcb \<Rightarrow> nat \<Rightarrow> stack_mem \<Rightarrow> assn"
-  where "p13_pre t x s st = (([A_Cur]\<^sub>v \<longmapsto> [t]\<^sub>n) ** ((thread_node t x) \<and>\<^sub>S\<^sub>L \<langle>[t \<diamondop> FIRST_PENDING_THREAD]\<^sub>v =\<^sub>b 
-  [stack_wait st]\<^sub>n\<rangle>\<^sub>S\<^sub>L)) ** (stack_node s st \<and>\<^sub>S\<^sub>L \<langle>[t \<diamondop> ADDR]\<^sub>v =\<^sub>b [s]\<^sub>n\<rangle>\<^sub>S\<^sub>L) ** thread_wait_sl 
+  where "p13_pre t x s st = (([A_Cur]\<^sub>v \<longmapsto> [t]\<^sub>n) ** ((thread_node t x) \<and>\<^sub>S\<^sub>L \<langle>[ FIRST_PENDING_THREAD]\<^sub>v =\<^sub>b 
+  [stack_wait st]\<^sub>n\<rangle>\<^sub>S\<^sub>L)) ** (stack_node s st \<and>\<^sub>S\<^sub>L \<langle>[ ADDR]\<^sub>v =\<^sub>b [s]\<^sub>n\<rangle>\<^sub>S\<^sub>L) ** thread_wait_sl 
   (stack_wait st) (stack_tcbs st)" 
 
 lemma p12_post_equiv : "p12_post t x s st \<equiv>\<^sub>S\<^sub>L p13_pre' t x s st"
@@ -319,23 +313,23 @@ lemma p12_post_implies : "p12_post t x s st \<sqsubseteq> p13_pre t x s st"
 
 definition p13_post :: "nat \<Rightarrow> tcb \<Rightarrow> nat \<Rightarrow> stack_mem \<Rightarrow> assn"
   where "p13_post t x s st = (([A_Cur]\<^sub>v \<longmapsto> [t]\<^sub>n) ** (thread_node t (x:=\<^sub>n\<^sub>x (stack_wait st)) \<and>\<^sub>S\<^sub>L 
-  \<langle>[t \<diamondop> FIRST_PENDING_THREAD]\<^sub>v =\<^sub>b [stack_wait st]\<^sub>n\<rangle>\<^sub>S\<^sub>L)) ** (stack_node s st \<and>\<^sub>S\<^sub>L \<langle>[t \<diamondop> ADDR]\<^sub>v =\<^sub>b [s]\<^sub>n\<rangle>\<^sub>S\<^sub>L) 
+  \<langle>[ FIRST_PENDING_THREAD]\<^sub>v =\<^sub>b [stack_wait st]\<^sub>n\<rangle>\<^sub>S\<^sub>L)) ** (stack_node s st \<and>\<^sub>S\<^sub>L \<langle>[ ADDR]\<^sub>v =\<^sub>b [s]\<^sub>n\<rangle>\<^sub>S\<^sub>L) 
   ** thread_wait_sl (stack_wait st) (stack_tcbs st)"
 
 definition p14_pre :: "nat \<Rightarrow> tcb \<Rightarrow> nat \<Rightarrow> stack_mem \<Rightarrow> assn"
   where "p14_pre t x s st = (([A_Cur]\<^sub>v \<longmapsto> [t]\<^sub>n) ** (thread_node t (x:=\<^sub>n\<^sub>x (stack_wait st)))) ** 
-  (stack_node s st \<and>\<^sub>S\<^sub>L \<langle>[t \<diamondop> ADDR]\<^sub>v =\<^sub>b [s]\<^sub>n\<rangle>\<^sub>S\<^sub>L) ** thread_wait_sl (stack_wait st) (stack_tcbs st)"
+  (stack_node s st \<and>\<^sub>S\<^sub>L \<langle>[ ADDR]\<^sub>v =\<^sub>b [s]\<^sub>n\<rangle>\<^sub>S\<^sub>L) ** thread_wait_sl (stack_wait st) (stack_tcbs st)"
 
 lemma p13_post_implies : "p13_post t x s st \<sqsubseteq> p14_pre t x s st"
   apply (simp add: p13_post_def p14_pre_def implies_def) by blast
 
 definition p14_post :: "nat \<Rightarrow> tcb \<Rightarrow> nat \<Rightarrow> stack_mem \<Rightarrow> assn"
   where "p14_post t x s st = (([A_Cur]\<^sub>v \<longmapsto> [t]\<^sub>n) ** (thread_node t (x:=\<^sub>n\<^sub>x (stack_wait st) :=\<^sub>s\<^sub>t BLOCKED))) ** 
-  (stack_node s st \<and>\<^sub>S\<^sub>L \<langle>[t \<diamondop> ADDR]\<^sub>v =\<^sub>b [s]\<^sub>n\<rangle>\<^sub>S\<^sub>L) ** thread_wait_sl (stack_wait st) (stack_tcbs st)"
+  (stack_node s st \<and>\<^sub>S\<^sub>L \<langle>[ ADDR]\<^sub>v =\<^sub>b [s]\<^sub>n\<rangle>\<^sub>S\<^sub>L) ** thread_wait_sl (stack_wait st) (stack_tcbs st)"
 
 definition p15_post :: "nat \<Rightarrow> tcb \<Rightarrow> nat \<Rightarrow> stack_mem \<Rightarrow> assn"
   where "p15_post t x s st = (([A_Cur]\<^sub>v \<longmapsto> [t]\<^sub>n) ** (thread_node t (x:=\<^sub>n\<^sub>x (stack_wait st) :=\<^sub>s\<^sub>t BLOCKED))) ** 
-  (stack_node s (st:=\<^sub>w\<^sub>a t) \<and>\<^sub>S\<^sub>L \<langle>[t \<diamondop> ADDR]\<^sub>v =\<^sub>b [s]\<^sub>n\<rangle>\<^sub>S\<^sub>L) ** thread_wait_sl (stack_wait st) (stack_tcbs st)"
+  (stack_node s (st:=\<^sub>w\<^sub>a t) \<and>\<^sub>S\<^sub>L \<langle>[ ADDR]\<^sub>v =\<^sub>b [s]\<^sub>n\<rangle>\<^sub>S\<^sub>L) ** thread_wait_sl (stack_wait st) (stack_tcbs st)"
 
 definition p16_pre :: "nat \<Rightarrow> tcb \<Rightarrow> nat \<Rightarrow> stack_mem \<Rightarrow> assn"
   where "p16_pre t x s st = (([A_Cur]\<^sub>v \<longmapsto> [t]\<^sub>n) ** (thread_node t (x:=\<^sub>n\<^sub>x (stack_wait st) :=\<^sub>s\<^sub>t BLOCKED))) ** 
@@ -364,10 +358,10 @@ lemma p16_post_equiv : "p16_post t x s st \<equiv>\<^sub>S\<^sub>L p16_post_nofr
 lemma safe_p1216_noframe : "fvAs \<Gamma> = {} \<Longrightarrow>
                           \<Gamma>(Cur := inv_cur, Readyq := inv_readyq, Stack := inv_stack) \<turnstile> 
                           {p12_pre_noframe t x s st}  
-                          (t \<diamondop> FIRST_PENDING_THREAD) :=\<^sub>C \<lbrakk>[t \<diamondop> ADDR]\<^sub>v\<Down>\<^sub>swait\<rbrakk> ;;                  
-                          \<lbrakk>[t]\<^sub>n\<Down>\<^sub>tnext\<rbrakk> :=\<^sub>C [t \<diamondop> FIRST_PENDING_THREAD]\<^sub>v ;;
+                          ( FIRST_PENDING_THREAD) :=\<^sub>C \<lbrakk>[ ADDR]\<^sub>v\<Down>\<^sub>swait\<rbrakk> ;;                  
+                          \<lbrakk>[t]\<^sub>n\<Down>\<^sub>tnext\<rbrakk> :=\<^sub>C [ FIRST_PENDING_THREAD]\<^sub>v ;;
                           \<lbrakk>[t]\<^sub>n\<Down>\<^sub>tstate\<rbrakk> :=\<^sub>C [BLOCKED]\<^sub>n ;;
-                          \<lbrakk>[t \<diamondop> ADDR]\<^sub>v\<Down>\<^sub>swait\<rbrakk> :=\<^sub>C [t]\<^sub>n ;;
+                          \<lbrakk>[ ADDR]\<^sub>v\<Down>\<^sub>swait\<rbrakk> :=\<^sub>C [t]\<^sub>n ;;
                           \<lbrakk>[A_Cur]\<^sub>v\<rbrakk> :=\<^sub>C [NULL]\<^sub>n 
                           {p16_post_noframe t x s st}"
    apply (rule_tac Q = "p15_post t x s st" in rule_seq)
@@ -375,10 +369,9 @@ lemma safe_p1216_noframe : "fvAs \<Gamma> = {} \<Longrightarrow>
      apply (rule_tac Q = "p13_post t x s st" in rule_seq)
       apply (rule_tac Q = "p12_post t x s st" in rule_seq)
         apply (simp add: p12_pre_noframe_def p12_post_def, rule rule_frame2)
-         apply (rule stack_node_read_wait, simp add: Thread_Local_def)
+         apply (rule stack_node_read_wait, simp add: )
           apply (simp_all add: fvA_Gamma2 fvA_inv_readyq fvA_is_cur fvA_thread_wait_sl fvA_inv_stack fvA_inv_cur)
-         apply (simp add: Thread_Local_def, simp add: Thread_Local_def)
-       apply (simp add: inv_cur1_def fvA_is_cur disjoint_def Thread_Local_def)
+       apply (simp add: inv_cur1_def fvA_is_cur disjoint_def )
       apply (rule_tac P = "p13_pre t x s st" and Q = "p13_post t x s st" in rule_conseq)
         apply (simp add: p13_pre_def p13_post_def, rule rule_frame, rule rule_frame, rule rule_frame1)
            apply (rule thread_node_write_next_var, simp_all, simp add: p12_post_implies, simp add: implies_def)
@@ -386,7 +379,7 @@ lemma safe_p1216_noframe : "fvAs \<Gamma> = {} \<Longrightarrow>
        apply (simp add: p14_pre_def p14_post_def, rule rule_frame, rule rule_frame, rule rule_frame1)
           apply (simp add: thread_node_write_st, simp_all, simp add: p13_post_implies, simp add: implies_def)
     apply (simp add: p14_post_def p15_post_def, rule rule_frame, rule rule_frame1, rule stack_node_write_wait)
-      apply (simp_all, simp add: fvA_Gamma2 fvA_inv_readyq fvA_inv_stack fvA_inv_cur Thread_Local_def)
+      apply (simp_all, simp add: fvA_Gamma2 fvA_inv_readyq fvA_inv_stack fvA_inv_cur )
    apply (rule_tac P = "p16_pre t x s st" and Q = "p16_post t x s st" in rule_conseq)
      apply (simp add: p16_pre_def p16_post_def, intro rule_frame)
        apply (rule rule_write, simp_all, simp add: p15_post_implies)
@@ -425,17 +418,17 @@ lemma p16_post_frame_equiv : " stack_base st = stack_next st \<Longrightarrow> p
 lemma safe_p1216 : "stack_base st = stack_next st \<Longrightarrow> fvAs \<Gamma> = {} \<Longrightarrow>
                           \<Gamma>(Cur := inv_cur, Readyq := inv_readyq, Stack := inv_stack) \<turnstile> 
                           {p12_pre_noframe t x s st ** p12_frame s st}  
-                          (t \<diamondop> FIRST_PENDING_THREAD) :=\<^sub>C \<lbrakk>[t \<diamondop> ADDR]\<^sub>v\<Down>\<^sub>swait\<rbrakk> ;;                  
-                          \<lbrakk>[t]\<^sub>n\<Down>\<^sub>tnext\<rbrakk> :=\<^sub>C [t \<diamondop> FIRST_PENDING_THREAD]\<^sub>v ;;
+                          ( FIRST_PENDING_THREAD) :=\<^sub>C \<lbrakk>[ ADDR]\<^sub>v\<Down>\<^sub>swait\<rbrakk> ;;                  
+                          \<lbrakk>[t]\<^sub>n\<Down>\<^sub>tnext\<rbrakk> :=\<^sub>C [ FIRST_PENDING_THREAD]\<^sub>v ;;
                           \<lbrakk>[t]\<^sub>n\<Down>\<^sub>tstate\<rbrakk> :=\<^sub>C [BLOCKED]\<^sub>n ;;
-                          \<lbrakk>[t \<diamondop> ADDR]\<^sub>v\<Down>\<^sub>swait\<rbrakk> :=\<^sub>C [t]\<^sub>n ;;
+                          \<lbrakk>[ ADDR]\<^sub>v\<Down>\<^sub>swait\<rbrakk> :=\<^sub>C [t]\<^sub>n ;;
                           \<lbrakk>[A_Cur]\<^sub>v\<rbrakk> :=\<^sub>C [NULL]\<^sub>n
                           {[A_Cur]\<^sub>v \<longmapsto> [NULL]\<^sub>n ** inv_stack1 s (st :=\<^sub>w\<^sub>a t :=\<^sub>t\<^sub>c ((x :=\<^sub>n\<^sub>x (stack_wait st) :=\<^sub>s\<^sub>t 
                           BLOCKED) # (stack_tcbs st)))}"
   apply (rule_tac Pa = "p12_pre_noframe t x s st ** p12_frame s st" and Qa = "p16_post_noframe t x s st 
   ** p12_frame s st" in safe_assn_equiv, simp add: assn_equiv_reflex, simp add: p16_post_frame_equiv)
   apply (rule rule_frame, simp add: safe_p1216_noframe, simp add: p12_frame_def fvA_buf)
-  by (simp add: disjoint_def inv_stack_buf_waitq_def inv_stack_pt_def Thread_Local_def)
+  by (simp add: disjoint_def inv_stack_buf_waitq_def inv_stack_pt_def )
 
 lemma p12_pre_frame_aux : "P1 ** P2 ** (P3 ** P4 \<and>\<^sub>S\<^sub>L \<langle>P5\<rangle>\<^sub>S\<^sub>L \<and>\<^sub>S\<^sub>L \<langle>P6\<rangle>\<^sub>S\<^sub>L) ** P7 \<equiv>\<^sub>S\<^sub>L
                           P7 ** P2 ** P3 ** (P1 ** P4 \<and>\<^sub>S\<^sub>L \<langle>P5\<rangle>\<^sub>S\<^sub>L \<and>\<^sub>S\<^sub>L \<langle>P6\<rangle>\<^sub>S\<^sub>L)"
@@ -453,10 +446,10 @@ lemma p12_pre_frame_aux : "P1 ** P2 ** (P3 ** P4 \<and>\<^sub>S\<^sub>L \<langle
 
 lemma p12_pre_frame_implies : " p4_post_noframe t s st ** p4_frame st ** inv_cur1 t x \<sqsubseteq>
                                 p12_pre_noframe t x s st ** p12_frame s st "
-  apply (rule_tac Q = "[A_Stack]\<^sub>v \<longmapsto> [s]\<^sub>n ** (stack_node s st \<and>\<^sub>S\<^sub>L \<langle>[t\<diamondop>ADDR]\<^sub>v =\<^sub>b [s]\<^sub>n\<rangle>\<^sub>S\<^sub>L) **
+  apply (rule_tac Q = "[A_Stack]\<^sub>v \<longmapsto> [s]\<^sub>n ** (stack_node s st \<and>\<^sub>S\<^sub>L \<langle>[ADDR]\<^sub>v =\<^sub>b [s]\<^sub>n\<rangle>\<^sub>S\<^sub>L) **
     p4_frame st ** inv_cur1 t x" in implies_trans, simp add: p4_post_noframe_def)
    apply (simp add: implies_def) apply blast apply (rule equiv_implies)
-  apply (rule_tac Q = "(inv_cur1 t x) ** (stack_node s st \<and>\<^sub>S\<^sub>L \<langle>[t \<diamondop> ADDR]\<^sub>v =\<^sub>b [s]\<^sub>n\<rangle>\<^sub>S\<^sub>L) 
+  apply (rule_tac Q = "(inv_cur1 t x) ** (stack_node s st \<and>\<^sub>S\<^sub>L \<langle>[ ADDR]\<^sub>v =\<^sub>b [s]\<^sub>n\<rangle>\<^sub>S\<^sub>L) 
   ** is_waitq (stack_wait st) (stack_tcbs st) ** p12_frame s st" in assn_equiv_trans)
   apply (simp add: p4_frame_def p12_frame_def inv_stack_buf_waitq_def inv_stack_pt_def)
    apply (simp add: p12_pre_frame_aux, rule assn_equiv_cong_star)
@@ -466,67 +459,69 @@ lemma p12_pre_frame_implies : " p4_post_noframe t s st ** p4_frame st ** inv_cur
 lemma rule_inv_stack : "\<forall>s st. \<Gamma> \<turnstile> {P ** inv_stack1 s st} C {Q} \<Longrightarrow> \<Gamma> \<turnstile> {P ** inv_stack} C {Q}"
   apply (simp add: CSL_def inv_stack_def) by blast
 
-lemma p5_cond_aux : "\<sigma> \<Turnstile> (p4_post_noframe t s st \<and>\<^sub>S\<^sub>L \<langle>[t\<diamondop>NEXT]\<^sub>v >\<^sub>b [t\<diamondop>BASE]\<^sub>v\<rangle>\<^sub>S\<^sub>L) ** p4_frame st
+lemma p5_cond_aux : "\<sigma> \<Turnstile> (p4_post_noframe t s st \<and>\<^sub>S\<^sub>L \<langle>[NEXT]\<^sub>v >\<^sub>b [BASE]\<^sub>v\<rangle>\<^sub>S\<^sub>L) ** p4_frame st
                       \<Longrightarrow> p5_cond_if st"
   apply (simp add: p4_post_noframe_def p4_frame_def inv_stack_pt_def stack_pt_def p5_cond_if_def
   inv_stack_buf_waitq_def stack_buf_waitq_def)
   apply (case_tac "stack_wait st", case_tac "stack_tcbs st") apply linarith
    apply (simp add: is_waitq_def thread_sl_def) by linarith
 
-lemma p12_cond_aux : "\<sigma> \<Turnstile> ((p4_post_noframe t s st  ** p4_frame st) \<and>\<^sub>S\<^sub>L \<langle>\<not>\<^sub>b [t\<diamondop>NEXT]\<^sub>v >\<^sub>b [t\<diamondop>BASE]\<^sub>v\<rangle>\<^sub>S\<^sub>L) 
+lemma p12_cond_aux : "\<sigma> \<Turnstile> ((p4_post_noframe t s st  ** p4_frame st) \<and>\<^sub>S\<^sub>L \<langle>\<not>\<^sub>b [NEXT]\<^sub>v >\<^sub>b [BASE]\<^sub>v\<rangle>\<^sub>S\<^sub>L) 
                       ** P \<Longrightarrow> stack_base st = stack_next st"
   by (simp add: p4_post_noframe_def p4_frame_def inv_stack_pt_def stack_pt_def, clarsimp)
 
 lemma p12_cond_aux1 : "user_cmd C \<Longrightarrow> stack_base st = stack_next st \<longrightarrow> \<Gamma> \<turnstile> {((p4_post_noframe t s st  ** p4_frame st) 
-     \<and>\<^sub>S\<^sub>L \<langle>\<not>\<^sub>b [t\<diamondop>NEXT]\<^sub>v >\<^sub>b [t\<diamondop>BASE]\<^sub>v\<rangle>\<^sub>S\<^sub>L) ** P} C {Q} \<Longrightarrow> \<Gamma> \<turnstile> {((p4_post_noframe t s st  ** p4_frame st) 
-     \<and>\<^sub>S\<^sub>L \<langle>\<not>\<^sub>b [t\<diamondop>NEXT]\<^sub>v >\<^sub>b [t\<diamondop>BASE]\<^sub>v\<rangle>\<^sub>S\<^sub>L) ** P} C {Q}"
+     \<and>\<^sub>S\<^sub>L \<langle>\<not>\<^sub>b [NEXT]\<^sub>v >\<^sub>b [BASE]\<^sub>v\<rangle>\<^sub>S\<^sub>L) ** P} C {Q} \<Longrightarrow> \<Gamma> \<turnstile> {((p4_post_noframe t s st  ** p4_frame st) 
+     \<and>\<^sub>S\<^sub>L \<langle>\<not>\<^sub>b [NEXT]\<^sub>v >\<^sub>b [BASE]\<^sub>v\<rangle>\<^sub>S\<^sub>L) ** P} C {Q}"
   apply (case_tac "stack_base st = stack_next st", simp, simp)
   apply (simp only: CSL_def) using p12_cond_aux by blast
 
 lemma safe_p1819 : "t \<noteq> NULL \<Longrightarrow> fvAs \<Gamma> = {} \<Longrightarrow>
                     \<Gamma>(Cur := inv_cur, Readyq := inv_readyq, Stack := inv_stack) 
-                      \<turnstile> {(Aemp \<and>\<^sub>S\<^sub>L \<langle>[t\<diamondop>END]\<^sub>v =\<^sub>b [K_NO_WAIT]\<^sub>n\<rangle>\<^sub>S\<^sub>L) \<and>\<^sub>S\<^sub>L \<langle>\<not>\<^sub>b [t\<diamondop>RET]\<^sub>v =\<^sub>b [EAGAIN]\<^sub>n\<rangle>\<^sub>S\<^sub>L  } 
-                      (t \<^enum> t\<diamondop>DATA :=\<^sub>C \<lbrakk>[t]\<^sub>n\<Down>\<^sub>tdata\<rbrakk>);; 
-                      (t \<^enum> t\<diamondop>RET :=\<^sub>C [K_NO_WAIT]\<^sub>n) 
+                      \<turnstile> {(Aemp \<and>\<^sub>S\<^sub>L \<langle>[END]\<^sub>v =\<^sub>b [K_NO_WAIT]\<^sub>n\<rangle>\<^sub>S\<^sub>L) \<and>\<^sub>S\<^sub>L \<langle>\<not>\<^sub>b [RET]\<^sub>v =\<^sub>b [EAGAIN]\<^sub>n\<rangle>\<^sub>S\<^sub>L  } 
+                      (t \<^enum> DATA :=\<^sub>C \<lbrakk>[t]\<^sub>n\<Down>\<^sub>tdata\<rbrakk>);; 
+                      (t \<^enum> RET :=\<^sub>C [K_NO_WAIT]\<^sub>n) 
                          { Aemp }"
   apply (rule_tac Q = Aemp in rule_seq, rule rule_stm_stack, simp)
-  apply (simp add: disjoint_def Thread_Local_def)
-      apply ( simp add: Thread_Local_def, simp, simp add: Thread_Local_def, intro allI)
-  apply (rule_tac P = "inv_cur1 t ta" and Q = "inv_cur1 t ta \<and>\<^sub>S\<^sub>L \<langle>[t\<diamondop>DATA]\<^sub>v =\<^sub>b [thd_data ta]\<^sub>n\<rangle>\<^sub>S\<^sub>L"
+  apply (simp add: disjoint_def )
+      apply ( simp add: , simp, simp add: , intro allI)
+  apply (rule_tac P = "inv_cur1 t ta" and Q = "inv_cur1 t ta \<and>\<^sub>S\<^sub>L \<langle>[DATA]\<^sub>v =\<^sub>b [thd_data ta]\<^sub>n\<rangle>\<^sub>S\<^sub>L"
   in rule_conseq, simp add: inv_cur1_def is_cur_def)
      apply (rule_tac Pa = "([A_Cur]\<^sub>v \<longmapsto> [t]\<^sub>n \<and>\<^sub>S\<^sub>L inv_is_running ta) ** thread_node t ta" and Qa = "
-      ([A_Cur]\<^sub>v \<longmapsto> [t]\<^sub>n  \<and>\<^sub>S\<^sub>L inv_is_running ta) ** (thread_node t ta \<and>\<^sub>S\<^sub>L \<langle>[t\<diamondop>DATA]\<^sub>v =\<^sub>b [thd_data ta]\<^sub>n\<rangle>\<^sub>S\<^sub>L)" 
+      ([A_Cur]\<^sub>v \<longmapsto> [t]\<^sub>n  \<and>\<^sub>S\<^sub>L inv_is_running ta) ** (thread_node t ta \<and>\<^sub>S\<^sub>L \<langle>[DATA]\<^sub>v =\<^sub>b [thd_data ta]\<^sub>n\<rangle>\<^sub>S\<^sub>L)" 
        in safe_assn_equiv)
        apply (simp add: inv_is_running_def assn_equiv_def) apply auto[1]
       apply (simp add: inv_is_running_def assn_equiv_def) apply auto[1]
      apply (rule rule_frame1, rule thread_node_read_data, simp add: fvA_Gamma2)
-      apply (simp add: fvA_inv_cur fvA_inv_readyq fvA_inv_stack Thread_Local_def, simp)
-     apply (simp add: inv_is_running_def disjoint_def Thread_Local_def)
+      apply (simp add: fvA_inv_cur fvA_inv_readyq fvA_inv_stack , simp)
+     apply (simp add: inv_is_running_def disjoint_def )
       apply (simp add: implies_def) apply (rule_tac Q = "inv_cur1 t ta" in implies_trans)
     apply (simp add: implies_def)
   apply (rule_tac Q = "inv_cur" in implies_trans, simp add: inv_cur_implies2)
    apply (simp add: implies_def, simp add: implies_def)
   apply (rule rule_stm_stack', simp_all)
-    apply (simp add: disjoint_def Thread_Local_def)
-   apply (rule_tac P = Aemp and Q = "Aemp \<and>\<^sub>S\<^sub>L \<langle>[t\<diamondop>RET]\<^sub>v =\<^sub>b [0]\<^sub>n\<rangle>\<^sub>S\<^sub>L" in rule_conseq)
+    apply (simp add: disjoint_def )
+   apply (rule_tac P = Aemp and Q = "Aemp \<and>\<^sub>S\<^sub>L \<langle>[RET]\<^sub>v =\<^sub>b [0]\<^sub>n\<rangle>\<^sub>S\<^sub>L" in rule_conseq)
      apply (rule rule_assign_num1, simp add: fvA_Gamma2 fvA_inv_stack fvA_inv_cur fvA_inv_readyq)
-     apply (simp add: Thread_Local_def, simp add: implies_def, simp add: implies_def)
-  by (simp add: Thread_Local_def)
+     apply (simp add: implies_def, simp add: implies_def)
+  done
   
 lemma safe_pop : "fvAs \<Gamma> = {} \<Longrightarrow> 
                    \<Gamma>(Cur := inv_cur, Readyq := inv_readyq, Stack := inv_stack) \<turnstile>
                     {Aemp \<and>\<^sub>S\<^sub>L \<langle>[t \<noteq> NULL]\<^sub>b\<rangle>\<^sub>S\<^sub>L} stack_pop t timeout { Aemp}"
-  apply (simp add: stack_pop_def) apply (case_tac t, simp add: CSL_def stm_def)
+  apply (simp only: stack_pop_def)
+  apply (rule rule_Clocals)
+  apply (case_tac t, simp add: CSL_def stm_def)
   apply (rule_tac Q = Aemp in rule_seq)
    apply (rule_tac Q = "p1_post t" in rule_seq, simp add: p1_post_def)
-    apply (rule rule_stm_stack', simp, simp add: disjoint_def Thread_Local_def, simp, simp, simp)
-    apply (rule_tac Pa = " Aemp" and Qa = "Aemp \<and>\<^sub>S\<^sub>L \<langle>[t\<diamondop>END]\<^sub>v =\<^sub>b [0]\<^sub>n\<rangle>\<^sub>S\<^sub>L"
+    apply (rule rule_stm_stack', simp, simp add: disjoint_def , simp, simp, simp)
+    apply (rule_tac Pa = " Aemp" and Qa = "Aemp \<and>\<^sub>S\<^sub>L \<langle>[END]\<^sub>v =\<^sub>b [0]\<^sub>n\<rangle>\<^sub>S\<^sub>L"
     in safe_assn_equiv, simp add: assn_equiv_def, simp add: assn_equiv_def) apply auto[1]
-     apply (simp, rule rule_assign_num1, simp add: fvA_Gamma2 fvA_inv_cur fvA_inv_stack fvA_inv_readyq)
-  apply (simp add: Thread_Local_def, simp add: Thread_Local_def)
+     apply (rule rule_assign_num1, simp add: fvA_Gamma2 fvA_inv_cur fvA_inv_stack fvA_inv_readyq)
+  apply (simp , simp)
    apply (rule rule_with_true, simp, rule rule_inv_stack, intro allI)
    apply (rule_tac Q = "p1_post t ** (p4_post_noframe t s st ** p4_frame st)" in rule_seq, simp add: safe_p24)
-   apply (rule rule_if, rule_tac P = "(p4_post_noframe t s st \<and>\<^sub>S\<^sub>L \<langle>[t\<diamondop>NEXT]\<^sub>v >\<^sub>b [t\<diamondop>BASE]\<^sub>v\<rangle>\<^sub>S\<^sub>L) 
+   apply (rule rule_if, rule_tac P = "(p4_post_noframe t s st \<and>\<^sub>S\<^sub>L \<langle>[NEXT]\<^sub>v >\<^sub>b [BASE]\<^sub>v\<rangle>\<^sub>S\<^sub>L) 
     ** p4_frame st" and Q = "inv_stack" in rule_conseq)
   apply (case_tac "\<not> p5_cond_if st", simp only: CSL_def) 
   using p5_cond_aux stm_def user_cmd.simps(15) apply fastforce
@@ -540,12 +535,12 @@ lemma safe_pop : "fvAs \<Gamma> = {} \<Longrightarrow>
       apply (simp add: implies_def p1_post_def) apply auto[1]
   apply (simp add: p10_pre_implies) 
   using Aemp_equiv assn_equiv_symmetry equiv_implies implies_trans inv_stack_implies apply blast
-   apply (rule rule_stm_stack, simp, simp add: disjoint_def Thread_Local_def)
+   apply (rule rule_stm_stack, simp, simp add: disjoint_def )
       apply (simp add: p4_frame_def fvA_buf fvA_is_waitq inv_stack_buf_waitq_def inv_stack_pt_def)
-      apply (simp add: p1_post_def p4_post_noframe_def stack_node_def Thread_Local_def, simp)
+      apply (simp add: p1_post_def p4_post_noframe_def stack_node_def , simp)
     apply (simp add: p4_frame_def fvA_buf fvA_is_waitq inv_stack_buf_waitq_def inv_stack_pt_def)
-    apply (simp add: p1_post_def p4_post_noframe_def stack_node_def Thread_Local_def, intro allI)
-   apply (rule_tac P = "((p4_post_noframe t s st ** p4_frame st) \<and>\<^sub>S\<^sub>L \<langle>\<not>\<^sub>b [t\<diamondop>NEXT]\<^sub>v >\<^sub>b [t\<diamondop>BASE]\<^sub>v\<rangle>\<^sub>S\<^sub>L) 
+    apply (simp add: p1_post_def p4_post_noframe_def stack_node_def , intro allI)
+   apply (rule_tac P = "((p4_post_noframe t s st ** p4_frame st) \<and>\<^sub>S\<^sub>L \<langle>\<not>\<^sub>b [NEXT]\<^sub>v >\<^sub>b [BASE]\<^sub>v\<rangle>\<^sub>S\<^sub>L) 
    ** inv_cur1 t ta" and Q = "inv_cur ** inv_stack" in rule_conseq)
      apply (rule p12_cond_aux1, simp add: stm_def, rule impI)
   apply (rule_tac P = "p12_pre_noframe t ta s st ** p12_frame s st" and Q = "[A_Cur]\<^sub>v \<longmapsto> [NULL]\<^sub>n ** 
@@ -563,6 +558,7 @@ apply (rule rule_if, rule rule_if)
     apply (simp add: safe_p1819, simp_all)
    apply (rule_tac P = Aemp and Q = Aemp in rule_conseq, simp add: rule_skip)
     apply (simp add: implies_def, simp add: implies_def)
+  apply (simp add: fvA_Gamma2 fvA_inv_stack fvA_inv_cur fvA_inv_readyq) 
   done
 
 end
