func_cor_push.thy
@@ -3,47 +3,45 @@ theory func_cor_push
 begin
 
 definition p1_post :: "nat \<Rightarrow> assn"
-  where "p1_post t = (\<langle>[t\<diamondop>END]\<^sub>v =\<^sub>b [K_NO_WAIT]\<^sub>n\<rangle>\<^sub>S\<^sub>L \<and>\<^sub>S\<^sub>L Aemp)"
+  where "p1_post t = (\<langle>[END]\<^sub>v =\<^sub>b [K_NO_WAIT]\<^sub>n\<rangle>\<^sub>S\<^sub>L \<and>\<^sub>S\<^sub>L Aemp)"
 
 
 definition p4_post_noframe :: "nat \<Rightarrow> nat \<Rightarrow> stack_mem \<Rightarrow> assn"
-  where "p4_post_noframe t s st = ([A_Stack]\<^sub>v \<longmapsto> [s]\<^sub>n) ** (stack_node s st \<and>\<^sub>S\<^sub>L \<langle>[t \<diamondop> ADDR]\<^sub>v =\<^sub>b [s]\<^sub>n\<rangle>\<^sub>S\<^sub>L
-      \<and>\<^sub>S\<^sub>L \<langle>[t \<diamondop> NEXT]\<^sub>v =\<^sub>b [stack_next st]\<^sub>n\<rangle>\<^sub>S\<^sub>L \<and>\<^sub>S\<^sub>L \<langle>[t \<diamondop> TOP]\<^sub>v =\<^sub>b [stack_top st]\<^sub>n\<rangle>\<^sub>S\<^sub>L)"
+  where "p4_post_noframe t s st = ([A_Stack]\<^sub>v \<longmapsto> [s]\<^sub>n) ** (stack_node s st \<and>\<^sub>S\<^sub>L \<langle>[ ADDR]\<^sub>v =\<^sub>b [s]\<^sub>n\<rangle>\<^sub>S\<^sub>L
+      \<and>\<^sub>S\<^sub>L \<langle>[ NEXT]\<^sub>v =\<^sub>b [stack_next st]\<^sub>n\<rangle>\<^sub>S\<^sub>L \<and>\<^sub>S\<^sub>L \<langle>[ TOP]\<^sub>v =\<^sub>b [stack_top st]\<^sub>n\<rangle>\<^sub>S\<^sub>L)"
 
 lemma safe_p24_noframe : "fvAs \<Gamma> = {} \<Longrightarrow> t \<noteq> NULL \<Longrightarrow>
                           \<Gamma>(Cur := inv_cur, Readyq := inv_readyq, Stack := inv_stack) \<turnstile>
                           {([A_Stack]\<^sub>v \<longmapsto> [s]\<^sub>n) ** stack_node s st}
-                            (t \<^enum> (t \<diamondop> ADDR) :=\<^sub>C \<lbrakk>[A_Stack]\<^sub>v\<rbrakk>) ;;
-                            (t \<^enum> (t \<diamondop> NEXT) :=\<^sub>C \<lbrakk>[t \<diamondop> ADDR]\<^sub>v\<Down>\<^sub>snext\<rbrakk>) ;;
-                            (t \<^enum> (t \<diamondop> TOP) :=\<^sub>C \<lbrakk>[t \<diamondop> ADDR]\<^sub>v\<Down>\<^sub>stop\<rbrakk>) 
+                            (t \<^enum> ( ADDR) :=\<^sub>C \<lbrakk>[A_Stack]\<^sub>v\<rbrakk>) ;;
+                            (t \<^enum> ( NEXT) :=\<^sub>C \<lbrakk>[ ADDR]\<^sub>v\<Down>\<^sub>snext\<rbrakk>) ;;
+                            (t \<^enum> ( TOP) :=\<^sub>C \<lbrakk>[ ADDR]\<^sub>v\<Down>\<^sub>stop\<rbrakk>) 
                           {p4_post_noframe t s st}"
-  apply (rule_tac Q = "([A_Stack]\<^sub>v \<longmapsto> [s]\<^sub>n) ** (stack_node s st \<and>\<^sub>S\<^sub>L \<langle>[t \<diamondop> ADDR]\<^sub>v =\<^sub>b [s]\<^sub>n\<rangle>\<^sub>S\<^sub>L
-      \<and>\<^sub>S\<^sub>L \<langle>[t \<diamondop> NEXT]\<^sub>v =\<^sub>b [stack_next st]\<^sub>n\<rangle>\<^sub>S\<^sub>L)" in rule_seq)
-   apply (rule_tac Q = "([A_Stack]\<^sub>v \<longmapsto> [s]\<^sub>n) ** (stack_node s st \<and>\<^sub>S\<^sub>L \<langle>[t \<diamondop> ADDR]\<^sub>v =\<^sub>b [s]\<^sub>n\<rangle>\<^sub>S\<^sub>L)" in rule_seq)
+  apply (rule_tac Q = "([A_Stack]\<^sub>v \<longmapsto> [s]\<^sub>n) ** (stack_node s st \<and>\<^sub>S\<^sub>L \<langle>[ ADDR]\<^sub>v =\<^sub>b [s]\<^sub>n\<rangle>\<^sub>S\<^sub>L
+      \<and>\<^sub>S\<^sub>L \<langle>[ NEXT]\<^sub>v =\<^sub>b [stack_next st]\<^sub>n\<rangle>\<^sub>S\<^sub>L)" in rule_seq)
+   apply (rule_tac Q = "([A_Stack]\<^sub>v \<longmapsto> [s]\<^sub>n) ** (stack_node s st \<and>\<^sub>S\<^sub>L \<langle>[ ADDR]\<^sub>v =\<^sub>b [s]\<^sub>n\<rangle>\<^sub>S\<^sub>L)" in rule_seq)
   apply (rule_tac Pa = "[A_Stack]\<^sub>v \<longmapsto> [s]\<^sub>n ** stack_node s st" and Qa = "([A_Stack]\<^sub>v \<longmapsto> [s]\<^sub>n \<and>\<^sub>S\<^sub>L 
-  \<langle>[t \<diamondop> ADDR]\<^sub>v =\<^sub>b [s]\<^sub>n\<rangle>\<^sub>S\<^sub>L) ** stack_node s st" in safe_assn_equiv, simp add: assn_equiv_reflex)
+  \<langle>[ ADDR]\<^sub>v =\<^sub>b [s]\<^sub>n\<rangle>\<^sub>S\<^sub>L) ** stack_node s st" in safe_assn_equiv, simp add: assn_equiv_reflex)
      apply (simp add: assn_equiv_def) apply auto[1]
     apply (rule rule_frame, rule rule_stm_stack', simp_all)
-         apply (simp add: disjoint_def Thread_Local_def, simp add: Thread_Local_def, simp add: Thread_Local_def)
+         apply (simp add: disjoint_def)
       apply (rule rule_read, simp add: fvA_Gamma2 fvA_inv_cur fvA_inv_readyq fvA_inv_stack)
-  apply (simp add: Thread_Local_def, simp add: Thread_Local_def)
     apply (simp add: stack_node_def) apply (rule rule_frame1)
-    apply (rule rule_stm_stack' , simp_all, simp add: disjoint_def Thread_Local_def)
-       apply (simp add: stack_node_def Thread_Local_def)
-      apply (simp add: stack_node_def Thread_Local_def)
-    apply (rule stack_node_read_next, simp add: Thread_Local_def)
-     apply (simp_all add: fvA_Gamma2 fvA_inv_cur fvA_inv_readyq fvA_inv_stack)
-     apply (simp add: Thread_Local_def, simp add: Thread_Local_def)
-    apply (simp add: Thread_Local_def, simp add: disjoint_def stm_def Thread_Local_def)
+    apply (rule rule_stm_stack' , simp_all, simp add: disjoint_def)
+       apply (simp add: stack_node_def)
+      apply (simp add: stack_node_def)
+    apply (rule stack_node_read_next)
+      apply (simp_all add: fvA_Gamma2 fvA_inv_cur fvA_inv_readyq fvA_inv_stack)
+    apply (simp add: disjoint_def stm_def)
   apply (simp add: p4_post_noframe_def, rule rule_frame1, rule rule_stm_stack', simp_all)
-       apply (simp add: disjoint_def Thread_Local_def)
-      apply (simp add: stack_node_def Thread_Local_def)
-     apply (simp add: stack_node_def Thread_Local_def)
+       apply (simp add: disjoint_def)
+      apply (simp add: stack_node_def)
+     apply (simp add: stack_node_def)
     apply (rule stack_node_read_top1)
-      apply (simp add: Thread_Local_def, simp add: Thread_Local_def)
-     apply (simp add: fvA_Gamma2 fvA_inv_stack fvA_inv_readyq fvA_inv_cur Thread_Local_def)
-  apply (simp add: fvA_Gamma2 fvA_inv_stack fvA_inv_readyq fvA_inv_cur Thread_Local_def)
-   apply (simp add: Thread_Local_def, simp add: disjoint_def stm_def Thread_Local_def)
+      apply (simp_all)
+     apply (simp add: fvA_Gamma2 fvA_inv_stack fvA_inv_readyq fvA_inv_cur )
+  apply (simp add: fvA_Gamma2 fvA_inv_stack fvA_inv_readyq fvA_inv_cur )
+   apply (simp add: disjoint_def stm_def)
   done
 
 definition p4_frame :: " stack_mem \<Rightarrow> assn"
@@ -68,19 +66,19 @@ lemma safe_p24_pre_equiv : "inv_stack1 s st \<equiv>\<^sub>S\<^sub>L  (([A_Stack
 lemma safe_p24 : "fvAs \<Gamma> = {} \<Longrightarrow> t \<noteq> NULL \<Longrightarrow>
                           \<Gamma>(Cur := inv_cur, Readyq := inv_readyq, Stack := inv_stack) \<turnstile>
                           {p1_post t ** inv_stack1 s st}
-                            (t \<^enum> (t \<diamondop> ADDR) :=\<^sub>C \<lbrakk>[A_Stack]\<^sub>v\<rbrakk>) ;;
-                            (t \<^enum> (t \<diamondop> NEXT) :=\<^sub>C \<lbrakk>[t \<diamondop> ADDR]\<^sub>v\<Down>\<^sub>snext\<rbrakk>) ;;
-                            (t \<^enum> (t \<diamondop> TOP) :=\<^sub>C \<lbrakk>[t \<diamondop> ADDR]\<^sub>v\<Down>\<^sub>stop\<rbrakk>) 
+                            (t \<^enum> ( ADDR) :=\<^sub>C \<lbrakk>[A_Stack]\<^sub>v\<rbrakk>) ;;
+                            (t \<^enum> ( NEXT) :=\<^sub>C \<lbrakk>[ ADDR]\<^sub>v\<Down>\<^sub>snext\<rbrakk>) ;;
+                            (t \<^enum> ( TOP) :=\<^sub>C \<lbrakk>[ ADDR]\<^sub>v\<Down>\<^sub>stop\<rbrakk>) 
                           {p1_post t ** (p4_post_noframe t s st ** p4_frame st)}"
   apply (rule rule_frame1, rule_tac Pa = "([A_Stack]\<^sub>v \<longmapsto> [s]\<^sub>n) ** stack_node s st ** p4_frame st"
   and Qa = "p4_post_noframe t s st ** p4_frame st" in safe_assn_equiv)
      apply (simp add: assn_equiv_symmetry safe_p24_pre_equiv, simp add: assn_equiv_reflex)
    apply (rule rule_frame, simp add: safe_p24_noframe)
    apply (simp add: p4_frame_def fvA_is_waitq fvA_buf inv_stack_pt_def inv_stack_buf_waitq_def)
-  apply (simp add: p1_post_def stm_def disjoint_def Thread_Local_def)
+  apply (simp add: p1_post_def stm_def disjoint_def )
   done
 
-lemma p5_pre_implies : "(p1_post t ** (p4_post_noframe t s st ** p4_frame st) \<and>\<^sub>S\<^sub>L \<langle>[t\<diamondop>NEXT]\<^sub>v =\<^sub>b [t\<diamondop>TOP]\<^sub>v\<rangle>\<^sub>S\<^sub>L)
+lemma p5_pre_implies : "(p1_post t ** (p4_post_noframe t s st ** p4_frame st) \<and>\<^sub>S\<^sub>L \<langle>[NEXT]\<^sub>v =\<^sub>b [TOP]\<^sub>v\<rangle>\<^sub>S\<^sub>L)
                          \<sqsubseteq> inv_stack1 s st"
   apply (rule_tac Q = "(([A_Stack]\<^sub>v \<longmapsto> [s]\<^sub>n) ** stack_node s st) **  p4_frame st" in implies_trans)
    apply (simp add: p1_post_def p4_post_noframe_def implies_def) apply blast
@@ -89,53 +87,53 @@ lemma p5_pre_implies : "(p1_post t ** (p4_post_noframe t s st ** p4_frame st) \<
 lemma safe_p56 : "fvAs \<Gamma> = {} \<Longrightarrow> t \<noteq> NULL \<Longrightarrow>
                  \<Gamma>(Cur := inv_cur, Readyq := inv_readyq, Stack := inv_stack) \<turnstile>
                           { inv_stack1 s st}
-                          (t \<^enum> (t \<diamondop> RET) :=\<^sub>C [ENOMEM]\<^sub>n) ;;
-                          (t \<^enum> (t \<diamondop> END) :=\<^sub>C [1]\<^sub>n)
+                          (t \<^enum> ( RET) :=\<^sub>C [ENOMEM]\<^sub>n) ;;
+                          (t \<^enum> ( END) :=\<^sub>C [1]\<^sub>n)
                           { inv_stack1 s st}"
-  apply (rule_tac Q = "inv_stack1 s st \<and>\<^sub>S\<^sub>L \<langle>[t \<diamondop> RET]\<^sub>v =\<^sub>b [ENOMEM]\<^sub>n\<rangle>\<^sub>S\<^sub>L" in rule_seq)
+  apply (rule_tac Q = "inv_stack1 s st \<and>\<^sub>S\<^sub>L \<langle>[ RET]\<^sub>v =\<^sub>b [ENOMEM]\<^sub>n\<rangle>\<^sub>S\<^sub>L" in rule_seq)
    apply (rule rule_stm_stack', simp_all)
-        apply (simp add: disjoint_def Thread_Local_def)
-      apply (simp add: inv_stack1_def fvA_is_stack Thread_Local_def)
-     apply (simp add: inv_stack1_def fvA_is_stack Thread_Local_def)
+        apply (simp add: disjoint_def )
+      apply (simp add: inv_stack1_def fvA_is_stack )
+     apply (simp add: inv_stack1_def fvA_is_stack )
     apply (rule rule_assign_num1, simp add: fvA_Gamma2 fvA_inv_stack fvA_inv_cur fvA_inv_readyq)
-    apply (simp add: inv_stack1_def fvA_is_stack Thread_Local_def, simp add: Thread_Local_def)
-  apply (rule_tac P = "inv_stack1 s st" and Q = "inv_stack1 s st \<and>\<^sub>S\<^sub>L \<langle>[t \<diamondop> END]\<^sub>v =\<^sub>b [1]\<^sub>n\<rangle>\<^sub>S\<^sub>L" in rule_conseq)
+    apply (simp add: inv_stack1_def fvA_is_stack)
+  apply (rule_tac P = "inv_stack1 s st" and Q = "inv_stack1 s st \<and>\<^sub>S\<^sub>L \<langle>[ END]\<^sub>v =\<^sub>b [1]\<^sub>n\<rangle>\<^sub>S\<^sub>L" in rule_conseq)
     apply (rule rule_stm_stack', simp_all)
-        apply (simp add: disjoint_def Thread_Local_def)
-       apply (simp add: inv_stack1_def fvA_is_stack Thread_Local_def)
-      apply (simp add: inv_stack1_def fvA_is_stack Thread_Local_def)
+        apply (simp add: disjoint_def )
+       apply (simp add: inv_stack1_def fvA_is_stack)
+      apply (simp add: inv_stack1_def fvA_is_stack)
      apply (rule rule_assign_num1, simp add: fvA_Gamma2 fvA_inv_stack fvA_inv_cur fvA_inv_readyq)
-  apply (simp add: inv_stack1_def fvA_is_stack Thread_Local_def, simp add: Thread_Local_def)
+  apply (simp add: inv_stack1_def fvA_is_stack)
   by (simp_all add: implies_def)
 
 definition p7_pre_noframe :: "nat \<Rightarrow> nat \<Rightarrow> stack_mem \<Rightarrow> assn"
-  where "p7_pre_noframe t s st = ([A_Stack]\<^sub>v \<longmapsto> [s]\<^sub>n) ** (stack_node s st \<and>\<^sub>S\<^sub>L \<langle>[t \<diamondop> ADDR]\<^sub>v =\<^sub>b [s]\<^sub>n\<rangle>\<^sub>S\<^sub>L
-          \<and>\<^sub>S\<^sub>L \<langle>[t \<diamondop> NEXT]\<^sub>v =\<^sub>b [stack_next st]\<^sub>n\<rangle>\<^sub>S\<^sub>L)"
+  where "p7_pre_noframe t s st = ([A_Stack]\<^sub>v \<longmapsto> [s]\<^sub>n) ** (stack_node s st \<and>\<^sub>S\<^sub>L \<langle>[ ADDR]\<^sub>v =\<^sub>b [s]\<^sub>n\<rangle>\<^sub>S\<^sub>L
+          \<and>\<^sub>S\<^sub>L \<langle>[ NEXT]\<^sub>v =\<^sub>b [stack_next st]\<^sub>n\<rangle>\<^sub>S\<^sub>L)"
 
 definition p7_post_noframe :: "nat \<Rightarrow> nat \<Rightarrow> stack_mem \<Rightarrow> assn"
-  where "p7_post_noframe t s st = ([A_Stack]\<^sub>v \<longmapsto> [s]\<^sub>n) ** (stack_node s st \<and>\<^sub>S\<^sub>L \<langle>[t \<diamondop> ADDR]\<^sub>v =\<^sub>b [s]\<^sub>n\<rangle>\<^sub>S\<^sub>L
-  \<and>\<^sub>S\<^sub>L \<langle>[t \<diamondop> NEXT]\<^sub>v =\<^sub>b [stack_next st]\<^sub>n\<rangle>\<^sub>S\<^sub>L \<and>\<^sub>S\<^sub>L \<langle>[t\<diamondop>FIRST_PENDING_THREAD]\<^sub>v =\<^sub>b [stack_wait st]\<^sub>n\<rangle>\<^sub>S\<^sub>L)"
+  where "p7_post_noframe t s st = ([A_Stack]\<^sub>v \<longmapsto> [s]\<^sub>n) ** (stack_node s st \<and>\<^sub>S\<^sub>L \<langle>[ ADDR]\<^sub>v =\<^sub>b [s]\<^sub>n\<rangle>\<^sub>S\<^sub>L
+  \<and>\<^sub>S\<^sub>L \<langle>[ NEXT]\<^sub>v =\<^sub>b [stack_next st]\<^sub>n\<rangle>\<^sub>S\<^sub>L \<and>\<^sub>S\<^sub>L \<langle>[FIRST_PENDING_THREAD]\<^sub>v =\<^sub>b [stack_wait st]\<^sub>n\<rangle>\<^sub>S\<^sub>L)"
 
 lemma safe_p7_noframe : "fvAs \<Gamma> = {} \<Longrightarrow> 
                  \<Gamma>(Cur := inv_cur, Readyq := inv_readyq, Stack := inv_stack) \<turnstile>
                           { p7_pre_noframe t s st}
-                     t\<diamondop>FIRST_PENDING_THREAD :=\<^sub>C \<lbrakk>[t\<diamondop>ADDR]\<^sub>v\<Down>\<^sub>swait\<rbrakk>
+                     FIRST_PENDING_THREAD :=\<^sub>C \<lbrakk>[ADDR]\<^sub>v\<Down>\<^sub>swait\<rbrakk>
                           { p7_post_noframe t s st}"
   apply (simp add: p7_pre_noframe_def p7_post_noframe_def, rule rule_frame1)
-  apply (rule_tac Pa = "(stack_node s st \<and>\<^sub>S\<^sub>L \<langle>[t \<diamondop> ADDR]\<^sub>v =\<^sub>b [s]\<^sub>n\<rangle>\<^sub>S\<^sub>L) ** (\<langle>[t \<diamondop> NEXT]\<^sub>v =\<^sub>b 
-  [stack_next st]\<^sub>n\<rangle>\<^sub>S\<^sub>L \<and>\<^sub>S\<^sub>L Aemp)" and Qa = "(stack_node s st \<and>\<^sub>S\<^sub>L \<langle>[t \<diamondop> ADDR]\<^sub>v =\<^sub>b [s]\<^sub>n\<rangle>\<^sub>S\<^sub>L  \<and>\<^sub>S\<^sub>L 
-  \<langle>[t\<diamondop>FIRST_PENDING_THREAD]\<^sub>v =\<^sub>b [stack_wait st]\<^sub>n\<rangle>\<^sub>S\<^sub>L) ** (\<langle>[t \<diamondop> NEXT]\<^sub>v =\<^sub>b [stack_next st]\<^sub>n\<rangle>\<^sub>S\<^sub>L \<and>\<^sub>S\<^sub>L Aemp)"
+  apply (rule_tac Pa = "(stack_node s st \<and>\<^sub>S\<^sub>L \<langle>[ ADDR]\<^sub>v =\<^sub>b [s]\<^sub>n\<rangle>\<^sub>S\<^sub>L) ** (\<langle>[ NEXT]\<^sub>v =\<^sub>b 
+  [stack_next st]\<^sub>n\<rangle>\<^sub>S\<^sub>L \<and>\<^sub>S\<^sub>L Aemp)" and Qa = "(stack_node s st \<and>\<^sub>S\<^sub>L \<langle>[ ADDR]\<^sub>v =\<^sub>b [s]\<^sub>n\<rangle>\<^sub>S\<^sub>L  \<and>\<^sub>S\<^sub>L 
+  \<langle>[FIRST_PENDING_THREAD]\<^sub>v =\<^sub>b [stack_wait st]\<^sub>n\<rangle>\<^sub>S\<^sub>L) ** (\<langle>[ NEXT]\<^sub>v =\<^sub>b [stack_next st]\<^sub>n\<rangle>\<^sub>S\<^sub>L \<and>\<^sub>S\<^sub>L Aemp)"
   in safe_assn_equiv, simp_all add: assn_equiv_def) apply auto[1]
-   apply (rule rule_frame, rule stack_node_read_wait, simp add: Thread_Local_def)
-  by (simp_all add: fvA_Gamma2 fvA_inv_cur fvA_inv_stack fvA_inv_readyq disjoint_def Thread_Local_def)
+   apply (rule rule_frame, rule stack_node_read_wait, simp add: )
+  by (simp_all add: fvA_Gamma2 fvA_inv_cur fvA_inv_stack fvA_inv_readyq disjoint_def )
 
 definition p9_pre_noframe :: "nat \<Rightarrow> nat \<Rightarrow> tcb \<Rightarrow> tcbs \<Rightarrow> stack_mem \<Rightarrow> assn"
-  where "p9_pre_noframe t s a list st = (stack_node s st \<and>\<^sub>S\<^sub>L \<langle>[t \<diamondop> ADDR]\<^sub>v =\<^sub>b [s]\<^sub>n\<rangle>\<^sub>S\<^sub>L \<and>\<^sub>S\<^sub>L 
-  \<langle>[t\<diamondop>FIRST_PENDING_THREAD]\<^sub>v =\<^sub>b [stack_wait st]\<^sub>n\<rangle>\<^sub>S\<^sub>L) ** is_waitq (stack_wait st) (a # list)"
+  where "p9_pre_noframe t s a list st = (stack_node s st \<and>\<^sub>S\<^sub>L \<langle>[ ADDR]\<^sub>v =\<^sub>b [s]\<^sub>n\<rangle>\<^sub>S\<^sub>L \<and>\<^sub>S\<^sub>L 
+  \<langle>[FIRST_PENDING_THREAD]\<^sub>v =\<^sub>b [stack_wait st]\<^sub>n\<rangle>\<^sub>S\<^sub>L) ** is_waitq (stack_wait st) (a # list)"
 
 definition p9_pre :: "nat \<Rightarrow> nat \<Rightarrow> tcb \<Rightarrow> tcbs \<Rightarrow> stack_mem \<Rightarrow> assn"
-  where "p9_pre t s a list st = (stack_node s st \<and>\<^sub>S\<^sub>L \<langle>[t \<diamondop> ADDR]\<^sub>v =\<^sub>b [s]\<^sub>n\<rangle>\<^sub>S\<^sub>L) ** (thread_node 
-  (stack_wait st) a \<and>\<^sub>S\<^sub>L \<langle>[t\<diamondop>FIRST_PENDING_THREAD]\<^sub>v =\<^sub>b [stack_wait st]\<^sub>n\<rangle>\<^sub>S\<^sub>L) ** (thread_wait_sl (thd_next a)
+  where "p9_pre t s a list st = (stack_node s st \<and>\<^sub>S\<^sub>L \<langle>[ ADDR]\<^sub>v =\<^sub>b [s]\<^sub>n\<rangle>\<^sub>S\<^sub>L) ** (thread_node 
+  (stack_wait st) a \<and>\<^sub>S\<^sub>L \<langle>[FIRST_PENDING_THREAD]\<^sub>v =\<^sub>b [stack_wait st]\<^sub>n\<rangle>\<^sub>S\<^sub>L) ** (thread_wait_sl (thd_next a)
   list )"
 
 lemma p9_pre_implies_aux : "(P1 \<and>\<^sub>S\<^sub>L \<langle>P2\<rangle>\<^sub>S\<^sub>L \<and>\<^sub>S\<^sub>L \<langle>P3\<rangle>\<^sub>S\<^sub>L) ** (P4 ** P5) \<equiv>\<^sub>S\<^sub>L 
@@ -147,11 +145,11 @@ lemma p9_pre_implies_aux : "(P1 \<and>\<^sub>S\<^sub>L \<langle>P2\<rangle>\<^su
   apply (simp add: assn_equiv_reflex, simp add: assn_equiv_def) by auto
 
 lemma p9_pre_implies : "p9_pre_noframe t s a list st \<sqsubseteq> p9_pre t s a list st"
-  apply (rule_tac Q = "(stack_node s st \<and>\<^sub>S\<^sub>L \<langle>[t \<diamondop> ADDR]\<^sub>v =\<^sub>b [s]\<^sub>n\<rangle>\<^sub>S\<^sub>L \<and>\<^sub>S\<^sub>L \<langle>[t\<diamondop>FIRST_PENDING_THREAD]\<^sub>v =\<^sub>b 
+  apply (rule_tac Q = "(stack_node s st \<and>\<^sub>S\<^sub>L \<langle>[ ADDR]\<^sub>v =\<^sub>b [s]\<^sub>n\<rangle>\<^sub>S\<^sub>L \<and>\<^sub>S\<^sub>L \<langle>[FIRST_PENDING_THREAD]\<^sub>v =\<^sub>b 
   [stack_wait st]\<^sub>n\<rangle>\<^sub>S\<^sub>L) ** thread_wait_sl (stack_wait st) (a # list)" in implies_trans)
   apply (rule equiv_implies, simp add: p9_pre_noframe_def)
   using assn_equiv_cong_star assn_equiv_reflex waitq_equiv apply auto[1]
-  apply (rule_tac Q = "(stack_node s st \<and>\<^sub>S\<^sub>L \<langle>[t \<diamondop> ADDR]\<^sub>v =\<^sub>b [s]\<^sub>n\<rangle>\<^sub>S\<^sub>L \<and>\<^sub>S\<^sub>L \<langle>[t\<diamondop>FIRST_PENDING_THREAD]\<^sub>v =\<^sub>b 
+  apply (rule_tac Q = "(stack_node s st \<and>\<^sub>S\<^sub>L \<langle>[ ADDR]\<^sub>v =\<^sub>b [s]\<^sub>n\<rangle>\<^sub>S\<^sub>L \<and>\<^sub>S\<^sub>L \<langle>[FIRST_PENDING_THREAD]\<^sub>v =\<^sub>b 
   [stack_wait st]\<^sub>n\<rangle>\<^sub>S\<^sub>L) ** (thread_node (stack_wait st) a ** thread_wait_sl (thd_next a) list)" in implies_trans)
    apply (rule implies_star, simp add: implies_def)
    apply (case_tac "stack_wait st", simp add: thread_wait_sl_def, simp add: implies_def)
@@ -159,13 +157,13 @@ lemma p9_pre_implies : "p9_pre_noframe t s a list st \<sqsubseteq> p9_pre t s a 
   by (rule equiv_implies, simp add: p9_pre_def p9_pre_implies_aux)
   
 definition p9_post :: "nat \<Rightarrow> nat \<Rightarrow> tcb \<Rightarrow> tcbs \<Rightarrow> stack_mem \<Rightarrow> assn"
-  where "p9_post t s a list st = (stack_node s st \<and>\<^sub>S\<^sub>L \<langle>[t \<diamondop> ADDR]\<^sub>v =\<^sub>b [s]\<^sub>n\<rangle>\<^sub>S\<^sub>L) ** (thread_node 
-  (stack_wait st) a \<and>\<^sub>S\<^sub>L \<langle>[t\<diamondop>FIRST_PENDING_THREAD]\<^sub>v =\<^sub>b [stack_wait st]\<^sub>n\<rangle>\<^sub>S\<^sub>L \<and>\<^sub>S\<^sub>L \<langle>[t\<diamondop>WAITQ]\<^sub>v =\<^sub>b [thd_next a]\<^sub>n\<rangle>\<^sub>S\<^sub>L) 
+  where "p9_post t s a list st = (stack_node s st \<and>\<^sub>S\<^sub>L \<langle>[ ADDR]\<^sub>v =\<^sub>b [s]\<^sub>n\<rangle>\<^sub>S\<^sub>L) ** (thread_node 
+  (stack_wait st) a \<and>\<^sub>S\<^sub>L \<langle>[FIRST_PENDING_THREAD]\<^sub>v =\<^sub>b [stack_wait st]\<^sub>n\<rangle>\<^sub>S\<^sub>L \<and>\<^sub>S\<^sub>L \<langle>[WAITQ]\<^sub>v =\<^sub>b [thd_next a]\<^sub>n\<rangle>\<^sub>S\<^sub>L) 
   ** (thread_wait_sl (thd_next a) list)"
 
 definition p10_pre :: "nat \<Rightarrow> nat \<Rightarrow> tcb \<Rightarrow> tcbs \<Rightarrow> stack_mem \<Rightarrow> assn"
-  where "p10_pre t s a list st = (stack_node s st \<and>\<^sub>S\<^sub>L \<langle>[t \<diamondop> ADDR]\<^sub>v =\<^sub>b [s]\<^sub>n\<rangle>\<^sub>S\<^sub>L \<and>\<^sub>S\<^sub>L \<langle>[t\<diamondop>WAITQ]\<^sub>v =\<^sub>b [thd_next a]\<^sub>n\<rangle>\<^sub>S\<^sub>L) 
-  ** (thread_node (stack_wait st) a \<and>\<^sub>S\<^sub>L \<langle>[t\<diamondop>FIRST_PENDING_THREAD]\<^sub>v =\<^sub>b [stack_wait st]\<^sub>n\<rangle>\<^sub>S\<^sub>L ) 
+  where "p10_pre t s a list st = (stack_node s st \<and>\<^sub>S\<^sub>L \<langle>[ ADDR]\<^sub>v =\<^sub>b [s]\<^sub>n\<rangle>\<^sub>S\<^sub>L \<and>\<^sub>S\<^sub>L \<langle>[WAITQ]\<^sub>v =\<^sub>b [thd_next a]\<^sub>n\<rangle>\<^sub>S\<^sub>L) 
+  ** (thread_node (stack_wait st) a \<and>\<^sub>S\<^sub>L \<langle>[FIRST_PENDING_THREAD]\<^sub>v =\<^sub>b [stack_wait st]\<^sub>n\<rangle>\<^sub>S\<^sub>L ) 
   ** (thread_wait_sl (thd_next a) list)"
 
 lemma p9_post_equiv_aux : "(P1 \<and>\<^sub>S\<^sub>L \<langle>P2\<rangle>\<^sub>S\<^sub>L \<and>\<^sub>S\<^sub>L \<langle>P3\<rangle>\<^sub>S\<^sub>L) ** (P4 \<and>\<^sub>S\<^sub>L \<langle>P5\<rangle>\<^sub>S\<^sub>L) ** P6 \<equiv>\<^sub>S\<^sub>L
@@ -177,39 +175,39 @@ lemma p9_post_equiv : "p10_pre t s a list st  \<equiv>\<^sub>S\<^sub>L p9_post t
   by (simp add: p10_pre_def p9_post_def p9_post_equiv_aux) 
 
 definition p10_post :: "nat \<Rightarrow> nat \<Rightarrow> tcb \<Rightarrow> tcbs \<Rightarrow> stack_mem \<Rightarrow> assn"
-  where "p10_post t s a list st = (stack_node s (st:=\<^sub>w\<^sub>a thd_next a) \<and>\<^sub>S\<^sub>L \<langle>[t \<diamondop> ADDR]\<^sub>v =\<^sub>b [s]\<^sub>n\<rangle>\<^sub>S\<^sub>L \<and>\<^sub>S\<^sub>L 
-  \<langle>[t\<diamondop>WAITQ]\<^sub>v =\<^sub>b [thd_next a]\<^sub>n\<rangle>\<^sub>S\<^sub>L)  ** (thread_node (stack_wait st) a \<and>\<^sub>S\<^sub>L \<langle>[t\<diamondop>FIRST_PENDING_THREAD]\<^sub>v 
+  where "p10_post t s a list st = (stack_node s (st:=\<^sub>w\<^sub>a thd_next a) \<and>\<^sub>S\<^sub>L \<langle>[ ADDR]\<^sub>v =\<^sub>b [s]\<^sub>n\<rangle>\<^sub>S\<^sub>L \<and>\<^sub>S\<^sub>L 
+  \<langle>[WAITQ]\<^sub>v =\<^sub>b [thd_next a]\<^sub>n\<rangle>\<^sub>S\<^sub>L)  ** (thread_node (stack_wait st) a \<and>\<^sub>S\<^sub>L \<langle>[FIRST_PENDING_THREAD]\<^sub>v 
   =\<^sub>b [stack_wait st]\<^sub>n\<rangle>\<^sub>S\<^sub>L) ** (thread_wait_sl (thd_next a) list)"
 
 definition p10_post_noframe :: "nat \<Rightarrow> nat \<Rightarrow> tcb \<Rightarrow> tcbs \<Rightarrow> stack_mem \<Rightarrow> assn"
   where "p10_post_noframe t s a list st = stack_node s (st:=\<^sub>w\<^sub>a thd_next a) ** (is_waitq (thd_next a) 
-  list) ** (thread_node (stack_wait st) a \<and>\<^sub>S\<^sub>L \<langle>[t\<diamondop>FIRST_PENDING_THREAD]\<^sub>v =\<^sub>b [stack_wait st]\<^sub>n\<rangle>\<^sub>S\<^sub>L) "
+  list) ** (thread_node (stack_wait st) a \<and>\<^sub>S\<^sub>L \<langle>[FIRST_PENDING_THREAD]\<^sub>v =\<^sub>b [stack_wait st]\<^sub>n\<rangle>\<^sub>S\<^sub>L) "
 
 lemma p10_post_implies : " p10_post t s a list st \<sqsubseteq> p10_post_noframe t s a list st"
   apply (rule_tac Q = "stack_node s (st :=\<^sub>w\<^sub>a thd_next a) ** (thread_node (stack_wait st) a \<and>\<^sub>S\<^sub>L 
-  \<langle>[t\<diamondop>FIRST_PENDING_THREAD]\<^sub>v =\<^sub>b [stack_wait st]\<^sub>n\<rangle>\<^sub>S\<^sub>L) ** thread_wait_sl (thd_next a) list" in implies_trans)
+  \<langle>[FIRST_PENDING_THREAD]\<^sub>v =\<^sub>b [stack_wait st]\<^sub>n\<rangle>\<^sub>S\<^sub>L) ** thread_wait_sl (thd_next a) list" in implies_trans)
    apply (simp add: p10_post_def implies_def) apply auto[1]
   apply (rule equiv_implies, simp add: p10_post_noframe_def)
   apply (rule_tac Q = "stack_node s (st :=\<^sub>w\<^sub>a thd_next a) ** (thread_node (stack_wait st) a \<and>\<^sub>S\<^sub>L 
-  \<langle>[t\<diamondop>FIRST_PENDING_THREAD]\<^sub>v =\<^sub>b [stack_wait st]\<^sub>n\<rangle>\<^sub>S\<^sub>L) ** is_waitq (thd_next a) list" in assn_equiv_trans)
+  \<langle>[FIRST_PENDING_THREAD]\<^sub>v =\<^sub>b [stack_wait st]\<^sub>n\<rangle>\<^sub>S\<^sub>L) ** is_waitq (thd_next a) list" in assn_equiv_trans)
    apply (meson Astar_commute_equiv assn_equiv_cong_star assn_equiv_symmetry assn_equiv_trans waitq_equiv)
   by (simp add: Astar_assoc_equiv2)
 
 lemma safe_p910_noframe : "\<lbrakk>fvAs \<Gamma> = {}; stack_pt st; stack_next st \<noteq> stack_top st\<rbrakk> \<Longrightarrow>
                  \<Gamma>(Cur := inv_cur, Readyq := inv_readyq, Stack := inv_stack) \<turnstile>
                           { p9_pre_noframe t s a list st}
-                          t\<diamondop>WAITQ :=\<^sub>C \<lbrakk>[t\<diamondop>FIRST_PENDING_THREAD]\<^sub>v\<Down>\<^sub>tnext\<rbrakk>;;
-                          \<lbrakk>[t\<diamondop>ADDR]\<^sub>v\<Down>\<^sub>swait\<rbrakk> :=\<^sub>C [t\<diamondop>WAITQ]\<^sub>v
+                          WAITQ :=\<^sub>C \<lbrakk>[FIRST_PENDING_THREAD]\<^sub>v\<Down>\<^sub>tnext\<rbrakk>;;
+                          \<lbrakk>[ADDR]\<^sub>v\<Down>\<^sub>swait\<rbrakk> :=\<^sub>C [WAITQ]\<^sub>v
                           { p10_post_noframe t s a list st}"
   apply (rule_tac P = "p9_pre t s a list st" and Q = "p10_post t s a list st" in rule_conseq)
     apply (rule_tac Q = "p9_post t s a list st" in rule_seq, simp add: p9_pre_def p9_post_def)
-     apply (rule rule_frame, rule rule_frame1, rule thread_node_readnext, simp add: Thread_Local_def)
+     apply (rule rule_frame, rule rule_frame1, rule thread_node_readnext, simp add: )
         apply (simp_all add: fvA_Gamma2 fvA_inv_cur fvA_inv_stack fvA_inv_readyq fvA_thread_wait_sl stack_node_def)
-       apply (simp add: Thread_Local_def, simp add: Thread_Local_def, simp add: disjoint_def Thread_Local_def)
+       apply (simp add: disjoint_def)
     apply (rule_tac Pa = "p10_pre t s a list st" and Qa = "p10_post t s a list st" in safe_assn_equiv)
       apply (simp add: p9_post_equiv, simp add: assn_equiv_reflex)
     apply (simp add: p10_pre_def p10_post_def, intro rule_frame, rule stack_node_write_wait_with_var)
-      apply (simp add: fvA_Gamma2 fvA_inv_cur fvA_inv_stack fvA_inv_readyq Thread_Local_def)
+      apply (simp add: fvA_Gamma2 fvA_inv_cur fvA_inv_stack fvA_inv_readyq )
      apply (simp add: fvA_thread_node fvA_thread_wait_sl, simp add: fvA_thread_wait_sl)
   by (simp add: p9_pre_implies, simp add: p10_post_implies)
 
@@ -218,7 +216,7 @@ definition p9_frame :: " nat \<Rightarrow> stack_mem \<Rightarrow> assn"
         \<and>\<^sub>S\<^sub>L (inv_stack_buf_waitq st) \<and>\<^sub>S\<^sub>L (inv_stack_pt st))"
 
 definition p13_pre_noframe :: "nat \<Rightarrow> tcb \<Rightarrow> stack_mem \<Rightarrow> assn"
-  where "p13_pre_noframe t a st = (thread_node (stack_wait st) a \<and>\<^sub>S\<^sub>L \<langle>[t\<diamondop>FIRST_PENDING_THREAD]\<^sub>v 
+  where "p13_pre_noframe t a st = (thread_node (stack_wait st) a \<and>\<^sub>S\<^sub>L \<langle>[FIRST_PENDING_THREAD]\<^sub>v 
   =\<^sub>b [stack_wait st]\<^sub>n\<rangle>\<^sub>S\<^sub>L)"
 
 lemma p9_pre_frame_implies_aux : "P1 ** P2 ** (P3 ** P4 \<and>\<^sub>S\<^sub>L \<langle>P5\<rangle>\<^sub>S\<^sub>L \<and>\<^sub>S\<^sub>L \<langle>P6\<rangle>\<^sub>S\<^sub>L) \<equiv>\<^sub>S\<^sub>L
@@ -231,9 +229,9 @@ lemma p9_pre_frame_implies_aux : "P1 ** P2 ** (P3 ** P4 \<and>\<^sub>S\<^sub>L \
    apply (simp add: assn_equiv_reflex, simp add: assn_equiv_def) by blast
 
 lemma p9_pre_frame_implies : "stack_tcbs st = a # list \<Longrightarrow> (p1_post t ** (p7_post_noframe t s st ** p4_frame st) 
-  \<and>\<^sub>S\<^sub>L \<langle>\<not>\<^sub>b [t\<diamondop>FIRST_PENDING_THREAD]\<^sub>v =\<^sub>b [K_NO_WAIT]\<^sub>n\<rangle>\<^sub>S\<^sub>L) \<sqsubseteq> p9_pre_noframe t s a list st ** p9_frame s st"
-  apply (rule_tac Q = "[A_Stack]\<^sub>v \<longmapsto> [s]\<^sub>n ** (stack_node s st \<and>\<^sub>S\<^sub>L \<langle>[t \<diamondop> ADDR]\<^sub>v =\<^sub>b [s]\<^sub>n\<rangle>\<^sub>S\<^sub>L \<and>\<^sub>S\<^sub>L 
-  \<langle>[t\<diamondop>FIRST_PENDING_THREAD]\<^sub>v =\<^sub>b [stack_wait st]\<^sub>n\<rangle>\<^sub>S\<^sub>L) ** p4_frame st" in implies_trans)
+  \<and>\<^sub>S\<^sub>L \<langle>\<not>\<^sub>b [FIRST_PENDING_THREAD]\<^sub>v =\<^sub>b [K_NO_WAIT]\<^sub>n\<rangle>\<^sub>S\<^sub>L) \<sqsubseteq> p9_pre_noframe t s a list st ** p9_frame s st"
+  apply (rule_tac Q = "[A_Stack]\<^sub>v \<longmapsto> [s]\<^sub>n ** (stack_node s st \<and>\<^sub>S\<^sub>L \<langle>[ ADDR]\<^sub>v =\<^sub>b [s]\<^sub>n\<rangle>\<^sub>S\<^sub>L \<and>\<^sub>S\<^sub>L 
+  \<langle>[FIRST_PENDING_THREAD]\<^sub>v =\<^sub>b [stack_wait st]\<^sub>n\<rangle>\<^sub>S\<^sub>L) ** p4_frame st" in implies_trans)
    apply (simp add: p1_post_def p7_post_noframe_def implies_def) apply auto[1]
   apply (rule equiv_implies, simp add: p4_frame_def p9_pre_noframe_def p9_frame_def)
   by (simp add: inv_stack_buf_waitq_def inv_stack_pt_def p9_pre_frame_implies_aux)
@@ -252,7 +250,7 @@ lemma p10_post_frame_equiv : "\<lbrakk> stack_next st \<noteq> stack_top st; sta
         stack_pt st; stack_wait st \<noteq> NULL\<rbrakk> \<Longrightarrow> p10_post_noframe t s a list st ** p9_frame s st \<equiv>\<^sub>S\<^sub>L 
         p13_pre_noframe t a st ** inv_stack1 s (st :=\<^sub>w\<^sub>a thd_next a :=\<^sub>t\<^sub>c list)"
   apply (simp add: inv_stack1_def p10_post_noframe_def p9_frame_def p13_pre_noframe_def)
-  apply (rule_tac Q = "(thread_node (stack_wait st) a \<and>\<^sub>S\<^sub>L \<langle>[t\<diamondop>FIRST_PENDING_THREAD]\<^sub>v =\<^sub>b [stack_wait st]\<^sub>n\<rangle>\<^sub>S\<^sub>L) 
+  apply (rule_tac Q = "(thread_node (stack_wait st) a \<and>\<^sub>S\<^sub>L \<langle>[FIRST_PENDING_THREAD]\<^sub>v =\<^sub>b [stack_wait st]\<^sub>n\<rangle>\<^sub>S\<^sub>L) 
   ** (([A_Stack]\<^sub>v \<longmapsto> [s]\<^sub>n) ** (stack_node s (st :=\<^sub>w\<^sub>a thd_next a) ** is_waitq (thd_next a) list ** buf 
   (stack_base st) (stack_top st) (stack_buf st) \<and>\<^sub>S\<^sub>L  inv_stack_buf_waitq st \<and>\<^sub>S\<^sub>L inv_stack_pt st))" 
   in assn_equiv_trans, simp add: inv_stack_buf_waitq_def inv_stack_pt_def p10_post_frame_equiv_aux)
@@ -266,38 +264,38 @@ lemma p10_post_frame_equiv : "\<lbrakk> stack_next st \<noteq> stack_top st; sta
 lemma safe_p910 : "\<lbrakk>fvAs \<Gamma> = {}; stack_next st \<noteq> stack_top st; stack_base st = stack_next st; 
                     stack_pt st; stack_wait st \<noteq> NULL; stack_tcbs st = a # list\<rbrakk> \<Longrightarrow>
                  \<Gamma>(Cur := inv_cur, Readyq := inv_readyq, Stack := inv_stack) \<turnstile>
-{(p1_post t ** (p7_post_noframe t s st ** p4_frame st) \<and>\<^sub>S\<^sub>L \<langle>\<not>\<^sub>b [t\<diamondop>FIRST_PENDING_THREAD]\<^sub>v =\<^sub>b [K_NO_WAIT]\<^sub>n\<rangle>\<^sub>S\<^sub>L)}
-                          t\<diamondop>WAITQ :=\<^sub>C \<lbrakk>[t\<diamondop>FIRST_PENDING_THREAD]\<^sub>v\<Down>\<^sub>tnext\<rbrakk>;;
-                          \<lbrakk>[t\<diamondop>ADDR]\<^sub>v\<Down>\<^sub>swait\<rbrakk> :=\<^sub>C [t\<diamondop>WAITQ]\<^sub>v  
+{(p1_post t ** (p7_post_noframe t s st ** p4_frame st) \<and>\<^sub>S\<^sub>L \<langle>\<not>\<^sub>b [FIRST_PENDING_THREAD]\<^sub>v =\<^sub>b [K_NO_WAIT]\<^sub>n\<rangle>\<^sub>S\<^sub>L)}
+                          WAITQ :=\<^sub>C \<lbrakk>[FIRST_PENDING_THREAD]\<^sub>v\<Down>\<^sub>tnext\<rbrakk>;;
+                          \<lbrakk>[ADDR]\<^sub>v\<Down>\<^sub>swait\<rbrakk> :=\<^sub>C [WAITQ]\<^sub>v  
 {p13_pre_noframe t a st ** inv_stack1 s (st :=\<^sub>w\<^sub>a thd_next a :=\<^sub>t\<^sub>c list)}"
   apply (rule_tac P = "p9_pre_noframe t s a list st ** p9_frame s st" and Q = "p10_post_noframe t s 
   a list st ** p9_frame s st" in rule_conseq)
     apply (rule rule_frame, rule safe_p910_noframe, simp_all)
-    apply (simp add: p9_frame_def fvA_buf inv_stack_pt_def inv_stack_buf_waitq_def disjoint_def Thread_Local_def)
+    apply (simp add: p9_frame_def fvA_buf inv_stack_pt_def inv_stack_buf_waitq_def disjoint_def )
   by (simp add: p9_pre_frame_implies, rule equiv_implies, rule p10_post_frame_equiv, simp_all)
 
 definition p11_pre_noframe :: "nat \<Rightarrow> nat \<Rightarrow> stack_mem \<Rightarrow> assn"
-  where "p11_pre_noframe t s st = (stack_node s st \<and>\<^sub>S\<^sub>L \<langle>[t \<diamondop> ADDR]\<^sub>v =\<^sub>b [s]\<^sub>n\<rangle>\<^sub>S\<^sub>L) ** (buf (stack_base st) 
-  (stack_top st) (stack_buf st) \<and>\<^sub>S\<^sub>L \<langle>[t \<diamondop> NEXT]\<^sub>v =\<^sub>b [stack_next st]\<^sub>n\<rangle>\<^sub>S\<^sub>L)"
+  where "p11_pre_noframe t s st = (stack_node s st \<and>\<^sub>S\<^sub>L \<langle>[ ADDR]\<^sub>v =\<^sub>b [s]\<^sub>n\<rangle>\<^sub>S\<^sub>L) ** (buf (stack_base st) 
+  (stack_top st) (stack_buf st) \<and>\<^sub>S\<^sub>L \<langle>[ NEXT]\<^sub>v =\<^sub>b [stack_next st]\<^sub>n\<rangle>\<^sub>S\<^sub>L)"
 
 definition p12_post_noframe :: "nat \<Rightarrow> nat \<Rightarrow> nat \<Rightarrow> stack_mem \<Rightarrow> assn"
   where "p12_post_noframe t s data st = stack_node s (st:=\<^sub>n\<^sub>e (stack_next st + 1)) ** buf (stack_base st) 
   (stack_top st) ((stack_buf st)[(stack_next st - stack_base st) := data])"
 
 definition p11_post :: "nat \<Rightarrow> nat \<Rightarrow> nat \<Rightarrow> stack_mem \<Rightarrow> assn"
-  where "p11_post t s data st = (stack_node s st \<and>\<^sub>S\<^sub>L \<langle>[t \<diamondop> ADDR]\<^sub>v =\<^sub>b [s]\<^sub>n\<rangle>\<^sub>S\<^sub>L) ** (buf (stack_base st) 
-  (stack_top st) ((stack_buf st)[(stack_next st -stack_base st) := data]) \<and>\<^sub>S\<^sub>L \<langle>[t \<diamondop> NEXT]\<^sub>v =\<^sub>b [stack_next st]\<^sub>n\<rangle>\<^sub>S\<^sub>L)"
+  where "p11_post t s data st = (stack_node s st \<and>\<^sub>S\<^sub>L \<langle>[ ADDR]\<^sub>v =\<^sub>b [s]\<^sub>n\<rangle>\<^sub>S\<^sub>L) ** (buf (stack_base st) 
+  (stack_top st) ((stack_buf st)[(stack_next st -stack_base st) := data]) \<and>\<^sub>S\<^sub>L \<langle>[ NEXT]\<^sub>v =\<^sub>b [stack_next st]\<^sub>n\<rangle>\<^sub>S\<^sub>L)"
 
 definition p12_pre :: "nat \<Rightarrow> nat \<Rightarrow> nat \<Rightarrow> stack_mem \<Rightarrow> assn"
-  where "p12_pre t s data st = (stack_node s st \<and>\<^sub>S\<^sub>L \<langle>[t \<diamondop> ADDR]\<^sub>v =\<^sub>b [s]\<^sub>n\<rangle>\<^sub>S\<^sub>L \<and>\<^sub>S\<^sub>L \<langle>[t \<diamondop> NEXT]\<^sub>v =\<^sub>b [stack_next st]\<^sub>n\<rangle>\<^sub>S\<^sub>L) 
+  where "p12_pre t s data st = (stack_node s st \<and>\<^sub>S\<^sub>L \<langle>[ ADDR]\<^sub>v =\<^sub>b [s]\<^sub>n\<rangle>\<^sub>S\<^sub>L \<and>\<^sub>S\<^sub>L \<langle>[ NEXT]\<^sub>v =\<^sub>b [stack_next st]\<^sub>n\<rangle>\<^sub>S\<^sub>L) 
   ** buf (stack_base st) (stack_top st) ((stack_buf st)[(stack_next st -stack_base st) := data])"
 
 lemma p12_pre_equiv : " p12_pre t s data st \<equiv>\<^sub>S\<^sub>L p11_post t s data st"
   apply (simp add: assn_equiv_def p12_pre_def p11_post_def) by auto
 
 definition p12_post :: "nat \<Rightarrow> nat \<Rightarrow> nat \<Rightarrow> stack_mem \<Rightarrow> assn"
-  where "p12_post t s data st = (stack_node s (st:=\<^sub>n\<^sub>e (stack_next st + 1)) \<and>\<^sub>S\<^sub>L \<langle>[t \<diamondop> ADDR]\<^sub>v =\<^sub>b [s]\<^sub>n\<rangle>\<^sub>S\<^sub>L 
-  \<and>\<^sub>S\<^sub>L \<langle>[t \<diamondop> NEXT]\<^sub>v =\<^sub>b [stack_next st]\<^sub>n\<rangle>\<^sub>S\<^sub>L) ** buf (stack_base st) (stack_top st) ((stack_buf st)
+  where "p12_post t s data st = (stack_node s (st:=\<^sub>n\<^sub>e (stack_next st + 1)) \<and>\<^sub>S\<^sub>L \<langle>[ ADDR]\<^sub>v =\<^sub>b [s]\<^sub>n\<rangle>\<^sub>S\<^sub>L 
+  \<and>\<^sub>S\<^sub>L \<langle>[ NEXT]\<^sub>v =\<^sub>b [stack_next st]\<^sub>n\<rangle>\<^sub>S\<^sub>L) ** buf (stack_base st) (stack_top st) ((stack_buf st)
   [(stack_next st -stack_base st) := data])"
 
 lemma p12_post_implies : "p12_post t s data st \<sqsubseteq> p12_post_noframe t s data st"
@@ -306,21 +304,21 @@ lemma p12_post_implies : "p12_post t s data st \<sqsubseteq> p12_post_noframe t 
 lemma safe_p1112_noframe : "\<lbrakk>fvAs \<Gamma> = {}; stack_pt st; stack_next st \<noteq> stack_top st; t \<noteq> NULL\<rbrakk> \<Longrightarrow>
                  \<Gamma>(Cur := inv_cur, Readyq := inv_readyq, Stack := inv_stack) \<turnstile>
                           { p11_pre_noframe t s st}
-                      (t \<^enum> \<lbrakk>[t \<diamondop> NEXT]\<^sub>v\<rbrakk> :=\<^sub>C [data]\<^sub>n) ;;
-                      (t \<^enum>  \<lbrakk>[t \<diamondop> ADDR]\<^sub>v\<Down>\<^sub>snext\<rbrakk> :=\<^sub>C [t \<diamondop> NEXT]\<^sub>v +\<^sub>e [1]\<^sub>n)
+                      (t \<^enum> \<lbrakk>[ NEXT]\<^sub>v\<rbrakk> :=\<^sub>C [data]\<^sub>n) ;;
+                      (t \<^enum>  \<lbrakk>[ ADDR]\<^sub>v\<Down>\<^sub>snext\<rbrakk> :=\<^sub>C [ NEXT]\<^sub>v +\<^sub>e [1]\<^sub>n)
                           { p12_post_noframe t s data st}"
   apply (rule_tac Q = "p11_post t s data st" in rule_seq, simp add: p11_pre_noframe_def p11_post_def)
    apply (rule rule_frame1, rule rule_stm_stack', simp, simp)
-        apply (simp add: fvA_buf Thread_Local_def, simp add: fvA_buf Thread_Local_def, simp)
-  apply (simp add: fvA_buf, simp add: Thread_Local_def)
+        apply (simp add: fvA_buf , simp add: fvA_buf , simp)
+  apply (simp add: fvA_buf)
     apply (rule update_buf_with_var, simp add: stack_pt_def, simp add: stack_node_def)
-  apply (simp add: stm_def disjoint_def Thread_Local_def stack_node_def)
+  apply (simp add: stm_def disjoint_def  stack_node_def)
   apply (rule_tac P = "p12_pre t s data st" and Q = "p12_post t s data st" in rule_conseq)
     apply (simp only: p12_post_def p12_pre_def, rule rule_frame, rule rule_stm_stack', simp, simp)
-       apply (simp add: stack_node_def Thread_Local_def, simp)
-  apply (simp add: stack_node_def Thread_Local_def)
-     apply (rule stack_node_write_next_add1, simp add: Thread_Local_def)
-      apply (simp_all add: fvA_Gamma2 fvA_inv_cur fvA_inv_readyq fvA_buf fvA_inv_stack Thread_Local_def)
+       apply (simp add: stack_node_def , simp)
+  apply (simp add: stack_node_def )
+     apply (rule stack_node_write_next_add1, simp add: )
+      apply (simp_all add: fvA_Gamma2 fvA_inv_cur fvA_inv_readyq fvA_buf fvA_inv_stack )
   by (simp add: assn_equiv_symmetry equiv_implies p12_pre_equiv, simp add: p12_post_implies)
 
 definition p11_frame :: "nat \<Rightarrow> stack_mem \<Rightarrow> assn"
@@ -336,10 +334,10 @@ lemma p11_pre_frame_implies_aux : "P1 ** (P2 \<and>\<^sub>S\<^sub>L \<langle>P3\
    stack_node_equiv1_aux stack_node_equiv2_aux)
    apply (simp add: assn_equiv_reflex, simp add: assn_equiv_def) by blast
 
-lemma p11_pre_frame_implies : "(p7_post_noframe t s st ** p4_frame st \<and>\<^sub>S\<^sub>L\<langle>[t\<diamondop>FIRST_PENDING_THREAD]\<^sub>v 
+lemma p11_pre_frame_implies : "(p7_post_noframe t s st ** p4_frame st \<and>\<^sub>S\<^sub>L\<langle>[FIRST_PENDING_THREAD]\<^sub>v 
                         =\<^sub>b [K_NO_WAIT]\<^sub>n\<rangle>\<^sub>S\<^sub>L) \<sqsubseteq> p11_pre_noframe t s st ** p11_frame s st"
-  apply (rule_tac Q = "([A_Stack]\<^sub>v \<longmapsto> [s]\<^sub>n ** (stack_node s st \<and>\<^sub>S\<^sub>L \<langle>[t\<diamondop>ADDR]\<^sub>v =\<^sub>b [s]\<^sub>n\<rangle>\<^sub>S\<^sub>L \<and>\<^sub>S\<^sub>L
-      \<langle>[t\<diamondop>NEXT]\<^sub>v =\<^sub>b [stack_next st]\<^sub>n\<rangle>\<^sub>S\<^sub>L)) ** p4_frame st" in implies_trans)
+  apply (rule_tac Q = "([A_Stack]\<^sub>v \<longmapsto> [s]\<^sub>n ** (stack_node s st \<and>\<^sub>S\<^sub>L \<langle>[ADDR]\<^sub>v =\<^sub>b [s]\<^sub>n\<rangle>\<^sub>S\<^sub>L \<and>\<^sub>S\<^sub>L
+      \<langle>[NEXT]\<^sub>v =\<^sub>b [stack_next st]\<^sub>n\<rangle>\<^sub>S\<^sub>L)) ** p4_frame st" in implies_trans)
    apply (simp add: p7_post_noframe_def implies_def) apply auto[1]
   apply (rule equiv_implies, simp add: p4_frame_def p11_pre_noframe_def p11_frame_def)
   by (simp add: inv_stack_buf_waitq_def inv_stack_pt_def p11_pre_frame_implies_aux)
@@ -371,14 +369,14 @@ thm p11_pre_frame_implies
 lemma safe_p1112 : "\<lbrakk>fvAs \<Gamma> = {}; stack_pt st; stack_next st \<noteq> stack_top st; stack_wait st = NULL; 
                      t \<noteq> NULL\<rbrakk> \<Longrightarrow>
                  \<Gamma>(Cur := inv_cur, Readyq := inv_readyq, Stack := inv_stack) \<turnstile>
-           {  p7_post_noframe t s st ** p4_frame st \<and>\<^sub>S\<^sub>L \<langle>[t\<diamondop>FIRST_PENDING_THREAD]\<^sub>v =\<^sub>b [K_NO_WAIT]\<^sub>n\<rangle>\<^sub>S\<^sub>L }
-                (t \<^enum> \<lbrakk>[t \<diamondop> NEXT]\<^sub>v\<rbrakk> :=\<^sub>C [data]\<^sub>n) ;;
-                (t \<^enum>  \<lbrakk>[t \<diamondop> ADDR]\<^sub>v\<Down>\<^sub>snext\<rbrakk> :=\<^sub>C [t \<diamondop> NEXT]\<^sub>v +\<^sub>e [1]\<^sub>n)
+           {  p7_post_noframe t s st ** p4_frame st \<and>\<^sub>S\<^sub>L \<langle>[FIRST_PENDING_THREAD]\<^sub>v =\<^sub>b [K_NO_WAIT]\<^sub>n\<rangle>\<^sub>S\<^sub>L }
+                (t \<^enum> \<lbrakk>[ NEXT]\<^sub>v\<rbrakk> :=\<^sub>C [data]\<^sub>n) ;;
+                (t \<^enum>  \<lbrakk>[ ADDR]\<^sub>v\<Down>\<^sub>snext\<rbrakk> :=\<^sub>C [ NEXT]\<^sub>v +\<^sub>e [1]\<^sub>n)
                  { inv_stack }"
   apply (rule_tac P = " p11_pre_noframe t s st ** p11_frame s st" and Q = "p12_post_noframe t s data st 
   ** p11_frame s st" in rule_conseq, rule rule_frame, rule safe_p1112_noframe, simp_all)
     apply (simp add: p11_frame_def stm_def disjoint_def fvA_is_waitq inv_stack_pt_def)
-    apply (simp add: inv_stack_buf_waitq_def, simp add: Thread_Local_def)
+    apply (simp add: inv_stack_buf_waitq_def)
   apply (rule p11_pre_frame_implies)
   apply (rule_tac Q = "inv_stack1 s (st :=\<^sub>n\<^sub>e (stack_next st + 1) :=\<^sub>b\<^sub>f ((stack_buf st)[(stack_next st 
   -stack_base st) := data]))" in implies_trans)
@@ -387,17 +385,17 @@ lemma safe_p1112 : "\<lbrakk>fvAs \<Gamma> = {}; stack_pt st; stack_next st \<no
 
 definition p14_post_noframe :: "nat \<Rightarrow> nat \<Rightarrow> tcb \<Rightarrow> stack_mem \<Rightarrow> assn"
   where "p14_post_noframe t d a st = (thread_node (stack_wait st) (a :=\<^sub>s\<^sub>t READY :=\<^sub>d\<^sub>t d) 
-  \<and>\<^sub>S\<^sub>L \<langle>[t\<diamondop>FIRST_PENDING_THREAD]\<^sub>v =\<^sub>b [stack_wait st]\<^sub>n\<rangle>\<^sub>S\<^sub>L)"
+  \<and>\<^sub>S\<^sub>L \<langle>[FIRST_PENDING_THREAD]\<^sub>v =\<^sub>b [stack_wait st]\<^sub>n\<rangle>\<^sub>S\<^sub>L)"
 
 definition p13_post :: "nat  \<Rightarrow> tcb \<Rightarrow> stack_mem \<Rightarrow> assn"
   where "p13_post t a st = (thread_node (stack_wait st) (a :=\<^sub>s\<^sub>t READY) \<and>\<^sub>S\<^sub>L 
-  \<langle>[t\<diamondop>FIRST_PENDING_THREAD]\<^sub>v =\<^sub>b [stack_wait st]\<^sub>n\<rangle>\<^sub>S\<^sub>L)"
+  \<langle>[FIRST_PENDING_THREAD]\<^sub>v =\<^sub>b [stack_wait st]\<^sub>n\<rangle>\<^sub>S\<^sub>L)"
 
 lemma safe_p1314_noframe : "\<lbrakk>fvAs \<Gamma> = {}; stack_pt st; stack_next st \<noteq> stack_top st\<rbrakk> \<Longrightarrow>
                  \<Gamma>(Cur := inv_cur, Readyq := inv_readyq, Stack := inv_stack) \<turnstile>
                           {p13_pre_noframe t a st}
-              \<lbrakk>[t \<diamondop> FIRST_PENDING_THREAD]\<^sub>v\<Down>\<^sub>tstate\<rbrakk> :=\<^sub>C [READY]\<^sub>n ;;
-              \<lbrakk>[t \<diamondop> FIRST_PENDING_THREAD]\<^sub>v\<Down>\<^sub>tdata\<rbrakk> :=\<^sub>C [d]\<^sub>n
+              \<lbrakk>[ FIRST_PENDING_THREAD]\<^sub>v\<Down>\<^sub>tstate\<rbrakk> :=\<^sub>C [READY]\<^sub>n ;;
+              \<lbrakk>[ FIRST_PENDING_THREAD]\<^sub>v\<Down>\<^sub>tdata\<rbrakk> :=\<^sub>C [d]\<^sub>n
                           { p14_post_noframe t d a st}"
   apply (rule_tac Q = "p13_post t a st" in rule_seq, simp only: p13_pre_noframe_def p13_post_def)
    apply (rule thread_node_write_st', simp only: p13_post_def p14_post_noframe_def)
@@ -406,9 +404,9 @@ lemma safe_p1314_noframe : "\<lbrakk>fvAs \<Gamma> = {}; stack_pt st; stack_next
 lemma safe_p1314 : "\<lbrakk>fvAs \<Gamma> = {}; stack_pt st; stack_next st \<noteq> stack_top st\<rbrakk> \<Longrightarrow>
                  \<Gamma>(Cur := inv_cur, Readyq := inv_readyq, Stack := inv_stack) \<turnstile>
    {p13_pre_noframe t a st ** inv_stack1 s (st :=\<^sub>w\<^sub>a thd_next a :=\<^sub>t\<^sub>c list) \<and>\<^sub>S\<^sub>L 
-            \<langle>\<not>\<^sub>b [t\<diamondop>FIRST_PENDING_THREAD]\<^sub>v =\<^sub>b [K_NO_WAIT]\<^sub>n\<rangle>\<^sub>S\<^sub>L}
-              \<lbrakk>[t \<diamondop> FIRST_PENDING_THREAD]\<^sub>v\<Down>\<^sub>tstate\<rbrakk> :=\<^sub>C [READY]\<^sub>n ;;
-              \<lbrakk>[t \<diamondop> FIRST_PENDING_THREAD]\<^sub>v\<Down>\<^sub>tdata\<rbrakk> :=\<^sub>C [d]\<^sub>n
+            \<langle>\<not>\<^sub>b [FIRST_PENDING_THREAD]\<^sub>v =\<^sub>b [K_NO_WAIT]\<^sub>n\<rangle>\<^sub>S\<^sub>L}
+              \<lbrakk>[ FIRST_PENDING_THREAD]\<^sub>v\<Down>\<^sub>tstate\<rbrakk> :=\<^sub>C [READY]\<^sub>n ;;
+              \<lbrakk>[ FIRST_PENDING_THREAD]\<^sub>v\<Down>\<^sub>tdata\<rbrakk> :=\<^sub>C [d]\<^sub>n
                 { p14_post_noframe t d a st ** inv_stack1 s (st :=\<^sub>w\<^sub>a thd_next a :=\<^sub>t\<^sub>c list)}"
   apply (rule_tac P = "p13_pre_noframe t a st ** inv_stack1 s (st :=\<^sub>w\<^sub>a thd_next a :=\<^sub>t\<^sub>c list)" and 
   Q = "p14_post_noframe t d a st ** inv_stack1 s (st :=\<^sub>w\<^sub>a thd_next a :=\<^sub>t\<^sub>c list)" in rule_conseq)
@@ -417,11 +415,11 @@ lemma safe_p1314 : "\<lbrakk>fvAs \<Gamma> = {}; stack_pt st; stack_next st \<no
 
 definition p15_post :: "nat \<Rightarrow> nat \<Rightarrow> tcb \<Rightarrow> stack_mem \<Rightarrow> nat \<Rightarrow> tcbs \<Rightarrow> assn"
   where "p15_post t d a st r xs = p14_post_noframe t d a st ** (([A_Readyq]\<^sub>v \<longmapsto> [r]\<^sub>n \<and>\<^sub>S\<^sub>L 
-  \<langle>[t\<diamondop>FIRST_READY]\<^sub>v =\<^sub>b [r]\<^sub>n\<rangle>\<^sub>S\<^sub>L) ** is_readyq r xs)"
+  \<langle>[FIRST_READY]\<^sub>v =\<^sub>b [r]\<^sub>n\<rangle>\<^sub>S\<^sub>L) ** is_readyq r xs)"
 
 definition p16_pre :: "nat \<Rightarrow> nat \<Rightarrow> tcb \<Rightarrow> stack_mem \<Rightarrow> nat \<Rightarrow> tcbs \<Rightarrow> assn"
   where "p16_pre t d a st r xs = (thread_node (stack_wait st) (a :=\<^sub>s\<^sub>t READY :=\<^sub>d\<^sub>t d) \<and>\<^sub>S\<^sub>L 
-  \<langle>[t\<diamondop>FIRST_PENDING_THREAD]\<^sub>v =\<^sub>b [stack_wait st]\<^sub>n\<rangle>\<^sub>S\<^sub>L \<and>\<^sub>S\<^sub>L \<langle>[t\<diamondop>FIRST_READY]\<^sub>v =\<^sub>b [r]\<^sub>n\<rangle>\<^sub>S\<^sub>L) ** (([A_Readyq]\<^sub>v
+  \<langle>[FIRST_PENDING_THREAD]\<^sub>v =\<^sub>b [stack_wait st]\<^sub>n\<rangle>\<^sub>S\<^sub>L \<and>\<^sub>S\<^sub>L \<langle>[FIRST_READY]\<^sub>v =\<^sub>b [r]\<^sub>n\<rangle>\<^sub>S\<^sub>L) ** (([A_Readyq]\<^sub>v
    \<longmapsto> [r]\<^sub>n) ** is_readyq r xs)"
 
 lemma p15_post_equiv : "p16_pre t d a st r xs  \<equiv>\<^sub>S\<^sub>L p15_post t d a st r xs"
@@ -429,19 +427,19 @@ lemma p15_post_equiv : "p16_pre t d a st r xs  \<equiv>\<^sub>S\<^sub>L p15_post
 
 definition p16_post :: "nat \<Rightarrow> nat \<Rightarrow> tcb \<Rightarrow> stack_mem \<Rightarrow> nat \<Rightarrow> tcbs \<Rightarrow> assn"
   where "p16_post t d a st r xs = (thread_node (stack_wait st) (a :=\<^sub>s\<^sub>t READY :=\<^sub>d\<^sub>t d :=\<^sub>n\<^sub>x r) \<and>\<^sub>S\<^sub>L 
-  \<langle>[t\<diamondop>FIRST_PENDING_THREAD]\<^sub>v =\<^sub>b [stack_wait st]\<^sub>n\<rangle>\<^sub>S\<^sub>L \<and>\<^sub>S\<^sub>L \<langle>[t\<diamondop>FIRST_READY]\<^sub>v =\<^sub>b [r]\<^sub>n\<rangle>\<^sub>S\<^sub>L) ** (([A_Readyq]\<^sub>v
+  \<langle>[FIRST_PENDING_THREAD]\<^sub>v =\<^sub>b [stack_wait st]\<^sub>n\<rangle>\<^sub>S\<^sub>L \<and>\<^sub>S\<^sub>L \<langle>[FIRST_READY]\<^sub>v =\<^sub>b [r]\<^sub>n\<rangle>\<^sub>S\<^sub>L) ** (([A_Readyq]\<^sub>v
    \<longmapsto> [r]\<^sub>n) ** is_readyq r xs)"
 
 definition p17_pre :: "nat \<Rightarrow> nat \<Rightarrow> tcb \<Rightarrow> stack_mem \<Rightarrow> nat \<Rightarrow> tcbs \<Rightarrow> assn"
   where "p17_pre t d a st r xs = (thread_node (stack_wait st) (a :=\<^sub>s\<^sub>t READY :=\<^sub>d\<^sub>t d :=\<^sub>n\<^sub>x r)) ** (
-  ([A_Readyq]\<^sub>v  \<longmapsto> [r]\<^sub>n \<and>\<^sub>S\<^sub>L \<langle>[t\<diamondop>FIRST_PENDING_THREAD]\<^sub>v =\<^sub>b [stack_wait st]\<^sub>n\<rangle>\<^sub>S\<^sub>L) ** is_readyq r xs)"
+  ([A_Readyq]\<^sub>v  \<longmapsto> [r]\<^sub>n \<and>\<^sub>S\<^sub>L \<langle>[FIRST_PENDING_THREAD]\<^sub>v =\<^sub>b [stack_wait st]\<^sub>n\<rangle>\<^sub>S\<^sub>L) ** is_readyq r xs)"
 
 lemma p16_post_implies : " p16_post t d a st r xs \<sqsubseteq> p17_pre t d a st r xs"
   apply (simp add: p16_post_def p17_pre_def implies_def) by blast
 
 definition p17_post :: "nat \<Rightarrow> nat \<Rightarrow> tcb \<Rightarrow> stack_mem \<Rightarrow> nat \<Rightarrow> tcbs \<Rightarrow> assn"
   where "p17_post t d a st r xs = (thread_node (stack_wait st) (a :=\<^sub>s\<^sub>t READY :=\<^sub>d\<^sub>t d :=\<^sub>n\<^sub>x r)) ** (
-  ([A_Readyq]\<^sub>v  \<longmapsto> [stack_wait st]\<^sub>n \<and>\<^sub>S\<^sub>L \<langle>[t\<diamondop>FIRST_PENDING_THREAD]\<^sub>v =\<^sub>b [stack_wait st]\<^sub>n\<rangle>\<^sub>S\<^sub>L) ** is_readyq r xs)"
+  ([A_Readyq]\<^sub>v  \<longmapsto> [stack_wait st]\<^sub>n \<and>\<^sub>S\<^sub>L \<langle>[FIRST_PENDING_THREAD]\<^sub>v =\<^sub>b [stack_wait st]\<^sub>n\<rangle>\<^sub>S\<^sub>L) ** is_readyq r xs)"
 
 definition p18_pre :: "nat \<Rightarrow> nat \<Rightarrow> tcb \<Rightarrow> stack_mem \<Rightarrow> nat \<Rightarrow> tcbs \<Rightarrow> assn"
   where "p18_pre t d a st r xs = (thread_node (stack_wait st) (a :=\<^sub>s\<^sub>t READY :=\<^sub>d\<^sub>t d :=\<^sub>n\<^sub>x r)) ** (
@@ -463,18 +461,18 @@ lemma p17_post_implies : "p17_post t d a st r xs \<sqsubseteq> inv_readyq1 (stac
 lemma safe_p1517_noframe : "fvAs \<Gamma> = {} \<Longrightarrow> 
                 \<Gamma>(Cur := inv_cur, Readyq := inv_readyq, Stack := inv_stack) \<turnstile>
                   {p14_post_noframe t d a st ** inv_readyq1 r xs}
-                  t\<diamondop>FIRST_READY :=\<^sub>C \<lbrakk>[A_Readyq]\<^sub>v\<rbrakk>;; 
-                  \<lbrakk>[t\<diamondop>FIRST_PENDING_THREAD]\<^sub>v\<Down>\<^sub>tnext\<rbrakk> :=\<^sub>C [t\<diamondop>FIRST_READY]\<^sub>v;;
-                  \<lbrakk>[A_Readyq]\<^sub>v\<rbrakk> :=\<^sub>C [t\<diamondop>FIRST_PENDING_THREAD]\<^sub>v
+                  FIRST_READY :=\<^sub>C \<lbrakk>[A_Readyq]\<^sub>v\<rbrakk>;; 
+                  \<lbrakk>[FIRST_PENDING_THREAD]\<^sub>v\<Down>\<^sub>tnext\<rbrakk> :=\<^sub>C [FIRST_READY]\<^sub>v;;
+                  \<lbrakk>[A_Readyq]\<^sub>v\<rbrakk> :=\<^sub>C [FIRST_PENDING_THREAD]\<^sub>v
             {inv_readyq1 (stack_wait st) ((a :=\<^sub>s\<^sub>t READY :=\<^sub>d\<^sub>t d :=\<^sub>n\<^sub>x r) # xs)}"
   apply (rule_tac Q = "p16_post t d a st r xs" in rule_seq)
     apply (rule_tac Q = "p15_post t d a st r xs" in rule_seq, simp add: p15_post_def)
      apply (rule rule_frame1, simp add: inv_readyq1_def, rule rule_frame)
-  apply (rule_tac P = "[A_Readyq]\<^sub>v \<longmapsto> [r]\<^sub>n" and Q = "[A_Readyq]\<^sub>v \<longmapsto> [r]\<^sub>n \<and>\<^sub>S\<^sub>L \<langle>[t\<diamondop>FIRST_READY]\<^sub>v =\<^sub>b 
+  apply (rule_tac P = "[A_Readyq]\<^sub>v \<longmapsto> [r]\<^sub>n" and Q = "[A_Readyq]\<^sub>v \<longmapsto> [r]\<^sub>n \<and>\<^sub>S\<^sub>L \<langle>[FIRST_READY]\<^sub>v =\<^sub>b 
   [r]\<^sub>n\<rangle>\<^sub>S\<^sub>L" in rule_conseq, rule rule_read, simp add: fvA_Gamma2 fvA_inv_cur fvA_inv_stack fvA_inv_stack)
-         apply (simp add: fvA_inv_readyq Thread_Local_def, simp add: implies_def, simp add: implies_def)
+         apply (simp add: fvA_inv_readyq , simp add: implies_def, simp add: implies_def)
   apply (simp add: disjoint_def fvA_is_readyq, simp add: p14_post_noframe_def fvA_thread_node)
-     apply (simp add: disjoint_def Thread_Local_def)
+     apply (simp add: disjoint_def )
     apply (rule_tac Pa = "p16_pre t d a st r xs" and Qa = "p16_post t d a st r xs" in safe_assn_equiv)
       apply (simp add: p15_post_equiv, simp add: assn_equiv_reflex)
     apply (simp add: p16_pre_def p16_post_def, rule rule_frame, rule thread_node_write_next_fromvar)
@@ -486,15 +484,15 @@ lemma safe_p1517_noframe : "fvAs \<Gamma> = {} \<Longrightarrow>
 lemma safe_p1517 : "fvAs \<Gamma> = {} \<Longrightarrow> 
                 \<Gamma>(Cur := inv_cur, Readyq := inv_readyq, Stack := inv_stack) \<turnstile>
       {p14_post_noframe t d a st ** inv_stack1 s (st :=\<^sub>w\<^sub>a thd_next a :=\<^sub>t\<^sub>c list) ** inv_readyq1 r xs}
-                  t\<diamondop>FIRST_READY :=\<^sub>C \<lbrakk>[A_Readyq]\<^sub>v\<rbrakk>;; 
-                  \<lbrakk>[t\<diamondop>FIRST_PENDING_THREAD]\<^sub>v\<Down>\<^sub>tnext\<rbrakk> :=\<^sub>C [t\<diamondop>FIRST_READY]\<^sub>v;;
-                  \<lbrakk>[A_Readyq]\<^sub>v\<rbrakk> :=\<^sub>C [t\<diamondop>FIRST_PENDING_THREAD]\<^sub>v
+                  FIRST_READY :=\<^sub>C \<lbrakk>[A_Readyq]\<^sub>v\<rbrakk>;; 
+                  \<lbrakk>[FIRST_PENDING_THREAD]\<^sub>v\<Down>\<^sub>tnext\<rbrakk> :=\<^sub>C [FIRST_READY]\<^sub>v;;
+                  \<lbrakk>[A_Readyq]\<^sub>v\<rbrakk> :=\<^sub>C [FIRST_PENDING_THREAD]\<^sub>v
                   {inv_stack ** inv_readyq }"
   apply (rule_tac P = "inv_stack1 s (st :=\<^sub>w\<^sub>a thd_next a :=\<^sub>t\<^sub>c list) ** (p14_post_noframe t d a st **
   inv_readyq1 r xs)" and Q = "inv_stack1 s (st :=\<^sub>w\<^sub>a thd_next a :=\<^sub>t\<^sub>c list) ** inv_readyq1 (stack_wait st) 
   ((a :=\<^sub>s\<^sub>t READY :=\<^sub>d\<^sub>t d :=\<^sub>n\<^sub>x r) # xs)" in rule_conseq)
     apply (rule rule_frame1, rule safe_p1517_noframe, simp, simp add: inv_stack1_def fvA_is_stack)
-    apply (simp add: disjoint_def Thread_Local_def) apply (rule equiv_implies) 
+    apply (simp add: disjoint_def ) apply (rule equiv_implies) 
   using Astar_assoc_equiv2 Astar_commute_equiv assn_equiv_trans apply blast
   by (simp add: implies_star inv_readyq_implies inv_stack_implies)
 
@@ -508,16 +506,18 @@ lemma rule_inv_readyq : "\<forall>r xs. \<Gamma> \<turnstile> {P ** inv_readyq1 
 lemma safe_push : "fvAs \<Gamma> = {} \<Longrightarrow> 
                    \<Gamma>(Cur := inv_cur, Readyq := inv_readyq, Stack := inv_stack) \<turnstile>
                     {Aemp \<and>\<^sub>S\<^sub>L \<langle>[t \<noteq> NULL]\<^sub>b\<rangle>\<^sub>S\<^sub>L} stack_push t d { Aemp}"
-  apply (simp add: stack_push_def, case_tac t, simp add: CSL_def) using stm_def apply auto[1]
+  apply (simp only: stack_push_def) 
+  apply (rule rule_Clocals)
+  apply (case_tac t, simp add: CSL_def) 
+  using stm_def apply auto[1]
   apply (rule_tac Pa = "Aemp" and Qa = "Aemp" in safe_assn_equiv)
   apply (simp add: assn_equiv_def, simp add: assn_equiv_def)
   apply (rule_tac Q = "Aemp" in rule_seq)
    apply (rule_tac Q = "p1_post t" in rule_seq, simp add: p1_post_def)
-    apply (rule rule_stm_stack', simp_all, simp add: disjoint_def Thread_Local_def)
-    apply (rule_tac Pa = "Aemp" and Qa = "(Aemp  \<and>\<^sub>S\<^sub>L \<langle>[t\<diamondop>END]\<^sub>v =\<^sub>b [0]\<^sub>n\<rangle>\<^sub>S\<^sub>L)"
+    apply (rule rule_stm_stack', simp_all, simp add: disjoint_def )
+    apply (rule_tac Pa = "Aemp" and Qa = "(Aemp  \<and>\<^sub>S\<^sub>L \<langle>[END]\<^sub>v =\<^sub>b [0]\<^sub>n\<rangle>\<^sub>S\<^sub>L)"
     in safe_assn_equiv, simp add: assn_equiv_def, simp add: assn_equiv_def) apply auto[1]
-     apply (simp, rule rule_assign_num1, simp add: fvA_Gamma2 fvA_inv_stack fvA_inv_cur fvA_inv_readyq)
-  apply (simp add: Thread_Local_def, simp add: Thread_Local_def)
+     apply (rule rule_assign_num1, simp add: fvA_Gamma2 fvA_inv_stack fvA_inv_cur fvA_inv_readyq)
    apply (rule rule_with_true, simp, rule rule_inv_stack, intro allI)
    apply (rule_tac Q = "p1_post t ** (p4_post_noframe t s st ** p4_frame st)" in rule_seq, simp add: safe_p24)
    apply (rule rule_if, rule_tac P = "inv_stack1 s st" and Q = "inv_stack1 s st" in rule_conseq)
@@ -531,19 +531,18 @@ lemma safe_push : "fvAs \<Gamma> = {} \<Longrightarrow>
 (* stack_wait st = NULL *)
   apply (case_tac "stack_wait st")
    apply (rule_tac Q = "p7_post_noframe t s st ** p4_frame st" in rule_seq)
-         apply (rule rule_stm_stack', simp_all, simp add: disjoint_def Thread_Local_def)
+         apply (rule rule_stm_stack', simp_all, simp add: disjoint_def )
             apply (simp add: p4_frame_def inv_stack_pt_def p1_post_def p7_pre_noframe_def)
-            apply (simp add: stack_node_def fvA_is_waitq fvA_buf inv_stack_buf_waitq_def Thread_Local_def)
+            apply (simp add: stack_node_def fvA_is_waitq fvA_buf inv_stack_buf_waitq_def )
            apply (simp add: p4_frame_def inv_stack_pt_def p1_post_def p7_pre_noframe_def)
-           apply (simp add: stack_node_def fvA_is_waitq fvA_buf inv_stack_buf_waitq_def Thread_Local_def)
+           apply (simp add: stack_node_def fvA_is_waitq fvA_buf inv_stack_buf_waitq_def )
     apply (rule_tac Q = "p1_post t ** (p7_post_noframe t s st ** p4_frame st)" in rule_seq)
      apply (simp, rule rule_frame1, rule rule_frame, simp add: safe_p7_noframe)
       apply (simp add: p4_frame_def fvA_buf fvA_is_waitq inv_stack_pt_def inv_stack_buf_waitq_def)
-     apply (simp add: p1_post_def, simp add: disjoint_def Thread_Local_def)
+     apply (simp add: p1_post_def, simp add: disjoint_def )
     apply (rule rule_if, rule_tac P = "p7_post_noframe t s st ** p4_frame st" and Q = "p7_post_noframe 
     t s st ** p4_frame st" in rule_conseq, simp add: rule_skip, simp add: p1_post_def, simp_all add: implies_def)
          apply (simp add: p7_post_noframe_def CSL_def) apply auto[1]
-    apply (simp add: Thread_Local_def)
      apply (rule rule_if, drule_tac t =t and s = s and data = d and st = st in safe_p1112, simp_all)
      apply (simp add: p7_post_noframe_def CSL_def) using stm_def apply auto[1]
 (* stack_wait st \<noteq>  NULL *)
@@ -553,35 +552,35 @@ lemma safe_push : "fvAs \<Gamma> = {} \<Longrightarrow>
     stack_buf_waitq_def CSL_def) using stm_def apply auto[1]
     apply (rule_tac Q = "p13_pre_noframe t a st ** inv_stack1 s (st :=\<^sub>w\<^sub>a thd_next a :=\<^sub>t\<^sub>c list)" in rule_seq)
        apply (rule rule_stm_stack', simp_all)
-           apply (simp add: disjoint_def Thread_Local_def)
+           apply (simp add: disjoint_def )
           apply (simp add: p4_frame_def inv_stack_pt_def p1_post_def p7_pre_noframe_def)
-            apply (simp add: stack_node_def fvA_is_waitq fvA_buf inv_stack_buf_waitq_def Thread_Local_def)
+            apply (simp add: stack_node_def fvA_is_waitq fvA_buf inv_stack_buf_waitq_def )
            apply (simp add: p4_frame_def inv_stack_pt_def p1_post_def p7_pre_noframe_def)
-           apply (simp add: stack_node_def fvA_is_waitq fvA_buf inv_stack_buf_waitq_def Thread_Local_def)
+           apply (simp add: stack_node_def fvA_is_waitq fvA_buf inv_stack_buf_waitq_def )
      apply (rule_tac Q = "p1_post t ** (p7_post_noframe t s st ** p4_frame st)" in rule_seq, simp)
       apply (rule rule_frame1, rule rule_frame, simp add: safe_p7_noframe)
        apply (simp add: p4_frame_def fvA_buf fvA_is_waitq inv_stack_pt_def inv_stack_buf_waitq_def)
-      apply (simp add: p1_post_def, simp add: disjoint_def Thread_Local_def)
+      apply (simp add: p1_post_def, simp add: disjoint_def )
         apply (rule rule_if, simp add: p7_post_noframe_def CSL_def) apply auto[1]
-    using safe_p910 apply auto[1] apply (simp add: Thread_Local_def)
+    using safe_p910 apply auto[1] 
      apply (rule rule_if)
      apply (simp add: p13_pre_noframe_def CSL_def) using stm_def apply auto[1]
       apply (rule rule_stm_stack', simp_all)
-          apply (simp add: disjoint_def Thread_Local_def)
-         apply (simp add: p13_pre_noframe_def inv_stack1_def fvA_is_stack Thread_Local_def)
-    apply (simp add: p13_pre_noframe_def inv_stack1_def fvA_is_stack Thread_Local_def)
+          apply (simp add: disjoint_def )
+         apply (simp add: p13_pre_noframe_def inv_stack1_def fvA_is_stack )
+    apply (simp add: p13_pre_noframe_def inv_stack1_def fvA_is_stack )
     apply (rule_tac Q = "p14_post_noframe t d a st ** inv_stack1 s (st :=\<^sub>w\<^sub>a thd_next a :=\<^sub>t\<^sub>c list)" in
     rule_seq) using  safe_p1314 apply auto[1]
        apply (rule rule_with_true, simp, rule rule_inv_readyq, intro allI, simp add: safe_p1517)
-    apply (simp add: Thread_Local_def)
+
      apply (simp add: p4_post_noframe_def p7_pre_noframe_def implies_def) apply blast
-   apply (rule rule_if, rule_tac P = Aemp and Q = "Aemp \<and>\<^sub>S\<^sub>L \<langle>[t\<diamondop>RET]\<^sub>v =\<^sub>b [0]\<^sub>n\<rangle>\<^sub>S\<^sub>L"  in rule_conseq)
+   apply (rule rule_if, rule_tac P = Aemp and Q = "Aemp \<and>\<^sub>S\<^sub>L \<langle>[RET]\<^sub>v =\<^sub>b [0]\<^sub>n\<rangle>\<^sub>S\<^sub>L"  in rule_conseq)
        apply (rule rule_stm_stack', simp_all)
-    apply (simp add: disjoint_def Thread_Local_def)
+    apply (simp add: disjoint_def )
         apply (rule rule_assign_num1, simp add: fvA_Gamma2 fvA_inv_stack fvA_inv_cur fvA_inv_readyq)
-    apply (simp add: Thread_Local_def, simp add: Thread_Local_def)
      apply (simp_all add: implies_def) apply (rule_tac P = Aemp and Q = Aemp in rule_conseq)
-      apply (simp add: rule_skip, simp_all add: implies_def)
+       apply (simp add: rule_skip, simp_all add: implies_def)
+    apply (simp add: fvA_Gamma2 fvA_inv_cur fvA_inv_stack fvA_inv_readyq)
     done
 
 end
