func_cor_scheduler.thy
@@ -3,28 +3,28 @@ theory func_cor_scheduler
 begin
 
 definition s6_pre_noframe :: "nat \<Rightarrow> tcb \<Rightarrow> nat \<Rightarrow> tcb \<Rightarrow> tcbs \<Rightarrow> assn"
-  where "s6_pre_noframe p t r x xs = ((thread_node p t) \<and>\<^sub>S\<^sub>L \<langle>[sched \<diamondop> CUR_RUNNING]\<^sub>v =\<^sub>b [p]\<^sub>n\<rangle>\<^sub>S\<^sub>L \<and>\<^sub>S\<^sub>L 
-  \<langle>[sched \<diamondop> SECOND_READY]\<^sub>v =\<^sub>b [thd_next x]\<^sub>n\<rangle>\<^sub>S\<^sub>L) ** (thread_ready_sl (thd_next x) xs) ** ([A_Readyq]\<^sub>v \<longmapsto> [r]\<^sub>n)"
+  where "s6_pre_noframe p t r x xs = ((thread_node p t) \<and>\<^sub>S\<^sub>L \<langle>[ CUR_RUNNING]\<^sub>v =\<^sub>b [p]\<^sub>n\<rangle>\<^sub>S\<^sub>L \<and>\<^sub>S\<^sub>L 
+  \<langle>[ SECOND_READY]\<^sub>v =\<^sub>b [thd_next x]\<^sub>n\<rangle>\<^sub>S\<^sub>L) ** (thread_ready_sl (thd_next x) xs) ** ([A_Readyq]\<^sub>v \<longmapsto> [r]\<^sub>n)"
 
 definition s6_post :: "nat \<Rightarrow> tcb \<Rightarrow> nat \<Rightarrow> tcb \<Rightarrow> tcbs \<Rightarrow> assn"
-  where "s6_post p t r x xs = ((thread_node p (t :=\<^sub>s\<^sub>t READY)) \<and>\<^sub>S\<^sub>L \<langle>[sched \<diamondop> CUR_RUNNING]\<^sub>v =\<^sub>b [p]\<^sub>n\<rangle>\<^sub>S\<^sub>L \<and>\<^sub>S\<^sub>L 
-  \<langle>[sched \<diamondop> SECOND_READY]\<^sub>v =\<^sub>b [thd_next x]\<^sub>n\<rangle>\<^sub>S\<^sub>L) ** (thread_ready_sl (thd_next x) xs) ** ([A_Readyq]\<^sub>v \<longmapsto> [r]\<^sub>n)"
+  where "s6_post p t r x xs = ((thread_node p (t :=\<^sub>s\<^sub>t READY)) \<and>\<^sub>S\<^sub>L \<langle>[ CUR_RUNNING]\<^sub>v =\<^sub>b [p]\<^sub>n\<rangle>\<^sub>S\<^sub>L \<and>\<^sub>S\<^sub>L 
+  \<langle>[ SECOND_READY]\<^sub>v =\<^sub>b [thd_next x]\<^sub>n\<rangle>\<^sub>S\<^sub>L) ** (thread_ready_sl (thd_next x) xs) ** ([A_Readyq]\<^sub>v \<longmapsto> [r]\<^sub>n)"
 
 definition s7_post :: "nat \<Rightarrow> tcb \<Rightarrow> nat \<Rightarrow> tcb \<Rightarrow> tcbs \<Rightarrow> assn"
   where "s7_post p t r x xs = ((thread_node p ((t :=\<^sub>s\<^sub>t READY) :=\<^sub>n\<^sub>x (thd_next x))) \<and>\<^sub>S\<^sub>L 
-  \<langle>[sched \<diamondop> CUR_RUNNING]\<^sub>v =\<^sub>b [p]\<^sub>n\<rangle>\<^sub>S\<^sub>L \<and>\<^sub>S\<^sub>L  \<langle>[sched \<diamondop> SECOND_READY]\<^sub>v =\<^sub>b [thd_next x]\<^sub>n\<rangle>\<^sub>S\<^sub>L) ** 
+  \<langle>[ CUR_RUNNING]\<^sub>v =\<^sub>b [p]\<^sub>n\<rangle>\<^sub>S\<^sub>L \<and>\<^sub>S\<^sub>L  \<langle>[ SECOND_READY]\<^sub>v =\<^sub>b [thd_next x]\<^sub>n\<rangle>\<^sub>S\<^sub>L) ** 
   (thread_ready_sl (thd_next x) xs) ** ([A_Readyq]\<^sub>v \<longmapsto> [r]\<^sub>n)"
 
 definition s8_pre :: "nat \<Rightarrow> tcb \<Rightarrow> nat \<Rightarrow> tcb \<Rightarrow> tcbs \<Rightarrow> assn"
   where "s8_pre p t r x xs = (thread_node p ((t :=\<^sub>s\<^sub>t READY) :=\<^sub>n\<^sub>x (thd_next x))) ** 
-  (thread_ready_sl (thd_next x) xs) ** ([A_Readyq]\<^sub>v \<longmapsto> [r]\<^sub>n \<and>\<^sub>S\<^sub>L \<langle>[sched \<diamondop> CUR_RUNNING]\<^sub>v =\<^sub>b [p]\<^sub>n\<rangle>\<^sub>S\<^sub>L)"
+  (thread_ready_sl (thd_next x) xs) ** ([A_Readyq]\<^sub>v \<longmapsto> [r]\<^sub>n \<and>\<^sub>S\<^sub>L \<langle>[ CUR_RUNNING]\<^sub>v =\<^sub>b [p]\<^sub>n\<rangle>\<^sub>S\<^sub>L)"
 
 lemma s7_post_implies : "s7_post p t r x xs \<sqsubseteq> s8_pre p t r x xs"
    apply (simp add: s7_post_def s8_pre_def implies_def) by blast
 
 definition s8_post :: "nat \<Rightarrow> tcb \<Rightarrow> nat \<Rightarrow> tcb \<Rightarrow> tcbs \<Rightarrow> assn"
   where "s8_post p t r x xs = (thread_node p ((t :=\<^sub>s\<^sub>t READY) :=\<^sub>n\<^sub>x (thd_next x))) ** 
-  (thread_ready_sl (thd_next x) xs) ** ([A_Readyq]\<^sub>v \<longmapsto> [p]\<^sub>n \<and>\<^sub>S\<^sub>L \<langle>[sched \<diamondop> CUR_RUNNING]\<^sub>v =\<^sub>b [p]\<^sub>n\<rangle>\<^sub>S\<^sub>L)"
+  (thread_ready_sl (thd_next x) xs) ** ([A_Readyq]\<^sub>v \<longmapsto> [p]\<^sub>n \<and>\<^sub>S\<^sub>L \<langle>[ CUR_RUNNING]\<^sub>v =\<^sub>b [p]\<^sub>n\<rangle>\<^sub>S\<^sub>L)"
 
 lemma s8_post_implies : "s8_post p t r x xs \<sqsubseteq> inv_readyq1 p ((Suc K_NO_WAIT, thd_next x, thd_data t) # xs)"
   apply (rule_tac Q = "(thread_node p ((t :=\<^sub>s\<^sub>t READY) :=\<^sub>n\<^sub>x (thd_next x))) ** (thread_ready_sl 
@@ -46,16 +46,16 @@ lemma s8_post_implies : "s8_post p t r x xs \<sqsubseteq> inv_readyq1 p ((Suc K_
 lemma safe_s68_noframe: "fvAs \<Gamma> = {} \<Longrightarrow>  
          \<Gamma>(Stack := inv_stack, Readyq := Aemp, Cur := Aemp) \<turnstile> 
               {s6_pre_noframe p t r x xs}
-             \<lbrakk>[sched \<diamondop> CUR_RUNNING]\<^sub>v\<Down>\<^sub>tstate\<rbrakk> :=\<^sub>C [READY]\<^sub>n ;;
-             \<lbrakk>[sched \<diamondop> CUR_RUNNING]\<^sub>v\<Down>\<^sub>tnext\<rbrakk> :=\<^sub>C [sched \<diamondop> SECOND_READY]\<^sub>v;;
-             \<lbrakk>[A_Readyq]\<^sub>v\<rbrakk> :=\<^sub>C [sched \<diamondop> CUR_RUNNING]\<^sub>v 
+             \<lbrakk>[ CUR_RUNNING]\<^sub>v\<Down>\<^sub>tstate\<rbrakk> :=\<^sub>C [READY]\<^sub>n ;;
+             \<lbrakk>[ CUR_RUNNING]\<^sub>v\<Down>\<^sub>tnext\<rbrakk> :=\<^sub>C [ SECOND_READY]\<^sub>v;;
+             \<lbrakk>[A_Readyq]\<^sub>v\<rbrakk> :=\<^sub>C [ CUR_RUNNING]\<^sub>v 
              {inv_readyq1 p ((READY, thd_next x, thd_data t) # xs)}"
    apply (rule_tac Q = "s7_post p t r x xs" in rule_seq)
     apply (rule_tac Q = "s6_post p t r x xs" in rule_seq)
      apply (simp add: s6_pre_noframe_def s6_post_def, intro rule_frame)
-  apply (rule_tac Pa = "(thread_node p t \<and>\<^sub>S\<^sub>L \<langle>[sched \<diamondop>CUR_RUNNING]\<^sub>v =\<^sub>b [p]\<^sub>n\<rangle>\<^sub>S\<^sub>L) ** (\<langle>[sched \<diamondop>SECOND_READY]\<^sub>v =\<^sub>b
-   [thd_next x]\<^sub>n\<rangle>\<^sub>S\<^sub>L \<and>\<^sub>S\<^sub>L Aemp)" and Qa = "(thread_node p (t :=\<^sub>s\<^sub>t READY) \<and>\<^sub>S\<^sub>L \<langle>[sched \<diamondop>CUR_RUNNING]\<^sub>v =\<^sub>b [p]\<^sub>n\<rangle>\<^sub>S\<^sub>L) 
-   ** (\<langle>[sched \<diamondop>SECOND_READY]\<^sub>v =\<^sub>b [thd_next x]\<^sub>n\<rangle>\<^sub>S\<^sub>L \<and>\<^sub>S\<^sub>L Aemp)"in safe_assn_equiv)
+  apply (rule_tac Pa = "(thread_node p t \<and>\<^sub>S\<^sub>L \<langle>[CUR_RUNNING]\<^sub>v =\<^sub>b [p]\<^sub>n\<rangle>\<^sub>S\<^sub>L) ** (\<langle>[SECOND_READY]\<^sub>v =\<^sub>b
+   [thd_next x]\<^sub>n\<rangle>\<^sub>S\<^sub>L \<and>\<^sub>S\<^sub>L Aemp)" and Qa = "(thread_node p (t :=\<^sub>s\<^sub>t READY) \<and>\<^sub>S\<^sub>L \<langle>[CUR_RUNNING]\<^sub>v =\<^sub>b [p]\<^sub>n\<rangle>\<^sub>S\<^sub>L) 
+   ** (\<langle>[SECOND_READY]\<^sub>v =\<^sub>b [thd_next x]\<^sub>n\<rangle>\<^sub>S\<^sub>L \<and>\<^sub>S\<^sub>L Aemp)"in safe_assn_equiv)
          apply (simp add: assn_equiv_def, simp add: assn_equiv_def)
        apply (rule rule_frame, simp add: thread_node_write_st', simp_all)
     apply (simp add: s6_post_def s7_post_def, intro rule_frame,simp add: thread_node_write_next_fromvar, simp_all)
@@ -80,14 +80,14 @@ lemma rule_inv_pre: "\<forall>p t. \<Gamma> \<turnstile> {P ** inv_cur1 p t} C {
   apply (simp add: CSL_def) by blast
 
 definition s1_post :: "nat \<Rightarrow> tcbs \<Rightarrow> assn"
-  where "s1_post r xs = ([A_Readyq]\<^sub>v \<longmapsto> [r]\<^sub>n \<and>\<^sub>S\<^sub>L \<langle>[sched \<diamondop> FIRST_READY]\<^sub>v =\<^sub>b [r]\<^sub>n \<rangle>\<^sub>S\<^sub>L) ** 
+  where "s1_post r xs = ([A_Readyq]\<^sub>v \<longmapsto> [r]\<^sub>n \<and>\<^sub>S\<^sub>L \<langle>[ FIRST_READY]\<^sub>v =\<^sub>b [r]\<^sub>n \<rangle>\<^sub>S\<^sub>L) ** 
         (is_readyq r xs)"
 
-lemma s1_post_implies : "(s1_post r xs \<and>\<^sub>S\<^sub>L \<langle>[sched \<diamondop>FIRST_READY]\<^sub>v =\<^sub>b [K_NO_WAIT]\<^sub>n\<rangle>\<^sub>S\<^sub>L) \<sqsubseteq> inv_readyq1 r xs"
+lemma s1_post_implies : "(s1_post r xs \<and>\<^sub>S\<^sub>L \<langle>[FIRST_READY]\<^sub>v =\<^sub>b [K_NO_WAIT]\<^sub>n\<rangle>\<^sub>S\<^sub>L) \<sqsubseteq> inv_readyq1 r xs"
   apply (simp add: s1_post_def inv_readyq1_def implies_def) by auto
 
 definition s3_pre :: "nat \<Rightarrow> tcb \<Rightarrow> tcbs \<Rightarrow> assn"
-  where "s3_pre r a list = ([A_Readyq]\<^sub>v \<longmapsto> [r]\<^sub>n) ** (thread_node r a \<and>\<^sub>S\<^sub>L \<langle>[sched \<diamondop> FIRST_READY]\<^sub>v =\<^sub>b 
+  where "s3_pre r a list = ([A_Readyq]\<^sub>v \<longmapsto> [r]\<^sub>n) ** (thread_node r a \<and>\<^sub>S\<^sub>L \<langle>[ FIRST_READY]\<^sub>v =\<^sub>b 
   [r]\<^sub>n \<rangle>\<^sub>S\<^sub>L) ** (thread_ready_sl (thd_next a) list)"
 
 lemma s3_pre_implies_aux : "(P1 \<and>\<^sub>S\<^sub>L \<langle>P2\<rangle>\<^sub>S\<^sub>L) ** (P3 ** P4) \<equiv>\<^sub>S\<^sub>L P1 ** (P3 \<and>\<^sub>S\<^sub>L \<langle>P2\<rangle>\<^sub>S\<^sub>L) ** P4"
@@ -98,21 +98,21 @@ lemma s3_pre_implies_aux : "(P1 \<and>\<^sub>S\<^sub>L \<langle>P2\<rangle>\<^su
    apply (simp add: assn_equiv_reflex, simp add: assn_equiv_def)
   by auto
 
-lemma s3_pre_implies : "xs = a # list \<Longrightarrow> (s1_post r xs \<and>\<^sub>S\<^sub>L \<langle>\<not>\<^sub>b [sched \<diamondop>FIRST_READY]\<^sub>v =\<^sub>b [K_NO_WAIT]\<^sub>n\<rangle>\<^sub>S\<^sub>L) 
+lemma s3_pre_implies : "xs = a # list \<Longrightarrow> (s1_post r xs \<and>\<^sub>S\<^sub>L \<langle>\<not>\<^sub>b [FIRST_READY]\<^sub>v =\<^sub>b [K_NO_WAIT]\<^sub>n\<rangle>\<^sub>S\<^sub>L) 
                        \<sqsubseteq> s3_pre r a list"
   apply (rule_tac Q = "s1_post r xs" in implies_trans, simp add: implies_def)
-  apply (rule_tac Q = "([A_Readyq]\<^sub>v \<longmapsto> [r]\<^sub>n \<and>\<^sub>S\<^sub>L \<langle>[sched \<diamondop> FIRST_READY]\<^sub>v =\<^sub>b [r]\<^sub>n \<rangle>\<^sub>S\<^sub>L) ** 
+  apply (rule_tac Q = "([A_Readyq]\<^sub>v \<longmapsto> [r]\<^sub>n \<and>\<^sub>S\<^sub>L \<langle>[ FIRST_READY]\<^sub>v =\<^sub>b [r]\<^sub>n \<rangle>\<^sub>S\<^sub>L) ** 
         (thread_ready_sl r (a # list))" in implies_trans, simp add: s1_post_def)
    apply (rule equiv_implies, rule assn_equiv_cong_star)
     apply (simp add: assn_equiv_reflex, simp add: readyq_equiv)
-  apply (rule_tac Q = "([A_Readyq]\<^sub>v \<longmapsto> [r]\<^sub>n \<and>\<^sub>S\<^sub>L \<langle>[sched \<diamondop> FIRST_READY]\<^sub>v =\<^sub>b [r]\<^sub>n \<rangle>\<^sub>S\<^sub>L) ** 
+  apply (rule_tac Q = "([A_Readyq]\<^sub>v \<longmapsto> [r]\<^sub>n \<and>\<^sub>S\<^sub>L \<langle>[ FIRST_READY]\<^sub>v =\<^sub>b [r]\<^sub>n \<rangle>\<^sub>S\<^sub>L) ** 
   ((thread_node r a ) ** (thread_ready_sl (thd_next a) list))" in implies_trans)
    apply (rule implies_star, simp add: implies_def, simp add: ready_sl_implies)
   by (rule equiv_implies, simp add: s3_pre_def, simp add: s3_pre_implies_aux)
 
 definition s3_post :: "nat \<Rightarrow> tcb \<Rightarrow> tcbs \<Rightarrow> assn"
-  where "s3_post r a list = ([A_Readyq]\<^sub>v \<longmapsto> [r]\<^sub>n) ** (thread_node r a \<and>\<^sub>S\<^sub>L \<langle>[sched \<diamondop> FIRST_READY]\<^sub>v =\<^sub>b 
-  [r]\<^sub>n \<rangle>\<^sub>S\<^sub>L \<and>\<^sub>S\<^sub>L \<langle>[sched \<diamondop> SECOND_READY]\<^sub>v =\<^sub>b [thd_next a]\<^sub>n\<rangle>\<^sub>S\<^sub>L) ** (thread_ready_sl (thd_next a) list)"
+  where "s3_post r a list = ([A_Readyq]\<^sub>v \<longmapsto> [r]\<^sub>n) ** (thread_node r a \<and>\<^sub>S\<^sub>L \<langle>[ FIRST_READY]\<^sub>v =\<^sub>b 
+  [r]\<^sub>n \<rangle>\<^sub>S\<^sub>L \<and>\<^sub>S\<^sub>L \<langle>[ SECOND_READY]\<^sub>v =\<^sub>b [thd_next a]\<^sub>n\<rangle>\<^sub>S\<^sub>L) ** (thread_ready_sl (thd_next a) list)"
 
 definition s4_pre1 :: "nat \<Rightarrow> tcb \<Rightarrow> tcbs \<Rightarrow> assn"
   where "s4_pre1 r a list = (s3_post r a list) ** ([A_Cur]\<^sub>v \<longmapsto> [NULL]\<^sub>n)"
@@ -121,19 +121,19 @@ definition s4_pre2 :: "nat \<Rightarrow> tcb \<Rightarrow> tcbs \<Rightarrow> as
   where "s4_pre2 r a list = (s3_post r a list) ** (Aexcur inv_cur1)"
 
 definition s4_post1 :: "nat \<Rightarrow> tcb \<Rightarrow> tcbs \<Rightarrow> assn"
-  where "s4_post1 r a list = (s3_post r a list) ** ([A_Cur]\<^sub>v \<longmapsto> [NULL]\<^sub>n \<and>\<^sub>S\<^sub>L \<langle>[sched \<diamondop>CUR_RUNNING]\<^sub>v 
+  where "s4_post1 r a list = (s3_post r a list) ** ([A_Cur]\<^sub>v \<longmapsto> [NULL]\<^sub>n \<and>\<^sub>S\<^sub>L \<langle>[CUR_RUNNING]\<^sub>v 
   =\<^sub>b [NULL]\<^sub>n\<rangle>\<^sub>S\<^sub>L)"
 
 definition s4_post2 :: "nat \<Rightarrow> tcb \<Rightarrow> tcbs \<Rightarrow> nat \<Rightarrow> tcb \<Rightarrow> assn"
-  where "s4_post2 r a list p t = (s3_post r a list) ** (([A_Cur]\<^sub>v \<longmapsto> [p]\<^sub>n \<and>\<^sub>S\<^sub>L \<langle>[sched \<diamondop>CUR_RUNNING]\<^sub>v 
+  where "s4_post2 r a list p t = (s3_post r a list) ** (([A_Cur]\<^sub>v \<longmapsto> [p]\<^sub>n \<and>\<^sub>S\<^sub>L \<langle>[CUR_RUNNING]\<^sub>v 
   =\<^sub>b [p]\<^sub>n\<rangle>\<^sub>S\<^sub>L) ** thread_node p t)"
 
 definition s5_frame :: "nat \<Rightarrow> tcb \<Rightarrow> tcbs  \<Rightarrow> assn"
-  where "s5_frame r x xs  = ((thread_node r x) \<and>\<^sub>S\<^sub>L \<langle>[sched \<diamondop> FIRST_READY]\<^sub>v =\<^sub>b [r]\<^sub>n\<rangle>\<^sub>S\<^sub>L) ** 
+  where "s5_frame r x xs  = ((thread_node r x) \<and>\<^sub>S\<^sub>L \<langle>[ FIRST_READY]\<^sub>v =\<^sub>b [r]\<^sub>n\<rangle>\<^sub>S\<^sub>L) ** 
         thread_ready_sl (thd_next x) xs ** ([A_Cur]\<^sub>v \<longmapsto> [NULL]\<^sub>n)"
 
 definition s5_pre :: "nat \<Rightarrow> tcb \<Rightarrow> tcbs \<Rightarrow> assn"
-  where "s5_pre r a list = ([A_Readyq]\<^sub>v \<longmapsto> [r]\<^sub>n \<and>\<^sub>S\<^sub>L \<langle>[sched \<diamondop> SECOND_READY]\<^sub>v =\<^sub>b 
+  where "s5_pre r a list = ([A_Readyq]\<^sub>v \<longmapsto> [r]\<^sub>n \<and>\<^sub>S\<^sub>L \<langle>[ SECOND_READY]\<^sub>v =\<^sub>b 
   [thd_next a]\<^sub>n\<rangle>\<^sub>S\<^sub>L) ** s5_frame r a list"
 
 lemma s5_pre_implies_aux : "P1 ** (P2 \<and>\<^sub>S\<^sub>L \<langle>P3\<rangle>\<^sub>S\<^sub>L \<and>\<^sub>S\<^sub>L \<langle>P4\<rangle>\<^sub>S\<^sub>L) ** P5 ** P6 \<equiv>\<^sub>S\<^sub>L
@@ -144,23 +144,23 @@ lemma s5_pre_implies_aux : "P1 ** (P2 \<and>\<^sub>S\<^sub>L \<langle>P3\<rangle
    apply (rule assn_equiv_cong_conj, simp add: stack_node_equiv1_aux)
    apply (simp add: assn_equiv_reflex, simp add: assn_equiv_def) by blast
 
-lemma s5_pre_implies : "(s4_post1 r a list \<and>\<^sub>S\<^sub>L \<langle>[sched \<diamondop>CUR_RUNNING]\<^sub>v =\<^sub>b [K_NO_WAIT]\<^sub>n\<rangle>\<^sub>S\<^sub>L) \<sqsubseteq> s5_pre r a list"
+lemma s5_pre_implies : "(s4_post1 r a list \<and>\<^sub>S\<^sub>L \<langle>[CUR_RUNNING]\<^sub>v =\<^sub>b [K_NO_WAIT]\<^sub>n\<rangle>\<^sub>S\<^sub>L) \<sqsubseteq> s5_pre r a list"
   apply (rule_tac Q = "s4_post1 r a list" in implies_trans, simp add: implies_def)
   apply (simp add: s4_post1_def s3_post_def s5_pre_def s5_frame_def)
-  apply (rule_tac Q = "[A_Readyq]\<^sub>v \<longmapsto> [r]\<^sub>n ** (thread_node r a \<and>\<^sub>S\<^sub>L \<langle>[sched \<diamondop>FIRST_READY]\<^sub>v =\<^sub>b [r]\<^sub>n\<rangle>\<^sub>S\<^sub>L 
-  \<and>\<^sub>S\<^sub>L \<langle>[sched \<diamondop>SECOND_READY]\<^sub>v =\<^sub>b [thd_next a]\<^sub>n\<rangle>\<^sub>S\<^sub>L) ** thread_ready_sl (thd_next a) list **
+  apply (rule_tac Q = "[A_Readyq]\<^sub>v \<longmapsto> [r]\<^sub>n ** (thread_node r a \<and>\<^sub>S\<^sub>L \<langle>[FIRST_READY]\<^sub>v =\<^sub>b [r]\<^sub>n\<rangle>\<^sub>S\<^sub>L 
+  \<and>\<^sub>S\<^sub>L \<langle>[SECOND_READY]\<^sub>v =\<^sub>b [thd_next a]\<^sub>n\<rangle>\<^sub>S\<^sub>L) ** thread_ready_sl (thd_next a) list **
   ([A_Cur]\<^sub>v \<longmapsto> [NULL]\<^sub>n)" in implies_trans, simp add: implies_def) apply auto[1]
   by (rule equiv_implies, simp add: s5_pre_implies_aux) 
   
 definition s5_post :: "nat \<Rightarrow> tcb \<Rightarrow> tcbs \<Rightarrow> assn"
-  where "s5_post r a list = ([A_Readyq]\<^sub>v \<longmapsto> [thd_next a]\<^sub>n \<and>\<^sub>S\<^sub>L \<langle>[sched \<diamondop> SECOND_READY]\<^sub>v =\<^sub>b 
+  where "s5_post r a list = ([A_Readyq]\<^sub>v \<longmapsto> [thd_next a]\<^sub>n \<and>\<^sub>S\<^sub>L \<langle>[ SECOND_READY]\<^sub>v =\<^sub>b 
   [thd_next a]\<^sub>n\<rangle>\<^sub>S\<^sub>L) ** s5_frame r a list"
 
 lemma s5_post_implies : " s5_post r a list \<sqsubseteq> [A_Readyq]\<^sub>v \<longmapsto> [thd_next a]\<^sub>n ** s5_frame r a list"
   apply (simp add: s5_post_def implies_def) by auto
 
 definition s6_frame :: "nat \<Rightarrow> tcb \<Rightarrow> nat \<Rightarrow> assn"
-  where "s6_frame r a p = ((thread_node r a) ** ([A_Cur]\<^sub>v \<longmapsto> [p]\<^sub>n) \<and>\<^sub>S\<^sub>L \<langle>[sched \<diamondop> FIRST_READY]\<^sub>v 
+  where "s6_frame r a p = ((thread_node r a) ** ([A_Cur]\<^sub>v \<longmapsto> [p]\<^sub>n) \<and>\<^sub>S\<^sub>L \<langle>[ FIRST_READY]\<^sub>v 
   =\<^sub>b [r]\<^sub>n\<rangle>\<^sub>S\<^sub>L)"
 
 lemma s6_pre_frame_implies_aux : "P1 ** (P2 \<and>\<^sub>S\<^sub>L \<langle>P3\<rangle>\<^sub>S\<^sub>L \<and>\<^sub>S\<^sub>L \<langle>P4\<rangle>\<^sub>S\<^sub>L) ** P5 ** ((P6 \<and>\<^sub>S\<^sub>L \<langle>P7\<rangle>\<^sub>S\<^sub>L) ** P8) \<equiv>\<^sub>S\<^sub>L
@@ -174,7 +174,7 @@ lemma s6_pre_frame_implies_aux : "P1 ** (P2 \<and>\<^sub>S\<^sub>L \<langle>P3\<
     apply (meson Astar_assoc_equiv assn_equiv_cong_star assn_equiv_reflex assn_equiv_symmetry assn_equiv_trans)
    apply (simp add: assn_equiv_reflex, simp add: assn_equiv_def) by auto
 
-lemma s6_pre_frame_implies : "(s4_post2 r a list p t \<and>\<^sub>S\<^sub>L \<langle>\<not>\<^sub>b [sched \<diamondop>CUR_RUNNING]\<^sub>v =\<^sub>b [K_NO_WAIT]\<^sub>n\<rangle>\<^sub>S\<^sub>L) 
+lemma s6_pre_frame_implies : "(s4_post2 r a list p t \<and>\<^sub>S\<^sub>L \<langle>\<not>\<^sub>b [CUR_RUNNING]\<^sub>v =\<^sub>b [K_NO_WAIT]\<^sub>n\<rangle>\<^sub>S\<^sub>L) 
       \<sqsubseteq> s6_pre_noframe p t r a list ** s6_frame r a p"
   apply (rule_tac Q = "s4_post2 r a list p t" in implies_trans, simp add: implies_def)
   apply (rule equiv_implies, simp add: s4_post2_def s3_post_def s6_pre_noframe_def s6_frame_def)
@@ -189,7 +189,7 @@ definition s9_frame2 :: "nat \<Rightarrow> tcb \<Rightarrow> tcb \<Rightarrow> t
         # xs))"
 
 definition s9_pre_noframe :: "nat \<Rightarrow> tcb \<Rightarrow> nat \<Rightarrow> assn"
-  where "s9_pre_noframe r x p = (thread_node r x \<and>\<^sub>S\<^sub>L \<langle>[sched \<diamondop> FIRST_READY]\<^sub>v =\<^sub>b [r]\<^sub>n\<rangle>\<^sub>S\<^sub>L) 
+  where "s9_pre_noframe r x p = (thread_node r x \<and>\<^sub>S\<^sub>L \<langle>[ FIRST_READY]\<^sub>v =\<^sub>b [r]\<^sub>n\<rangle>\<^sub>S\<^sub>L) 
                           ** ([A_Cur]\<^sub>v \<longmapsto> [p]\<^sub>n)"
 
 lemma s9_pre_frame1_equiv : "s9_pre_noframe r a NULL ** s9_frame1 r a list  \<equiv>\<^sub>S\<^sub>L 
@@ -199,30 +199,30 @@ lemma s9_pre_frame1_equiv : "s9_pre_noframe r a NULL ** s9_frame1 r a list  \<eq
       stack_node_equiv2_aux)
 
 definition s10_pre_noframe :: "nat \<Rightarrow> tcb \<Rightarrow> nat \<Rightarrow> assn"
-  where "s10_pre_noframe r x p = (thread_node r (x :=\<^sub>s\<^sub>t RUNNING) \<and>\<^sub>S\<^sub>L \<langle>[sched \<diamondop> FIRST_READY]\<^sub>v =\<^sub>b [r]\<^sub>n\<rangle>\<^sub>S\<^sub>L)
+  where "s10_pre_noframe r x p = (thread_node r (x :=\<^sub>s\<^sub>t RUNNING) \<and>\<^sub>S\<^sub>L \<langle>[ FIRST_READY]\<^sub>v =\<^sub>b [r]\<^sub>n\<rangle>\<^sub>S\<^sub>L)
         ** ([A_Cur]\<^sub>v \<longmapsto> [p]\<^sub>n)"
 
 lemma safe_s9_noframe : "fvAs \<Gamma> = {} \<Longrightarrow>
                         \<Gamma>(Stack := inv_stack, Readyq := Aemp,Cur :=Aemp) \<turnstile> 
                         { s9_pre_noframe r a p } 
-                        \<lbrakk>[sched \<diamondop>FIRST_READY]\<^sub>v\<Down>\<^sub>tstate\<rbrakk> :=\<^sub>C [EAGAIN]\<^sub>n 
+                        \<lbrakk>[FIRST_READY]\<^sub>v\<Down>\<^sub>tstate\<rbrakk> :=\<^sub>C [EAGAIN]\<^sub>n 
                         { s10_pre_noframe r a p}"
   apply (simp add: s9_pre_noframe_def s10_pre_noframe_def)
   by (rule rule_frame, simp add: thread_node_write_st', simp add: disjoint_def)
 
 definition s10_post_noframe :: "nat \<Rightarrow> tcb \<Rightarrow> assn"
-  where "s10_post_noframe r x  = (thread_node r (x :=\<^sub>s\<^sub>t RUNNING) \<and>\<^sub>S\<^sub>L \<langle>[sched \<diamondop> FIRST_READY]\<^sub>v =\<^sub>b [r]\<^sub>n\<rangle>\<^sub>S\<^sub>L)
+  where "s10_post_noframe r x  = (thread_node r (x :=\<^sub>s\<^sub>t RUNNING) \<and>\<^sub>S\<^sub>L \<langle>[ FIRST_READY]\<^sub>v =\<^sub>b [r]\<^sub>n\<rangle>\<^sub>S\<^sub>L)
         ** ([A_Cur]\<^sub>v \<longmapsto> [r]\<^sub>n)"
 
 lemma safe_s10_noframe : "fvAs \<Gamma> = {} \<Longrightarrow>
          \<Gamma>(Stack := inv_stack, Readyq := Aemp, Cur := Aemp) \<turnstile> 
          { s10_pre_noframe r a p } 
-        \<lbrakk>[A_Cur]\<^sub>v\<rbrakk> :=\<^sub>C [sched \<diamondop>FIRST_READY]\<^sub>v 
+        \<lbrakk>[A_Cur]\<^sub>v\<rbrakk> :=\<^sub>C [FIRST_READY]\<^sub>v 
         { s10_post_noframe r a}"
   apply (simp add: s10_pre_noframe_def s10_post_noframe_def)
-  apply (rule_tac Pa = "(([A_Cur]\<^sub>v \<longmapsto>[p]\<^sub>n) \<and>\<^sub>S\<^sub>L \<langle>[sched \<diamondop>FIRST_READY]\<^sub>v =\<^sub>b [r]\<^sub>n\<rangle>\<^sub>S\<^sub>L) 
+  apply (rule_tac Pa = "(([A_Cur]\<^sub>v \<longmapsto>[p]\<^sub>n) \<and>\<^sub>S\<^sub>L \<langle>[FIRST_READY]\<^sub>v =\<^sub>b [r]\<^sub>n\<rangle>\<^sub>S\<^sub>L) 
          ** (thread_node r (a :=\<^sub>s\<^sub>t RUNNING))" and Qa = "(([A_Cur]\<^sub>v \<longmapsto>[r]\<^sub>n) 
-         \<and>\<^sub>S\<^sub>L \<langle>[sched \<diamondop>FIRST_READY]\<^sub>v =\<^sub>b [r]\<^sub>n\<rangle>\<^sub>S\<^sub>L)** (thread_node r (a :=\<^sub>s\<^sub>t RUNNING))" in safe_assn_equiv)
+         \<and>\<^sub>S\<^sub>L \<langle>[FIRST_READY]\<^sub>v =\<^sub>b [r]\<^sub>n\<rangle>\<^sub>S\<^sub>L)** (thread_node r (a :=\<^sub>s\<^sub>t RUNNING))" in safe_assn_equiv)
      apply (simp add: assn_equiv_def) using disjoint_search(1) map_add_commute apply blast
    apply (simp add: assn_equiv_def) using disjoint_search(1) map_add_commute apply blast
   by (simp add: rule_frame rule_write_var2)
@@ -270,13 +270,14 @@ lemma s10_post_frame2_implies : " s10_post_noframe r a ** s9_frame2 p t a list \
 lemma safe_scheduler : "fvAs \<Gamma> = {} \<Longrightarrow> 
                       \<Gamma>(Cur := inv_cur, Readyq := inv_readyq, Stack := inv_stack) \<turnstile>
                       {Aemp} scheduler {Aemp}"
+  apply (rule rule_Clocals)
   apply (rule rule_with_true', simp) 
   apply (rule_tac Pa = "inv_readyq" and Qa = "inv_readyq" in safe_assn_equiv)
     apply (simp add: assn_equiv_def, simp add: assn_equiv_def)
   apply (rule rule_inv_readyq, intro allI)
   apply (rule_tac Q = "s1_post r xs" in rule_seq, simp add: inv_readyq1_def s1_post_def)
    apply (rule rule_frame, rule rule_read)
-    apply (simp add: fvA_Gamma fvA_inv_cur fvA_inv_stack sched_local_def)
+    apply (simp add: fvA_Gamma fvA_inv_cur fvA_inv_stack)
    apply (simp add: fvA_is_readyq)
   apply (rule rule_if)
 (* Readyq = NULL *)
@@ -288,10 +289,10 @@ lemma safe_scheduler : "fvAs \<Gamma> = {} \<Longrightarrow>
   apply (rule_tac Q = "s3_post r a list" in rule_seq)
    apply (rule_tac P = "s3_pre r a list" and Q = "s3_post r a list" in rule_conseq)
   apply (simp only: s3_pre_def s3_post_def, rule rule_frame, rule rule_frame1)
-       apply (rule thread_node_readnext, simp add: sched_local_def)
-        apply (simp add: fvA_Gamma fvA_inv_cur fvA_inv_stack sched_local_def)
-       apply (simp add: fvA_Gamma fvA_inv_cur fvA_inv_stack sched_local_def)
-      apply (simp add: disjoint_def sched_local_def, simp add: fvA_thread_ready_sl)
+       apply (rule thread_node_readnext, simp)
+        apply (simp add: fvA_Gamma fvA_inv_cur fvA_inv_stack)
+       apply (simp add: fvA_Gamma fvA_inv_cur fvA_inv_stack)
+      apply (simp add: disjoint_def, simp add: fvA_thread_ready_sl)
     apply (simp add: s3_pre_implies, simp add: implies_def)
   apply (rule rule_with_true', simp)
     apply (rule_tac Pa = "(s4_pre1 r a list) \<or>\<^sub>S\<^sub>L (s4_pre2 r a list)" and Qa = "(inv_readyq ** inv_cur)
@@ -304,8 +305,8 @@ lemma safe_scheduler : "fvAs \<Gamma> = {} \<Longrightarrow>
     apply (rule_tac Q = "[A_Readyq]\<^sub>v \<longmapsto> [thd_next a]\<^sub>n ** s5_frame r a list " in rule_seq)
      apply (rule_tac Q = "s4_post1 r a list" in rule_seq, simp add: s4_post1_def s4_pre1_def)
       apply (rule rule_frame1, rule rule_read)
-       apply (simp add: fvA_Gamma1 fvA_inv_stack fvA_inv_cur sched_local_def)
-      apply (simp add: s3_post_def fvA_thread_ready_sl disjoint_def sched_local_def)
+       apply (simp add: fvA_Gamma1 fvA_inv_stack fvA_inv_cur)
+      apply (simp add: s3_post_def fvA_thread_ready_sl disjoint_def)
   apply (rule rule_if)
       apply (rule_tac P = "s5_pre r a list" and Q = "s5_post r a list" in rule_conseq)
         apply (simp add: s5_pre_def s5_post_def, rule rule_frame)
@@ -327,10 +328,10 @@ lemma safe_scheduler : "fvAs \<Gamma> = {} \<Longrightarrow>
     apply (rule_tac Q = "s4_post2 r a list p t" in rule_seq, simp add: s4_post2_def)
      apply (rule rule_frame1, simp add: inv_cur1_def is_cur_def)
   apply (rule_tac P = "[A_Cur]\<^sub>v \<longmapsto> [p]\<^sub>n **  (thread_node p t)" and Q = "([A_Cur]\<^sub>v \<longmapsto> [p]\<^sub>n \<and>\<^sub>S\<^sub>L 
-  \<langle>[sched \<diamondop>CUR_RUNNING]\<^sub>v =\<^sub>b [p]\<^sub>n\<rangle>\<^sub>S\<^sub>L) ** thread_node p t" in rule_conseq)
-        apply (rule rule_frame, rule rule_read, simp add: fvA_Gamma1 fvA_inv_stack sched_local_def)
+  \<langle>[CUR_RUNNING]\<^sub>v =\<^sub>b [p]\<^sub>n\<rangle>\<^sub>S\<^sub>L) ** thread_node p t" in rule_conseq)
+        apply (rule rule_frame, rule rule_read, simp add: fvA_Gamma1 fvA_inv_stack)
         apply (simp add: fvA_thread_node, simp add: implies_def) apply auto[1]
-      apply (simp add: implies_def, simp add: s3_post_def fvA_thread_ready_sl disjoint_def sched_local_def)
+      apply (simp add: implies_def, simp add: s3_post_def fvA_thread_ready_sl disjoint_def)
     apply (rule rule_if, simp add: s4_post2_def, case_tac p, simp add: CSL_def)
      apply (simp add: CSL_def) using stm_def apply linarith
   apply (rule_tac P = "s6_pre_noframe p t r a list ** s6_frame r a p" and Q = "inv_readyq1 p ((READY, 
@@ -342,7 +343,8 @@ lemma safe_scheduler : "fvAs \<Gamma> = {} \<Longrightarrow>
   ** s9_frame2 p t a list" in rule_conseq)
     apply (rule rule_frame, simp add: safe_s10_noframe)
     apply (simp, simp add: implies_def)
-  apply (simp add: s10_post_frame2_implies)
+   apply (simp add: s10_post_frame2_implies)
+  apply (simp add: fvA_Gamma2 fvA_inv_cur fvA_inv_stack fvA_inv_readyq)
   done
 
 end
