Syntax_text.thy
@@ -1,6 +1,0 @@
-theory Syntax_text
-  imports Syntax
-begin
-
-
-lemma "Cresource Cpar (CSkip) (CSkip)"
